<?xml version="1.0"?>
<!DOCTYPE rdf:RDF [
        <!ENTITY dcterms "http://purl.org/dc/terms/" >
        <!ENTITY foaf "http://xmlns.com/foaf/0.1/" >
        <!ENTITY vann "http://purl.org/vocab/vann/" >
        <!ENTITY cc "http://creativecommons.org/ns#" >
        <!ENTITY owl "http://www.w3.org/2002/07/owl#" >
        <!ENTITY xsd "http://www.w3.org/2001/XMLSchema#" >
        <!ENTITY wdrs "http://www.w3.org/2007/05/powder-s#" >
        <!ENTITY skos "http://www.w3.org/2004/02/skos/core#" >
        <!ENTITY xml "http://www.w3.org/XML/1998/namespace" >
        <!ENTITY rdfs "http://www.w3.org/2000/01/rdf-schema#" >
        <!ENTITY rdf "http://www.w3.org/1999/02/22-rdf-syntax-ns#" >
        ]>
<rdf:RDF xmlns="http://www.semanticweb.org/owl/owlapi/turtle#"
         xml:base="http://www.semanticweb.org/owl/owlapi/turtle"
         xmlns:foaf="http://xmlns.com/foaf/0.1/"
         xmlns:vann="http://purl.org/vocab/vann/"
         xmlns:xml="http://www.w3.org/XML/1998/namespace"
         xmlns:dcterms="http://purl.org/dc/terms/"
         xmlns:rdfs="http://www.w3.org/2000/01/rdf-schema#"
         xmlns:xsd="http://www.w3.org/2001/XMLSchema#"
         xmlns:owl="http://www.w3.org/2002/07/owl#"
         xmlns:rdf="http://www.w3.org/1999/02/22-rdf-syntax-ns#"
         xmlns:skos="http://www.w3.org/2004/02/skos/core#"
         xmlns:cc="http://creativecommons.org/ns#">
    <owl:Ontology rdf:about="http://data.europa.eu/dr8">
        <rdfs:label xml:lang="en">Controlled vocabulary for the European Interoperability Reference Architecture (EIRA)</rdfs:label>
        <dcterms:modified rdf:datatype="&xsd;date">2021-08-02</dcterms:modified>
        <dcterms:rights xml:lang="en">Copyright (c) 2016 European Union.</dcterms:rights>
        <cc:attributionName xml:lang="en">European Commission</cc:attributionName>
        <rdfs:comment xml:lang="en">This file specifies the controlled vocabulary defined by the EIRA as SKOS concept schemes and SKOS concepts.</rdfs:comment>
        <dcterms:description xml:lang="en">This file specifies the controlled vocabulary defined by the EIRA as SKOS concept schemes and SKOS concepts.</dcterms:description>
        <dcterms:abstract xml:lang="en">This file specifies the controlled vocabulary defined by the EIRA as SKOS concept schemes and SKOS concepts.</dcterms:abstract>
        <owl:versionInfo xml:lang="en">EIRA v4.1.0</owl:versionInfo>
        <vann:preferredNamespacePrefix xml:lang="en">eira</vann:preferredNamespacePrefix>
        <vann:preferredNamespaceUri xml:lang="en">http://data.europa.eu/dr8/</vann:preferredNamespaceUri>
        <foaf:maker rdf:resource="https://joinup.ec.europa.eu/asset/eia"/>
        <dcterms:creator rdf:resource="https://joinup.ec.europa.eu/asset/eia"/>
        <cc:attributionURL rdf:resource="https://joinup.ec.europa.eu/asset/eia"/>
        <dcterms:license rdf:resource="https://joinup.ec.europa.eu/category/licence/isa-open-metadata-licence-v11"/>
        <dcterms:conformsTo rdf:resource="https://joinup.ec.europa.eu/elibrary/document/isa-deliverable-process-and-methodology-developing-core-vocabularies"/>
    </owl:Ontology>

    <skos:ConceptScheme rdf:about="http://data.europa.eu/dr8">
        <skos:notation>EIRA</skos:notation>
        <skos:prefLabel xml:lang="en">EIRA taxonomy</skos:prefLabel>
        <skos:hasTopConcept rdf:resource="http://data.europa.eu/dr8/PublicPolicy"/>
        <skos:hasTopConcept rdf:resource="http://data.europa.eu/dr8/InteroperableDigitalPublicServicesImplementationOrientation"/>
        <skos:hasTopConcept rdf:resource="http://data.europa.eu/dr8/PublicPolicyCycle"/>
        <skos:hasTopConcept rdf:resource="http://data.europa.eu/dr8/LegalAct"/>
        <skos:hasTopConcept rdf:resource="http://data.europa.eu/dr8/LegislationCatalogue"/>
        <skos:hasTopConcept rdf:resource="http://data.europa.eu/dr8/LegalInteroperabilityAgreement"/>
        <skos:hasTopConcept rdf:resource="http://data.europa.eu/dr8/LegalAuthority"/>
        <skos:hasTopConcept rdf:resource="http://data.europa.eu/dr8/SharedLegalFramework"/>
        <skos:hasTopConcept rdf:resource="http://data.europa.eu/dr8/LegalAgreements/InternationalTreaties"/>
        <skos:hasTopConcept rdf:resource="http://data.europa.eu/dr8/PublicService"/>
        <skos:hasTopConcept rdf:resource="http://data.europa.eu/dr8/InteroperabilityStrategy"/>
        <skos:hasTopConcept rdf:resource="http://data.europa.eu/dr8/InteroperabilityFramework"/>
        <skos:hasTopConcept rdf:resource="http://data.europa.eu/dr8/InteroperabilityGovernance"/>
        <skos:hasTopConcept rdf:resource="http://data.europa.eu/dr8/InteroperabilityOrganisationalAuthority"/>
        <skos:hasTopConcept rdf:resource="http://data.europa.eu/dr8/SecurityFramework"/>
        <skos:hasTopConcept rdf:resource="http://data.europa.eu/dr8/PrivacyFramework"/>
        <skos:hasTopConcept rdf:resource="http://data.europa.eu/dr8/InteroperabilitySkill"/>
        <skos:hasTopConcept rdf:resource="http://data.europa.eu/dr8/PublicServiceAgent"/>
        <skos:hasTopConcept rdf:resource="http://data.europa.eu/dr8/PublicServiceConsumerAgent"/>
        <skos:hasTopConcept rdf:resource="http://data.europa.eu/dr8/PublicServiceConsumer"/>
        <skos:hasTopConcept rdf:resource="http://data.europa.eu/dr8/OrganisationalInteroperabilityAgreement"/>
        <skos:hasTopConcept rdf:resource="http://data.europa.eu/dr8/PublicServiceProvider"/>
        <skos:hasTopConcept rdf:resource="http://data.europa.eu/dr8/PublicServiceDeliveryAgent"/>
        <skos:hasTopConcept rdf:resource="http://data.europa.eu/dr8/ServiceDeliveryModel"/>
        <skos:hasTopConcept rdf:resource="http://data.europa.eu/dr8/BusinessCapability"/>
        <skos:hasTopConcept rdf:resource="http://data.europa.eu/dr8/ExchangeOfBusinessInformation"/>
        <skos:hasTopConcept rdf:resource="http://data.europa.eu/dr8/BusinessInformation"/>
        <skos:hasTopConcept rdf:resource="http://data.europa.eu/dr8/PublicServiceCatalogue"/>
        <skos:hasTopConcept rdf:resource="http://data.europa.eu/dr8/SharedGovernanceFramework"/>
        <skos:hasTopConcept rdf:resource="http://data.europa.eu/dr8/DataPolicy"/>
        <skos:hasTopConcept rdf:resource="http://data.europa.eu/dr8/Representation"/>
        <skos:hasTopConcept rdf:resource="http://data.europa.eu/dr8/DataSetCatalogue"/>
        <skos:hasTopConcept rdf:resource="http://data.europa.eu/dr8/DataSet"/>
        <skos:hasTopConcept rdf:resource="http://data.europa.eu/dr8/Data"/>
        <skos:hasTopConcept rdf:resource="http://data.europa.eu/dr8/SharedKnowledgeBase"/>
        <skos:hasTopConcept rdf:resource="http://data.europa.eu/dr8/DataMapping"/>
        <skos:hasTopConcept rdf:resource="http://data.europa.eu/dr8/OntologiesCatalogue"/>
        <skos:hasTopConcept rdf:resource="http://data.europa.eu/dr8/Ontology"/>
        <skos:hasTopConcept rdf:resource="http://data.europa.eu/dr8/DataOwner"/>
        <skos:hasTopConcept rdf:resource="http://data.europa.eu/dr8/SemanticInteroperabilityAgreement"/>
        <skos:hasTopConcept rdf:resource="http://data.europa.eu/dr8/DataMappingCatalogue"/>
        <skos:hasTopConcept rdf:resource="http://data.europa.eu/dr8/SemanticAgreement"/>
        <skos:hasTopConcept rdf:resource="http://data.europa.eu/dr8/SecurityPolicy"/>
        <skos:hasTopConcept rdf:resource="http://data.europa.eu/dr8/PrivacyPolicy"/>
        <skos:hasTopConcept rdf:resource="http://data.europa.eu/dr8/MachineToMachineInterface"/>
        <skos:hasTopConcept rdf:resource="http://data.europa.eu/dr8/HumanInterface"/>
        <skos:hasTopConcept rdf:resource="http://data.europa.eu/dr8/InteroperableEuropeanSolutionService"/>
        <skos:hasTopConcept rdf:resource="http://data.europa.eu/dr8/InteroperableEuropeanSolutionComponent"/>
        <skos:hasTopConcept rdf:resource="http://data.europa.eu/dr8/AccessManagementService"/>
        <skos:hasTopConcept rdf:resource="http://data.europa.eu/dr8/AccessManagementComponent"/>
        <skos:hasTopConcept rdf:resource="http://data.europa.eu/dr8/AuditService"/>
        <skos:hasTopConcept rdf:resource="http://data.europa.eu/dr8/AuditComponent"/>
        <skos:hasTopConcept rdf:resource="http://data.europa.eu/dr8/InteroperableEuropeanSolution"/>
        <skos:hasTopConcept rdf:resource="http://data.europa.eu/dr8/DataTransformationService"/>
        <skos:hasTopConcept rdf:resource="http://data.europa.eu/dr8/DataTransformationComponent"/>
        <skos:hasTopConcept rdf:resource="http://data.europa.eu/dr8/DataValidationService"/>
        <skos:hasTopConcept rdf:resource="http://data.europa.eu/dr8/DataValidationComponent"/>
        <skos:hasTopConcept rdf:resource="http://data.europa.eu/dr8/ServiceDiscoveryService"/>
        <skos:hasTopConcept rdf:resource="http://data.europa.eu/dr8/ServiceDiscoveryComponent"/>
        <skos:hasTopConcept rdf:resource="http://data.europa.eu/dr8/OrchestrationService"/>
        <skos:hasTopConcept rdf:resource="http://data.europa.eu/dr8/OrchestrationComponent"/>
        <skos:hasTopConcept rdf:resource="http://data.europa.eu/dr8/TechnicalSpecification"/>
        <skos:hasTopConcept rdf:resource="http://data.europa.eu/dr8/TechnicalInteroperabilityAgreement"/>
        <skos:hasTopConcept rdf:resource="http://data.europa.eu/dr8/SharedPlatform"/>
        <skos:hasTopConcept rdf:resource="http://data.europa.eu/dr8/ConformanceTestingService"/>
        <skos:hasTopConcept rdf:resource="http://data.europa.eu/dr8/ConformanceTestingComponent"/>
        <skos:hasTopConcept rdf:resource="http://data.europa.eu/dr8/ConformanceTestReport"/>
        <skos:hasTopConcept rdf:resource="http://data.europa.eu/dr8/ConformanceTestScenario"/>
        <skos:hasTopConcept rdf:resource="http://data.europa.eu/dr8/TechnicalAgreement"/>
        <skos:hasTopConcept rdf:resource="http://data.europa.eu/dr8/DigitalServiceInfrastructure"/>
        <skos:hasTopConcept rdf:resource="http://data.europa.eu/dr8/MetadataManagementComponent"/>
        <skos:hasTopConcept rdf:resource="http://data.europa.eu/dr8/E-archivingComponent"/>
        <skos:hasTopConcept rdf:resource="http://data.europa.eu/dr8/FormsManagementComponent"/>
        <skos:hasTopConcept rdf:resource="http://data.europa.eu/dr8/DataPublicationComponent"/>
        <skos:hasTopConcept rdf:resource="http://data.europa.eu/dr8/PrivacyComponent"/>
        <skos:hasTopConcept rdf:resource="http://data.europa.eu/dr8/ConfigurationAndSolutionCartographyServiceComponent"/>
        <skos:hasTopConcept rdf:resource="http://data.europa.eu/dr8/E-paymentComponent"/>
        <skos:hasTopConcept rdf:resource="http://data.europa.eu/dr8/ServiceRegistryComponent"/>
        <skos:hasTopConcept rdf:resource="http://data.europa.eu/dr8/MachineTranslationComponent"/>
        <skos:hasTopConcept rdf:resource="http://data.europa.eu/dr8/TrustServiceProvisioningComponent"/>
        <skos:hasTopConcept rdf:resource="http://data.europa.eu/dr8/IdentityManagementComponent"/>
        <skos:hasTopConcept rdf:resource="http://data.europa.eu/dr8/TrustRegistryComponent"/>
        <skos:hasTopConcept rdf:resource="http://data.europa.eu/dr8/DataExchangeComponent"/>
        <skos:hasTopConcept rdf:resource="http://data.europa.eu/dr8/HostingAndNetworkingInfrastructure"/>
        <skos:hasTopConcept rdf:resource="http://data.europa.eu/dr8/Network"/>
        <skos:hasTopConcept rdf:resource="http://data.europa.eu/dr8/NetworkingService"/>
        <skos:hasTopConcept rdf:resource="http://data.europa.eu/dr8/HostingService"/>
        <skos:hasTopConcept rdf:resource="http://data.europa.eu/dr8/HostingFacility"/>
        <skos:hasTopConcept rdf:resource="http://data.europa.eu/dr8/ContentManagementService"/>
        <skos:hasTopConcept rdf:resource="http://data.europa.eu/dr8/DataWarehouseService"/>
        <skos:hasTopConcept rdf:resource="http://data.europa.eu/dr8/DataWarehouseComponent"/>
        <skos:hasTopConcept rdf:resource="http://data.europa.eu/dr8/DataRepository"/>
        <skos:hasTopConcept rdf:resource="http://data.europa.eu/dr8/DataAnalyticsService"/>
        <skos:hasTopConcept rdf:resource="http://data.europa.eu/dr8/DataAnalyticsComponent"/>
        <skos:hasTopConcept rdf:resource="http://data.europa.eu/dr8/ArtificialIntelligenceService"/>
        <skos:hasTopConcept rdf:resource="http://data.europa.eu/dr8/ArtificialIntelligenceComponent"/>
        <skos:hasTopConcept rdf:resource="http://data.europa.eu/dr8/SmartDevices"/>
        <skos:hasTopConcept rdf:resource="http://data.europa.eu/dr8/HighPerformanceInfrastructure"/>
        <skos:hasTopConcept rdf:resource="http://data.europa.eu/dr8/DataInfrastructure"/>
        <skos:hasTopConcept rdf:resource="http://data.europa.eu/dr8/DataHub"/>
        <skos:hasTopConcept rdf:resource="http://data.europa.eu/dr8/DataLake"/>
        <skos:hasTopConcept rdf:resource="http://data.europa.eu/dr8/DataRepositoryExchangeService"/>
        <skos:hasTopConcept rdf:resource="http://data.europa.eu/dr8/DataRepositoryExchangeComponent"/>
        <skos:hasTopConcept rdf:resource="http://data.europa.eu/dr8/EiraViewpoint"/>
        <skos:hasTopConcept rdf:resource="http://data.europa.eu/dr8/ArchitectureBuildingBlock"/>
        <skos:hasTopConcept rdf:resource="http://data.europa.eu/dr8/SolutionBuildingBlock"/>
        <skos:hasTopConcept rdf:resource="http://data.europa.eu/dr8/EiraView"/>
        <skos:hasTopConcept rdf:resource="http://data.europa.eu/dr8/Solution"/>
        <skos:hasTopConcept rdf:resource="http://data.europa.eu/dr8/EifInteroperabilityLevel"/>
        <skos:hasTopConcept rdf:resource="http://data.europa.eu/dr8/InteroperabilityAspect"/>
        <skos:hasTopConcept rdf:resource="http://data.europa.eu/dr8/InteroperabilityRequirement"/>
        <skos:hasTopConcept rdf:resource="http://data.europa.eu/dr8/EifPrinciple"/>
        <skos:hasTopConcept rdf:resource="http://data.europa.eu/dr8/ArchitecturePrinciple"/>
        <skos:hasTopConcept rdf:resource="http://data.europa.eu/dr8/ArchitectureRequirement"/>
        <skos:hasTopConcept rdf:resource="http://data.europa.eu/dr8/SolutionSpecification"/>
        <skos:hasTopConcept rdf:resource="http://data.europa.eu/dr8/EvidenceBasedPublicPolicy"/>
        <skos:hasTopConcept rdf:resource="http://data.europa.eu/dr8/Transparency"/>
        <skos:hasTopConcept rdf:resource="http://data.europa.eu/dr8/PublicValue"/>
        <skos:hasTopConcept rdf:resource="http://data.europa.eu/dr8/SuccessfulPublicServiceImplementationOrientation"/>
        <skos:hasTopConcept rdf:resource="http://data.europa.eu/dr8/SocialParticipation"/>
        <skos:hasTopConcept rdf:resource="http://data.europa.eu/dr8/Accountability"/>
        <skos:hasTopConcept rdf:resource="http://data.europa.eu/dr8/MarketCollaboration"/>
        <skos:hasTopConcept rdf:resource="http://data.europa.eu/dr8/DigitalInclusion"/>
        <skos:hasTopConcept rdf:resource="http://data.europa.eu/dr8/Accessibility"/>
        <skos:hasTopConcept rdf:resource="http://data.europa.eu/dr8/EuropeanDigitalSovereignty"/>
        <skos:hasTopConcept rdf:resource="http://data.europa.eu/dr8/EuLegislationCompliance"/>
        <skos:hasTopConcept rdf:resource="http://data.europa.eu/dr8/IntegratedHorizontalUserExperience"/>
        <skos:hasTopConcept rdf:resource="http://data.europa.eu/dr8/OnceOnly"/>
        <skos:hasTopConcept rdf:resource="http://data.europa.eu/dr8/CodeOfEthicsCompliance"/>
        <skos:hasTopConcept rdf:resource="http://data.europa.eu/dr8/Privacy"/>
        <skos:hasTopConcept rdf:resource="http://data.europa.eu/dr8/EulfCompliance"/>
        <skos:hasTopConcept rdf:resource="http://data.europa.eu/dr8/TechnologyNeutrality"/>
        <skos:hasTopConcept rdf:resource="http://data.europa.eu/dr8/ServiceOrientation"/>
        <skos:hasTopConcept rdf:resource="http://data.europa.eu/dr8/Proactiveness"/>
        <skos:hasTopConcept rdf:resource="http://data.europa.eu/dr8/AdministrativeSimplification"/>
        <skos:hasTopConcept rdf:resource="http://data.europa.eu/dr8/NewPublicManagementApproach"/>
        <skos:hasTopConcept rdf:resource="http://data.europa.eu/dr8/ConvergenceAssuranceOnPublicPolicyGoalsAttainment"/>
        <skos:hasTopConcept rdf:resource="http://data.europa.eu/dr8/Multilingulism"/>
        <skos:hasTopConcept rdf:resource="http://data.europa.eu/dr8/Openness"/>
        <skos:hasTopConcept rdf:resource="http://data.europa.eu/dr8/User-centricity"/>
        <skos:hasTopConcept rdf:resource="http://data.europa.eu/dr8/Reusability"/>
        <skos:hasTopConcept rdf:resource="http://data.europa.eu/dr8/SubsidiarityAndProportionality"/>
        <skos:hasTopConcept rdf:resource="http://data.europa.eu/dr8/DataPortability"/>
        <skos:hasTopConcept rdf:resource="http://data.europa.eu/dr8/Security"/>
        <skos:hasTopConcept rdf:resource="http://data.europa.eu/dr8/ConvergenceControlOnPublicPolicyGoalsAttainment"/>
        <skos:hasTopConcept rdf:resource="http://data.europa.eu/dr8/PreservationOfInformation"/>
        <skos:hasTopConcept rdf:resource="http://data.europa.eu/dr8/Trust"/>
        <skos:hasTopConcept rdf:resource="http://data.europa.eu/dr8/Innovation"/>
    </skos:ConceptScheme>

    <skos:Collection rdf:about="http://data.europa.eu/dr8/view/LegalView">
        <skos:notation>LegalView</skos:notation>
        <skos:prefLabel xml:lang="en">Legal View</skos:prefLabel>
        <skos:member rdf:resource="http://data.europa.eu/dr8/PublicPolicy"/>
        <skos:member rdf:resource="http://data.europa.eu/dr8/InteroperableDigitalPublicServicesImplementationOrientation"/>
        <skos:member rdf:resource="http://data.europa.eu/dr8/PublicPolicyCycle"/>
        <skos:member rdf:resource="http://data.europa.eu/dr8/BindingInstrument"/>
        <skos:member rdf:resource="http://data.europa.eu/dr8/Non-bindingInstrument"/>
        <skos:member rdf:resource="http://data.europa.eu/dr8/LegalAct"/>
        <skos:member rdf:resource="http://data.europa.eu/dr8/LegislationCatalogue"/>
        <skos:member rdf:resource="http://data.europa.eu/dr8/LegalInteroperabilityAgreement"/>
        <skos:member rdf:resource="http://data.europa.eu/dr8/LegislationOnDataInformationAndKnowledgeExchange"/>
        <skos:member rdf:resource="http://data.europa.eu/dr8/LegalAuthority"/>
        <skos:member rdf:resource="http://data.europa.eu/dr8/SharedLegalFramework"/>
        <skos:member rdf:resource="http://data.europa.eu/dr8/LegalAgreements/InternationalTreaties"/>
    </skos:Collection>

    <skos:Concept rdf:about="http://data.europa.eu/dr8/PublicPolicy">
        <skos:notation>PublicPolicy</skos:notation>
        <skos:prefLabel xml:lang="en">[ABB9] Public Policy</skos:prefLabel>
        <skos:definition xml:lang="en">DESCRIPTION:
Set of principles followed by a public authority to bring about social change in the medium and long term in a given area. It is based on certain values and objectives and is implemented using a variety of methods. It applies on the territory within which the authority is authorised to act.

Based on EuroVoc
http://eurovoc.europa.eu/drupal/?q=request&amp;concepturi=http%3A%2F%2Feurovoc.europa.eu%2F8466&amp;termuri=http%3A%2F%2Feurovoc.europa.eu%2F209598&amp;language=en&amp;view=pt&amp;ifacelang=en

The policies; overview of EU activities in all areas, from agriculture to transport: http://ec.europa.eu/policies/index_en.htm

Syn. Policy Action

INTEROPERABILITY SALIENCY:
IoP Dimension: Governance IoP
The Public Policy ABB is salient for legal interoperability because it drives the production and formulation of legislation, and it is one of the main context elements to be taken into account when organisation need to work together, as stated in the EIF: &quot;Legal interoperability is about ensuring that organisations operating under different legal frameworks, policies and strategies are able to work together&quot;.

EXAMPLES:
The following implementation is an example on how this specific Architecture Building Block (ABB) can be instantiated as a Solution Building Block (SBB):

Common Agricultural Policy (CAP)
The common agricultural policy (CAP)  one of Europes oldest policies  has evolved along with the EU. Today&apos;s CAP supports a modern, market-oriented farming sector ensuring the provision of safe, affordable, high quality food, produced sustainably and respecting strict standards (environmental, animal welfare, food safety, etc.), as well as supporting investment in the broader rural economy.
https://ec.europa.eu/info/strategy/agriculture_en</skos:definition>
        <skos:topConceptOf rdf:resource="http://data.europa.eu/dr8"/>
    </skos:Concept>

    <skos:Concept rdf:about="http://data.europa.eu/dr8/InteroperableDigitalPublicServicesImplementationOrientation">
        <skos:notation>InteroperableDigitalPublicServicesImplementationOrientation</skos:notation>
        <skos:prefLabel xml:lang="en">[ABB111] Interoperable Digital Public Services Implementation Orientation</skos:prefLabel>
        <skos:definition xml:lang="en">DESCRIPTION:
It is the specific set of decision making rules/criteria/principles followed at implementing a digital public services through organisations, persons, objects or events (Hill &amp; Hupe, 2002). In the MIS literature it is considered as the focus selected for the implementation (Hill &amp; Hupe, 2002; Marchand et al., 2000; Santosuosso &amp; Malerba, 2014).  The following implementation orientations are identified in the literature: integration, technology, governance and legal.

	The INTEGRATION ORIENTATION (Marchand et al., 2000) is characterized by a focus on data resources and on information management capabilities to manage information resources over their life cycle (i.e. scanning, collecting, organising, processing, maintaining, etc.) to understand societal needs, to embed data throughout the policy cycle, and to develop a culture of data analytics (OECD, 2018). The integration orientation will be based on semantic interoperability aiming for the design of a shared knowledge base of usable data, information and knowledge resources that enables:
i)	structural interoperability by using and/or sharing of data, organisational information and organisational knowledge (i.e. data set catalogue, base registries, catalogue of ontologies);
ii)	behavioural interoperability by exchanging capabilities of data, organisational information and organisational knowledge with the environment (i.e. representation, data mappings); and
iii)	governance interoperability by semantic interoperability agreements (i.e. ontologies).

	The TECHNOLOGY ORIENTATION (Marchand et al., 2000) is characterized by a focus on ICT resources like solutions and infrastructure and on ICT management capabilities to manage the provision of services (i.e. business operations, decision making, internal support, etc.) to users and the consumption of services by ministries and agencies (OECD, 2018). The technology orientation will be based on technical interoperability aiming for the design of a shared platform of ICT resources (i.e. the platform) that enables:
i) structural interoperability by reusing and/or sharing of software components (i.e. service registry service, networks, reusable building blocks, common [back office] services);
ii) behavioural interoperability with ICT exchanging capabilities of data, information or knowledge with internal/external peers (i.e. intermediation services, interfaces); an
iii) governance interoperability with technical interoperability agreements (i.e. protocols, choreography rules).

	The GOVERNANCE ORIENTATION (Marchand et al., 2000) is characterized by a focus on the governance resources (Grant et al., 2007) and on governance management capabilities/archetypes to manage the effective use of information (i.e. sharing, security, privacy, etc.) for the effective use of information (i.e. sharing, security, privacy, etc.) to achieve a more agile, effective, and digitally inclusive public engagement, to increase trust in government, and to enhance government transparency (OECD, 2018; Weill &amp; Woodham, 2002). The governance orientation will be based on organisational interoperability aiming for the design of a shared governance framework of [re]usable organisational resources that enables:
i)	structural interoperability by reusing and/or sharing of digital public services (i.e. public services catalogue);
ii)	behavioural interoperability with organisational exchanging capabilities of data, information or knowledge with internal/external peers (i.e. service delivery model); and
iii)	governance interoperability with organisational interoperability agreements (i.e. service level agreements, governance structures).

	The LEGAL ORIENTATION (Santosuossa and Malerba, 2014) is characterized by a focus on legal and regulatory frameworks based in displayed leadership and political commitment to ensure adaptation to rapidly changing technological and diverse social environments with high-level requirements to achieve coherence and effective support to digital public services implementation (OECD, 2018). The legal orientation will be based in legal interoperability aiming for the design of a shared legal framework of [re]usable legal resources that enables:
i)	structural interoperability by legislation on reusing and/or sharing orientation and guidelines (i.e. legislation catalogue, interoperability reference architectures);
ii)	behavioural interoperability by legislation on exchanging capabilities of data, information or knowledge with internal/external peers (i.e. interoperability frameworks); and
iii)	governance interoperability by legislation on governance agreements (i.e. GDPR).

INTEROPERABILITY SALIENCY:
IoP Dimension: Behavioural IoP
The Interoperable Digital Public Service Implementation Orientation ABB is salient for organizational interoperability because the extent of support to the public policy goals by a digital interoperable public service might be influenced by the selected implementation orientation.

The following implementation is an example on how this specific Architecture Building Block (ABB) can be instantiated as a Solution Building Block (SBB):

Next Generation Digital Government Architecture v1.0 by Republic of Estonia (2020)
https://docs.google.com/document/d/1UJ-5wi9wavWzA2n4LhsbONJqdxjUSIgMxKJNaZZslas/edit?fbclid=IwAR2rrBNjwHFagHIvi-9Pv6uvKI0IZH_m4IdAfaq7hbjALlIjRH8nEuUVuic
Customs 2020 is an EU cooperation programme providing national customs administrations with the possibility to create and exchange information and expertise. It allows developing and operating major trans-European IT systems in partnership and establishing various human networks by bringing together national officials from across Europe. The programme has a budget of  547.3 million and will run for 7 years from January 1 2014.
https://ec.europa.eu/taxation_customs/business/customs-cooperation-programmes/customs-2020-programme_en</skos:definition>
        <skos:topConceptOf rdf:resource="http://data.europa.eu/dr8"/>
    </skos:Concept>

    <skos:Concept rdf:about="http://data.europa.eu/dr8/PublicPolicyCycle">
        <skos:notation>PublicPolicyCycle</skos:notation>
        <skos:prefLabel xml:lang="en">[ABB102] Public Policy Cycle</skos:prefLabel>
        <skos:definition xml:lang="en">DESCRIPTION:
The series of public policy phases that are regularly repeated in order to manage all aspects of a public policy.

Based on EU Better Regulation (list of phases) and Oxford dictionary (cycle definition)
http://ec.europa.eu/smart-regulation/guidelines/ug_chap1_en.htm (chapter 2 &quot;What is Better Regulation?&quot;)
http://publicadministrationtheone.blogspot.be/2012/08/public-policy-models-of-policy-making_27.html

Syn. Policy Cycle

INTEROPERABILITY SALIENCY:
IoP Dimension: Governance IoP
The Public Policy Cycle ABB is salient for legal interoperability because it impacts the design and formulation of public policies, which are implemented through legal acts. Interoperability principles need to be taken into account during the whole public policy cycle.

EXAMPLES:
The following implementation is an example on how this specific Architecture Building Block (ABB) can be instantiated as a Solution Building Block (SBB):

Performance-based Full Policy Cycle for the Digital Single Market
The key features of a performance-based full policy cycle are a clear articulation of policy objectives, the identification and use of quantitative indicators of expected short-term and longer-term policy impacts, the identification of synergies between policies, a much greater use of quantitative data in ex-ante impact assessments, the implementation of robust, data-based, independent ex post assessments of the performance of policies relative to their expected impacts and a wide dissemination of lessons learned in such ex-post performance assessments.
http://www.europarl.europa.eu/RegData/etudes/etudes/join/2013/507457/IPOL-IMCO_ET(2013)507457_EN.pdf</skos:definition>
        <skos:topConceptOf rdf:resource="http://data.europa.eu/dr8"/>
    </skos:Concept>

    <skos:Concept rdf:about="http://data.europa.eu/dr8/BindingInstrument">
        <skos:notation>BindingInstrument</skos:notation>
        <skos:prefLabel xml:lang="en">[ABB17] Binding Instrument</skos:prefLabel>
        <skos:definition xml:lang="en">DESCRIPTION:
Legal means, involving an obligation, which are available to the European institutions to carry out their tasks. The European binding instruments listed in Article 288 of the Treaty on the Functioning of the European Union are:
	regulations: these are binding in their entirety and directly applicable in all EU countries;
	directives: these bind the EU countries as to the results to be achieved; they have to be transposed into the national legal framework and thus leave margin for manoeuvre as to the form and means of implementation;
	decisions: these are fully binding on those to whom they are addressed.

Based on EUR-Lex
http://eur-lex.europa.eu/summary/glossary/community_legal_instruments.html

The binding legal instruments that make up the secondary legislation of the EU are Regulations, Directives and Decisions.  As set out in Article 288 of the Treaty on the Functioning of the European Union:
- A Regulation shall have general application. It shall be binding in its entirety and directly applicable in
all Member States.
- A Directive shall be binding, as to the result to be achieved, upon each Member State to which it is
addressed, but shall leave to the national authorities the choice of form and methods.
- A Decision shall be binding in its entirety. A Decision which specifies those to whom it is addressed
shall be binding only on them.

Source:
https://ox.libguides.com/c.php?g=422926&amp;p=2888217

INTEROPERABILITY SALIENCY:
IoP Dimension: Governance IoP
The Binding Instrument ABB is relevant for interoperability as, by being a specialisation of Legal Act, it makes mandatory the implementation of the policy (and therefore the underlying interoperability implications).

EXAMPLES:
The following implementation is an example on how this specific Architecture Building Block (ABB) can be instantiated as a Solution Building Block (SBB):

Decision No 922/2009/EC of the European Parliament and of the Council of 16 September 2009 on interoperability solutions for European public administrations (ISA)
	1.	This Decision establishes, for the period 2010-2015, a programme on interoperability solutions for European public administrations, including local and regional administrations and Community institutions and bodies, providing common and 		shared solutions facilitating interoperability (the ISA programme).
	2.	The objective of the ISA programme is to support cooperation between European public administrations by facilitating the efficient and effective electronic cross-border and cross-sectoral interaction between such administrations, including 		bodies performing public functions on their behalf, enabling the delivery of electronic public services supporting the implementation of Community policies and activities.
http://eur-lex.europa.eu/legal-content/EN/TXT/?uri=CELEX%3A32009D0922</skos:definition>
        <skos:narrower rdf:resource="http://data.europa.eu/dr8/LegalAct"/>
    </skos:Concept>

    <skos:Concept rdf:about="http://data.europa.eu/dr8/Non-bindingInstrument">
        <skos:notation>Non-bindingInstrument</skos:notation>
        <skos:prefLabel xml:lang="en">[ABB113] Non-binding Instrument</skos:prefLabel>
        <skos:definition xml:lang="en">DESCRIPTION:
Legal means, involving no obligation, which are available to the European institutions to carry out their tasks. The European non-binding, declaratory instruments listed in Article 288 of the Treaty on the Functioning of the European Union are recommendations and opinions:
	Recommendations are non-mandatory acts issued by the European Commission, the Council of the European Union, or the European Central Bank which suggest a certain form of conduct to those to whom they are addressed without imposing any legal obligations.
	Opinions are non-binding legal acts adopted by the European institutions which do not bind those to whom they are addressed.

Based on EUR-Lex and EuroVoc
http://eur-lex.europa.eu/summary/glossary/community_legal_instruments.html?locale=en
http://eurovoc.europa.eu/drupal/?q=request&amp;concepturi=http%3A%2F%2Feurovoc.europa.eu%2F2927&amp;termuri=http%3A%2F%2Feurovoc.europa.eu%2F439743&amp;language=en&amp;view=pt&amp;ifacelang=en
http://eurovoc.europa.eu/drupal/?q=request&amp;concepturi=http%3A%2F%2Feurovoc.europa.eu%2F6284&amp;termuri=http%3A%2F%2Feurovoc.europa.eu%2F438412&amp;language=en&amp;view=pt&amp;ifacelang=en

Article 288 of the Treaty on the Functioning of the European Union also provides for non binding legal instruments.
- Recommendations call upon the party to whom they are addressed to behave in a particular way without placing them under any legal obligation
- Opinions issued by the EU institutions give assessments of situations or developments in the Union or in the individual Member States. They may also also prepare the way for subsequent, legally binding acts, or be a prerequisite for the institution of proceedings before the Court of Justice
Recommendations and Opinions have moral and political significance, without being legally binding
The three other main forms of actions that shape the EU legal order without having legally binding effect are Resolutions, Declarations and Action programmes.

INTEROPERABILITY SALIENCY:
IoP Dimension: Governance IoP
The Non-binding Instrument ABB is a key interoperability enabler as a specialisation of the Legal Act.

EXAMPLES:
The following implementation is an example on how this specific Architecture Building Block (ABB) can be instantiated as a Solution Building Block (SBB):

Action Plan for the future of Organic Production in the European Union
The Commission launched a consultation for the review of the European policy on organic agriculture in 2012-2013. This consultation has also been an opportunity to consult experts, stakeholders and the public on areas where a new action plan might be needed. To help organic farmers, producers and retailers adjust to the proposed policy changes and meet future challenges, the Commission has also approved an Action Plan on the future of Organic Production in Europe. The Plan foresees to better inform farmers on rural development and EU farm policy initiatives encouraging organic farming, to strengthen links between EU research and innovation projects and organic production and to encourage the use of organic food, e.g. in schools.
https://ec.europa.eu/agriculture/organic/eu-policy/european-action-plan_en</skos:definition>
        <skos:narrower rdf:resource="http://data.europa.eu/dr8/LegalAct"/>
    </skos:Concept>

    <skos:Concept rdf:about="http://data.europa.eu/dr8/LegalAct">
        <skos:notation>LegalAct</skos:notation>
        <skos:prefLabel xml:lang="en">[ABB164] Legal Act</skos:prefLabel>
        <skos:definition xml:lang="en">DESCRIPTION:
Formalised set of rules on a subject potentially including requirements concerning digital public services. The granularity of the  requirements might be of high level or detail level. Requirements of high-level granularity contain generic/abstract functional requirements like principles and/or recommendations with considerable degrees for transposition/execution and of not binding nature. On the other side, requirements of detail-level granularity imply a limited degree for transposition/execution and they contain specific/concrete functionalities, solution components, data, procedures, and/or technical specifications or standards to be used. EU legal acts are legislative or non-legislative acts adopted by the European institutions (Article 288 TFEU). With the entry into force of the Treaty of Lisbon on 1 December 2009. The names &quot;European Union&quot; or &quot;EU&quot; have replaced &quot;European Community&quot;, &quot;Community&quot; or &quot;EC&quot;.

Source: https://eur-lex.europa.eu/summary/glossary/legislative_acts.html

INTEROPERABILITY SALIENCY:
IoP Dimension: Governance IoP
The Legal Act ABB is salient for interoperability because it helps achieve legal interoperability by ensuring compatible legal/juridical certainty in the exchange of information.

EXAMPLES:
The following implementation is an example on how this specific Architecture Building Block (ABB) can be instantiated as a Solution Building Block (SBB):

COMMISSION REGULATION (EU) 2018/1881
 of 3 December 2018
amending Regulation (EC) No 1907/2006 of the European Parliament and of the Council on the Registration, Evaluation, Authorisation and Restriction of Chemicals (REACH) as regards Annexes I, III,VI, VII, VIII, IX, X, XI, and XII to address nanoforms of substances.
https://eur-lex.europa.eu/legal-content/EN/TXT/?qid=1544102387245&amp;uri=CELEX:32018R1881</skos:definition>
        <skos:topConceptOf rdf:resource="http://data.europa.eu/dr8"/>
    </skos:Concept>

    <skos:Concept rdf:about="http://data.europa.eu/dr8/LegislationCatalogue">
        <skos:notation>LegislationCatalogue</skos:notation>
        <skos:prefLabel xml:lang="en">[ABB165] Legislation Catalogue</skos:prefLabel>
        <skos:definition xml:lang="en">DESCRIPTION:
Indexed inventory of legal documents with comprehensiveness and trustiness value

(*)DECISION (EU) 2015/2240 OF THE EUROPEAN PARLIAMENT AND OF THE COUNCIL of 25 November 2015  establishing a programme on interoperability solutions and common frameworks for European public administrations, businesses and citizens (ISA2 programme) as a means for modernising the public sector

Based on IATE (definition of catalogue, entry Documentation [COM])
http://iate.europa.eu/

Syn. Official Journal

INTEROPERABILITY SALIENCY:
IoP Dimension: Structural IoP
This ABB is a key interoperability enabler because it supports to achieve legal structural interoperability by  enabling sharing/provisioning and reusing/consumption of legislation on digital public services

EXAMPLES:
The following implementation is an example on how this specific Architecture Building Block (ABB) can be instantiated as a Solution Building Block (SBB):

EUR-Lex
EUR-Lex provides free access, in the 24 official EU languages, to:

	the authentic Official Journal of the European Union
	EU law (EU treaties, directives, regulations, decisions, consolidated legislation, etc.)
	preparatory acts (legislative proposals, reports, green and white papers, etc.)
	EU case-law (judgments, orders, etc.)
	international agreements
	EFTA documents
	summaries of EU legislation, which put legal acts into a policy context, explained in plain language
	other public documents.

It also allows you to follow the procedures leading to the adoption of legal acts.
http://eur-lex.europa.eu/</skos:definition>
        <skos:topConceptOf rdf:resource="http://data.europa.eu/dr8"/>
    </skos:Concept>

    <skos:Concept rdf:about="http://data.europa.eu/dr8/LegalInteroperabilityAgreement">
        <skos:notation>LegalInteroperabilityAgreement</skos:notation>
        <skos:prefLabel xml:lang="en">[ABB226] Legal Interoperability Agreement</skos:prefLabel>
        <skos:definition xml:lang="en">DESCRIPTION:
A legal interoperability agreement is legal resource formalizing governance rules enabling collaboration between digital public services

Based on EIF:
https://ec.europa.eu/isa2/sites/isa/files/eif_brochure_final.pdf#page=27

INTEROPERABILITY SALIENCY:
IoP Dimension: Governance IoP
The Legal Interoperability Agreement ABB  is a key interoperability enabler because it supports legal interoperability by enabling the seamless exchange of data, information, and knowledge.

EXAMPLES:
The following implementation is an example on how this specific Architecture Building Block (ABB) can be instantiated as a Solution Building Block (SBB):

RDA-CODATA
Agreement that provides the guidelines and principles on the legal interoperability of research data.
http://www.codata.org/uploads/Legal%20Interoperability%20Principles%20and%20Implementation%20Guidelines_Final2.pdf</skos:definition>
        <skos:topConceptOf rdf:resource="http://data.europa.eu/dr8"/>
    </skos:Concept>

    <skos:Concept rdf:about="http://data.europa.eu/dr8/LegislationOnDataInformationAndKnowledgeExchange">
        <skos:notation>LegislationOnDataInformationAndKnowledgeExchange</skos:notation>
        <skos:prefLabel xml:lang="en">[ABB356] Legislation on Data Information and Knowledge Exchange</skos:prefLabel>
        <skos:definition xml:lang="en">DESCRIPTION:
Legal act on the exchange of data, information, and knowledge between different agents (private and public) at national and/or cross-border level.

INTEROPERABILITY SALIENCY
IoP Dimension: Behavioural IoP
The Legislation on Data, information, and Knowledge  Exchange ABB is a key interoperability enabler because it supports to achieve legal interoperability by ensuring  legal/juridical certainty and determinacy in the exchange of data, information, and knowledge.

EXAMPLE:
The following implementation is an example on how this specific Architecture Building Block (ABB) can be instantiated as a Solution Building Block (SBB):

Regulation on the free flow of non-personal data
The Regulation, applicable as of 28 May 2019, aims at removing obstacles to the free movement of non-personal data across Member States and IT systems in Europe.
The Regulation ensures:
- Free movement of non-personal data across borders: every organisation should be able to store and process data anywhere in the European Union,
- The availability of data for regulatory control: public authorities will retain access to data, also when it is located in another Member State or when it is stored or processed in the cloud,
- Easier switching of cloud service providers for professional users. The Commission has started facilitating self-regulation in this area, encouraging providers to develop codes of conduct regarding the conditions under which users can port data between cloud service providers and back into their own IT environments,
- Full consistency and synergies with the cybersecurity package, and clarification that any security requirements that already apply to businesses storing and processing data will continue to do so when they store or process data across borders in the EU or in the cloud.
https://ec.europa.eu/knowledge4policy/publication/regulation-free-flow-non-personal-data_en</skos:definition>
        <skos:narrower rdf:resource="http://data.europa.eu/dr8/LegalAct"/>
    </skos:Concept>

    <skos:Concept rdf:about="http://data.europa.eu/dr8/LegalAuthority">
        <skos:notation>LegalAuthority</skos:notation>
        <skos:prefLabel xml:lang="en">[ABB227] Legal Authority</skos:prefLabel>
        <skos:definition xml:lang="en">DESCRIPTION:
It is an entity with entitled powers.  The powers that a public administration exercises during the above mentioned life cycle are of the following four types: Legislation, control (monitoring, enforcing, sanctioning, etc.), economic (taxes, subsidies, expenditures, funding, etc.) and (public service) provision (Thijs et al., 2017).

Sources:
Thijs, N.; Hammerschmid, G. and Palaric, E. (2017). EUPACK synthesis report. A comparative analysis of Public Administration Characteristics and Performance in the EU28. European Commission.

Based on EIF:
https://ec.europa.eu/isa2/sites/isa/files/eif_brochure_final.pdf

INTEROPERABILITY SALIENCY:
IoP Dimension: Governance IoP
The Legal Authority ABB is salient for interoperability because it supports legal interoperability by providing reliability and trustworthiness of Legal Interoperability Agreement.

EXAMPLES:
The following implementation is an example on how this specific Architecture Building Block (ABB) can be instantiated as a Solution Building Block (SBB):

EU Parliament
European Parliament
The European Parliament (EP) is the directly elected parliamentary institution of the European Union (EU). Together with the Council of the European Union (the Council) and the European Commission, it exercises the legislative function of the EU.
http://www.europarl.europa.eu/plenary/en/home.html</skos:definition>
        <skos:topConceptOf rdf:resource="http://data.europa.eu/dr8"/>
    </skos:Concept>

    <skos:Concept rdf:about="http://data.europa.eu/dr8/SharedLegalFramework">
        <skos:notation>SharedLegalFramework</skos:notation>
        <skos:prefLabel xml:lang="en">[ABB357] Shared Legal Framework</skos:prefLabel>
        <skos:definition xml:lang="en">DESCRIPTION:
A shared legal framework is formed by [re]usable legal resources, with  convergence power, in relation to public policy goals attainment, given by their legally binding nature, across the levels of a public administration (central, regional, local) towards the achievement of the public policy goals, enabling :
i)	structural interoperability by legal resources supporting reusing and/or sharing legislation (i.e. legislation catalogue  enabling provisioning/consuming legal texts cross public administrations and cross borders);
ii)	behavioural interoperability by legal resources supporting exchanging capabilities of data, information or knowledge with internal/external peers (i.e. Legislation on Knowledge, Information and data exchange enabling that data/information/knowledge be provisioned/consumed cross public administrations and cross borders ); and
iii)	governance interoperability by legislation supporting the collaboration with internal/external peers exchanging data, information or knowledge (i.e. Legal Interoperability Agreements on legal terms assuring juridical certainty enabling agreed legal terms/conditions for sharing, reuse and exchange of data/information/knowledge cross public administrations and cross borders).

INTEROPERABILITY SALIENCY:
IoP dimensions: Structural IoP, Behavioral IoP, Governance IoP
This ABB is a key interoperability enabler because it supports to achieve legal interoperability with public policy goals convergence value by  all in all enabling i) sharing/provisioning/reusing/consumption of legislation on digital public services,  ii) the exchange of data, information, and knowledge between digital public services, and iii) collaboration between digital public services</skos:definition>
        <skos:topConceptOf rdf:resource="http://data.europa.eu/dr8"/>
    </skos:Concept>

    <skos:Concept rdf:about="http://data.europa.eu/dr8/LegalAgreements/InternationalTreaties">
        <skos:notation>LegalAgreements/InternationalTreaties</skos:notation>
        <skos:prefLabel xml:lang="en">[ABB368] Legal Agreements / International Treaties</skos:prefLabel>
        <skos:definition xml:lang="en">DESCRIPTION:
Under international law, a treaty is any legally binding agreement between states (countries). A treaty can be called a Convention, a Protocol, a Pact, an Accord, etc.; it is the content of the agreement, not its name, which makes it a treaty.

Based on EIF:
https://eur-lex.europa.eu/legal-content/EN/TXT/?uri=celex%3A12016E207

INTEROPERABILITY SALIENCY:
Not applicable

EXAMPLES:
The following implementation is an example on how this specific Architecture Building Block (ABB) can be instantiated as a Solution Building Block (SBB):

An example of a treaty that does have provisions for further binding agreements is the UN Charter. By signing and ratifying the Charter, countries agreed to be legally bound by resolutions passed by UN bodies such as the General Assembly and the Security Council. Thus, UN resolutions are legally binding on UN Member States, and no signature or ratification is necessary.</skos:definition>
        <skos:topConceptOf rdf:resource="http://data.europa.eu/dr8"/>
    </skos:Concept>

    <skos:Collection rdf:about="http://data.europa.eu/dr8/view/OrganisationalView">
        <skos:notation>OrganisationalView</skos:notation>
        <skos:prefLabel xml:lang="en">Organisational View</skos:prefLabel>
        <skos:member rdf:resource="http://data.europa.eu/dr8/PublicService"/>
        <skos:member rdf:resource="http://data.europa.eu/dr8/InteroperabilityStrategy"/>
        <skos:member rdf:resource="http://data.europa.eu/dr8/InteroperabilityFramework"/>
        <skos:member rdf:resource="http://data.europa.eu/dr8/InteroperabilityGovernance"/>
        <skos:member rdf:resource="http://data.europa.eu/dr8/InteroperabilityOrganisationalAuthority"/>
        <skos:member rdf:resource="http://data.europa.eu/dr8/SecurityFramework"/>
        <skos:member rdf:resource="http://data.europa.eu/dr8/PrivacyFramework"/>
        <skos:member rdf:resource="http://data.europa.eu/dr8/InteroperabilitySkill"/>
        <skos:member rdf:resource="http://data.europa.eu/dr8/Business"/>
        <skos:member rdf:resource="http://data.europa.eu/dr8/PublicAdministration"/>
        <skos:member rdf:resource="http://data.europa.eu/dr8/Organisation"/>
        <skos:member rdf:resource="http://data.europa.eu/dr8/Citizen"/>
        <skos:member rdf:resource="http://data.europa.eu/dr8/PublicServiceAgent"/>
        <skos:member rdf:resource="http://data.europa.eu/dr8/PublicServiceConsumerAgent"/>
        <skos:member rdf:resource="http://data.europa.eu/dr8/PublicServiceConsumer"/>
        <skos:member rdf:resource="http://data.europa.eu/dr8/OrganisationalInteroperabilityAgreement"/>
        <skos:member rdf:resource="http://data.europa.eu/dr8/PublicServiceProvider"/>
        <skos:member rdf:resource="http://data.europa.eu/dr8/PublicServiceDeliveryAgent"/>
        <skos:member rdf:resource="http://data.europa.eu/dr8/ServiceDeliveryModel"/>
        <skos:member rdf:resource="http://data.europa.eu/dr8/BusinessCapability"/>
        <skos:member rdf:resource="http://data.europa.eu/dr8/ExchangeOfBusinessInformation"/>
        <skos:member rdf:resource="http://data.europa.eu/dr8/BusinessInformation"/>
        <skos:member rdf:resource="http://data.europa.eu/dr8/PublicServiceCatalogue"/>
        <skos:member rdf:resource="http://data.europa.eu/dr8/SharedGovernanceFramework"/>
    </skos:Collection>

    <skos:Concept rdf:about="http://data.europa.eu/dr8/PublicService">
        <skos:notation>PublicService</skos:notation>
        <skos:prefLabel xml:lang="en">[ABB1] Public Service</skos:prefLabel>
        <skos:definition xml:lang="en">DESCRIPTION:
It is an interoperable public service provisioned by or on behalf of a public administration in support to the realization of a Public Administration digital business capability. An European digital public service comprises any digital public service exposed to a cross-border dimension in the Union.

Sources: EIF, ISA2 Core Vocabularies, IMM
http://eur-lex.europa.eu/resource.html?uri=cellar:2c2f2554-0faf-11e7-8a35-01aa75ed71a1.0017.02/DOC_3&amp;format=PDF
https://joinup.ec.europa.eu/catalogue/distribution/cpsv-ap-specification-v20-pdf
https://joinup.ec.europa.eu/sites/default/files/imm_guideline_1.pdf
https://ec.europa.eu/isa2/actions/assessing-progress-being-made-towards-interoperability_en

INTEROPERABILITY SALIENCY:
IoP Dimension: Structural IoP, Behavioral IoP, Governance IoP
The Public Service ABB is salient for organisational interoperability because it is the central element around which interoperabilty needs to be ensured, as stated in the EIF: &quot;The European Interoperability Framework is a commonly agreed approach to the delivery of European public services in an interoperable manner&quot;.

EXAMPLES:
The following implementation is an example on how this specific Architecture Building Block (ABB) can be instantiated as a Solution Building Block (SBB):

EUROPASS2 - Make better use of skills and opportunities across Europe
Europass is a service to help individuals to communicate their skills, qualifications and experience through the use of standardised documents templates.
http://ec.europa.eu/social/main.jsp?catId=1266&amp;langId=en</skos:definition>
        <skos:topConceptOf rdf:resource="http://data.europa.eu/dr8"/>
    </skos:Concept>

    <skos:Concept rdf:about="http://data.europa.eu/dr8/InteroperabilityStrategy">
        <skos:notation>InteroperabilityStrategy</skos:notation>
        <skos:prefLabel xml:lang="en">[ABB208] Interoperability Strategy</skos:prefLabel>
        <skos:definition xml:lang="en">DESCRIPTION:
The overarching strategic plan in the area of cross-border interoperability.

Source: ISA2
https://ec.europa.eu/isa2/actions/continuously-updating-european-interoperability-strategy_en

INTEROPERABILITY SALIENCY:
IoP Dimension: Governance IoP
The Interoperability Strategy ABB is an interoperability enabler because it helps achieve organisational interoperability by setting up the vision and principles for the development of the interoperability capabilities. The European Interoperability Framework implements the European Interoperability Strategy.

EXAMPLES:
The following implementation is an example on how this specific Architecture Building Block (ABB) can be instantiated as a Solution Building Block (SBB):

European Interoperability Strategy (EIS)
COMMUNICATION FROM THE COMMISSION TO THE EUROPEAN PARLIAMENT, THE COUNCIL, THE EUROPEAN ECONOMIC AND SOCIAL COMMITTEE AND THE COMMITTEE OF THE REGIONS - Towards interoperability for European public services
This Communication introduces the European Interoperability Strategy (EIS) and the European Interoperability Framework (EIF) for European public services, two key elements in the Digital Agenda. Together, they promote interoperability among public administrations.
The European Interoperability Strategy (EIS) is developed by the European Commissions Directorate-General for Informatics. The EIS aims to provide guidance and to prioritise the actions needed to improve interaction, exchange and cooperation among European public administrations across borders and across sectors for the delivery of European public services.
http://eur-lex.europa.eu/resource.html?uri=cellar:f132547a-7d66-4626-8eb6-9f7428394de7.0017.03/DOC_2&amp;format=PDF</skos:definition>
        <skos:topConceptOf rdf:resource="http://data.europa.eu/dr8"/>
    </skos:Concept>

    <skos:Concept rdf:about="http://data.europa.eu/dr8/InteroperabilityFramework">
        <skos:notation>InteroperabilityFramework</skos:notation>
        <skos:prefLabel xml:lang="en">[ABB206] Interoperability Framework</skos:prefLabel>
        <skos:definition xml:lang="en">DESCRIPTION:
An agreed governance approach to interoperability for organisations that wish to collaborate towards the joint delivery of public services. Within its scope of applicability, it specifies a set of common elements such as vocabulary, concepts, principles, guidelines, and recommendations,

Source: ISA2, EIFv2
https://ec.europa.eu/isa2/isa2_en

Syn. Interoperability Supporting Structure

INTEROPERABILITY SALIENCY:
IoP Dimension: Governance IoP
The Interoperability Framework ABB is an interoperability enabler because it helps achieve organisational interoperability by defining a set of rules, practices and a commonly agreed approach to the delivery of European public services. The EIF is an instance of this building block: &quot;The European interoperability framework is a commonly agreed approach to the delivery of European public services in an interoperable manner. It defines basic interoperability guidelines in the form of common principles, models and recommendations.&quot;

EXAMPLES:
The following implementation is an example on how this specific Architecture Building Block (ABB) can be instantiated as a Solution Building Block (SBB):

The new European Interoperability Framework (EIF)
The new European Interoperability Framework (EIF) is part of the Communication (COM(2017)134) from the European Commission adopted on 23 March 2017. The framework gives specific guidance on how to set up interoperable digital public services.
It offers public administrations 47 concrete recommendations on how to improve governance of their interoperability activities, establish cross-organisational relationships, streamline processes supporting end-to-end digital services, and ensure that both existing and new legislation do not compromise interoperability efforts.
The new EIF is undertaken in the context of the Commission priority to create a Digital Single Market in Europe. The public sector, which accounts for over a quarter of total employment and represents approximately a fifth of the EUs GDP through public procurement, plays a key role in the Digital Single Market as a regulator, services provider and employer.
The successful implementation of the EIF will improve the quality of European public services and will create an environment where public administrations can collaborate digitally.
https://ec.europa.eu/isa2/eif_en</skos:definition>
        <skos:topConceptOf rdf:resource="http://data.europa.eu/dr8"/>
    </skos:Concept>

    <skos:Concept rdf:about="http://data.europa.eu/dr8/InteroperabilityGovernance">
        <skos:notation>InteroperabilityGovernance</skos:notation>
        <skos:prefLabel xml:lang="en">[ABB214] Interoperability Governance</skos:prefLabel>
        <skos:definition xml:lang="en">DESCRIPTION:
Set of organizing rules assuring the functioning of an Interoperability Framework . These rules include structures, roles, responsibilities, policies, standards, specifications, practices, decision making and operational procedures.

Source: the New EIF
http://eur-lex.europa.eu/resource.html?uri=cellar:2c2f2554-0faf-11e7-8a35-01aa75ed71a1.0017.02/DOC_3&amp;format=PDF

Syn. Interoperability management method or system

INTEROPERABILITY SALIENCY:
IoP Dimension: Governance IoP
The Interoperability Governance ABB is an interoperability enabler because it helps achieve organisational interoperability as it is &quot; the key to a holistic approach on interoperability, as it brings together all the instruments needed to apply it&quot; (EIF). As stated in EIF Recommendation 20: &quot;Ensure holistic governance of interoperability activities across administrative levels and sectors.&quot;

EXAMPLES:
The following implementations are examples on how this specific Architecture Building Block (ABB) can be instantiated as a Solution Building Block (SBB):

INSPIRE Directive 2007/2/EC of 14 March 2007, Article 18
Member States shall ensure that appropriate structures and mechanisms are designated for coordinating, across the different levels of government, the contributions of all those with an interest in their infrastructures for spatial information. These structures shall coordinate the contributions of, inter alia, users, producers, added-value service providers and coordinating bodies, concerning the identification of relevant data sets, user needs, the provision of information on existing practices and the provision of feedback on the implementation of this Directive.
http://eur-lex.europa.eu/legal-content/EN/TXT/PDF/?uri=CELEX:32007L0002&amp;from=EN

Governance defined in the new European Interoperability Framework (EIF)
 3.1 of the new EIF Annex II: Interoperability governance refers to decisions on interoperability frameworks, institutional arrangements, organisational structures, roles and responsibilities, policies, agreements and other aspects of ensuring and monitoring interoperability at national and EU levels. The European interoperability framework, the Interoperability Action Plan (Annex 1 to the Communication) and the European interoperability architecture (EIRA) are important parts of interoperability governance at the EU level.
http://eur-lex.europa.eu/resource.html?uri=cellar:2c2f2554-0faf-11e7-8a35-01aa75ed71a1.0017.02/DOC_3&amp;format=PDF</skos:definition>
        <skos:topConceptOf rdf:resource="http://data.europa.eu/dr8"/>
    </skos:Concept>

    <skos:Concept rdf:about="http://data.europa.eu/dr8/InteroperabilityOrganisationalAuthority">
        <skos:notation>InteroperabilityOrganisationalAuthority</skos:notation>
        <skos:prefLabel xml:lang="en">[ABB205] Interoperability Organisational Authority</skos:prefLabel>
        <skos:definition xml:lang="en">DESCRIPTION:
An organisation having the powers to govern the interoperability of public administration

Based on the definitions of authority and organisational in the Oxford dictionary.
https://en.oxforddictionaries.com/definition/authority

Syn. Interoperability Coordination Power or Right, or Control

INTEROPERABILITY SALIENCY:
IoP Dimension: Governance IoP
The Interoperability Organisational Authority ABB is an interoperability enabler because it helps achieve organisational interoperability by ensuring political and/or administrative governance of the interoperability capabilities of an organisation as stated in the EIF Recommendation 20: &quot;Ensure holistic governance of interoperability activities across administrative levels and sectors&quot;.

EXAMPLES:
The following implementation is an example on how this specific Architecture Building Block (ABB) can be instantiated as a Solution Building Block (SBB):

INSPIRE Directive 2007/2/EC of 14 March 2007, Article 19

1.	The Commission shall be responsible for coordinating Inspire at Community level and shall be assisted for that purpose by relevant organisations and, in particular, by the European Environment Agency.
2.	Each Member State shall designate a contact point, usually a public authority, to be responsible for contacts with the Commission in relation to this Directive. This contact point will be supported by a coordination structure, taking account of the distribution of powers and responsibilities within the Member State.

http://eur-lex.europa.eu/legal-content/EN/TXT/PDF/?uri=CELEX:32007L0002&amp;from=EN</skos:definition>
        <skos:topConceptOf rdf:resource="http://data.europa.eu/dr8"/>
    </skos:Concept>

    <skos:Concept rdf:about="http://data.europa.eu/dr8/SecurityFramework">
        <skos:notation>SecurityFramework</skos:notation>
        <skos:prefLabel xml:lang="en">[ABB223] Security Framework</skos:prefLabel>
        <skos:definition xml:lang="en">DESCRIPTION:
Agreed governance approach focusing on protection aspects on data, information and knowledge assets and organizational resources handling them.

Source: ISA2, EIFv2
https://ec.europa.eu/isa2/isa2_en

INTEROPERABILITY SALIENCY:
IoP Dimension: Governance IoP
The Security Framework ABB is salient for interoperability because &quot;security and privacy are primary concerns in the provision of public services&quot; (EIF) and, as stated in EIF Recommendation 15: &quot;Define a common security and privacy framework and establish processes for public services to ensure secure and trustworthy data exchange between public administrations and in interactions with citizens and businesses.&quot;

EXAMPLES:

The EU cybersecurity certification framework
The European Commission puts forward the creation of a EU certification framework for ICT security products in its 2017 proposal for a regulation.
On 13 September 2017 the Commission issued a proposal for a regulation on ENISA, the &quot;&quot;EU Cybersecurity Agency&quot;&quot;, and on Information and Communication Technology cybersecurity certification (&apos;&apos;Cybersecurity Act&apos;&apos;).
Certification plays a critical role in increasing trust and security in products and services that are crucial for the digital single market. At the moment, a number of different security certification schemes for ICT products exist in the EU. Without a common framework for EU-wide valid cybersecurity certificates, there is an increasing risk of fragmentation and barriers in the single market.
The proposed certification framework will provide EU-wide certification schemes as a comprehensive set of rules, technical requirements, standards and procedures. This will be based on agreement at EU level for the evaluation of the security properties of a specific ICT-based product or service e.g. smart cards.
The certification will attest that ICT products and services that have been certified in accordance with such a scheme comply with specified cybersecurity requirements. The resulting certificate will be recognized in all Member States, making it easier for businesses to trade across borders and for purchasers to understand the security features of the product or service.
The schemes proposed in the future European framework will rely as much as possible on international standards as a way to avoid creating trade barriers and ensuring coherence with international initiatives.&quot;
https://ec.europa.eu/digital-single-market/en/eu-cybersecurity-certification-framework</skos:definition>
        <skos:topConceptOf rdf:resource="http://data.europa.eu/dr8"/>
    </skos:Concept>

    <skos:Concept rdf:about="http://data.europa.eu/dr8/PrivacyFramework">
        <skos:notation>PrivacyFramework</skos:notation>
        <skos:prefLabel xml:lang="en">[ABB228] Privacy Framework</skos:prefLabel>
        <skos:definition xml:lang="en">DESCRIPTION:
Agreed governance approach focusing on confidentiality aspects on data, information and knowledge assets and organizational resources handling them.

Source: ISA2, EIFv2
https://ec.europa.eu/isa2/isa2_en

INTEROPERABILITY SALIENCY:
IoP Dimension: Governance IoP
The Privacy Framework ABB is salient for interoperability because &quot;security and privacy are primary concerns in the provision of public services&quot; (EIF) and, as stated in EIF Recommendation 15: &quot;Define a common security and privacy framework and establish processes for public services to ensure secure and trustworthy data exchange between public administrations and in interactions with citizens and businesses.&quot;

EXAMPLES:

European Privacy Framework
European privacy legislation is made up of two parts: The Data Protection Directive (95/46/EC) exists as a common ground across Europe. The Directive is a legislative act of the European Union that requires all member states to ensure there is an &quot;adequate&quot; level of data protection. The second part consists of diverse national laws.
https://www.privacy-europe.com/european-privacy-framework.html</skos:definition>
        <skos:topConceptOf rdf:resource="http://data.europa.eu/dr8"/>
    </skos:Concept>

    <skos:Concept rdf:about="http://data.europa.eu/dr8/InteroperabilitySkill">
        <skos:notation>InteroperabilitySkill</skos:notation>
        <skos:prefLabel xml:lang="en">[ABB220] Interoperability Skill</skos:prefLabel>
        <skos:definition xml:lang="en">DESCRIPTION:
Expertise in organizing, implementing and managing interoperability in digital public services

Based on the definitions of skill and organisational in the Oxford dictionary.
https://en.oxforddictionaries.com/definition/skill

Syn. Interoperability Competence

INTEROPERABILITY SALIENCY:
IoP Dimension: Governance IoP
The Interoperability Skill ABB is an interoperability enabler because it helps achieve organisational interoperability by removing a barrier to implement interoperability policies, as stated in the EIF: &quot;Member States should include interoperability skills in their interoperability strategies, acknowledging that interoperability is a multi-dimensional issue that needs awareness and skills in legal, organisational, semantic and technical.&quot;

EXAMPLES:
The following implementation is an example on how this specific Architecture Building Block (ABB) can be instantiated as a Solution Building Block (SBB):

Surveillance3 - Knowledge of English to access and use the open data provided through the EU Open Data Portal
Knowledge of English is required in order to access and use the database of specific products under surveillance or monitoring imported into the EU customs territory in the present and past years. The database for surveillance on the EUROPA web-site displays the volumes of specific products imported into the EU customs territory in the present and in the past year.
https://data.europa.eu/euodp/data/dataset/surveillance</skos:definition>
        <skos:topConceptOf rdf:resource="http://data.europa.eu/dr8"/>
    </skos:Concept>

    <skos:Concept rdf:about="http://data.europa.eu/dr8/Business">
        <skos:notation>Business</skos:notation>
        <skos:prefLabel xml:lang="en">[ABB169] Business</skos:prefLabel>
        <skos:definition xml:lang="en">DESCRIPTION:
Economic operator with a legal entity entitled to perform a private  activity for a profit.

Source: IATE (definition of business, entry Environment [CdT])
http://iate.europa.eu/

Syn. Company

INTEROPERABILITY SALIENCY:
IoP Dimension: Governance IoP
The Business ABB is salient for organisation interoperability because organisations can play the role of consumers of Public Services (Public Administration or businesses), as stated in the EIF: &quot;A European public service comprises any public sector service exposed to a cross-border dimension and supplied by public administrations, either to one another or to businesses and citizens in the Union.&quot;

EXAMPLES:
The following implementation is an example on how this specific Architecture Building Block (ABB) can be instantiated as a Solution Building Block (SBB):

Cosmetic Product Notification Portal - Economic operators
Economic operators involved in intra-community trade are using the Cosmetic Product Notification Portal in order to either notify cosmetic products put on the EU market (distributors) or notify and update the data (manufacturers and importers).
https://webgate.ec.europa.eu/cpnp/faq/?event=faq.show</skos:definition>
        <skos:narrower rdf:resource="http://data.europa.eu/dr8/Organisation"/>
    </skos:Concept>

    <skos:Concept rdf:about="http://data.europa.eu/dr8/PublicAdministration">
        <skos:notation>PublicAdministration</skos:notation>
        <skos:prefLabel xml:lang="en">[ABB172] Public Administration</skos:prefLabel>
        <skos:definition xml:lang="en">DESCRIPTION:
A state, regional or local authority governed by public law or an association formed by one or several such authorities or a private entity mandated by at least one of those authorities or associations to provide public services, when acting under such a mandate.

Source: Connecting Europe Facility (CEF), eIDAS regulation
https://ec.europa.eu/cefdigital/wiki/display/CEFDIGITAL/CEF+Definitions

Syn. Public institution, public body

INTEROPERABILITY SALIENCY:
IoP Dimension: Governance IoP
The Public Administration ABB is salient for organisation interoperability because Public Administrations can play the role both of providers and consumers of Public Services, as stated in the EIF: &quot;A European public service comprises any public sector service exposed to a cross-border dimension and supplied by public administrations, either to one another or to businesses and citizens in the Union.&quot;

EXAMPLES:
The following implementation is an example on how this specific Architecture Building Block (ABB) can be instantiated as a Solution Building Block (SBB):

EWRS  ECHA
The European Chemicals Agency (ECHA) is the driving force among regulatory authorities in implementing the EU&apos;s ground breaking chemicals legislation for the benefit of human health and the environment as well as for innovation and competitiveness.
https://echa.europa.eu/about-us</skos:definition>
        <skos:narrower rdf:resource="http://data.europa.eu/dr8/Organisation"/>
    </skos:Concept>

    <skos:Concept rdf:about="http://data.europa.eu/dr8/Organisation">
        <skos:notation>Organisation</skos:notation>
        <skos:prefLabel xml:lang="en">[ABB7] Organisation</skos:prefLabel>
        <skos:definition xml:lang="en">DESCRIPTION:
An Organisation is a principal that provides and/or consumes Public Services.

Based on the New EIF and the ISA2 Core Vocabularies
http://eur-lex.europa.eu/resource.html?uri=cellar:2c2f2554-0faf-11e7-8a35-01aa75ed71a1.0017.02/DOC_3&amp;format=PDF
https://joinup.ec.europa.eu/asset/cpov/asset_release/core-public-organisation-vocabulary-v100#download-links

Syn. Institution, body

INTEROPERABILITY SALIENCY:
IoP Dimension: Governance IoP
The Organisation ABB is salient for organisation interoperability because organisations can play the role both of providers of Public Services (mainly Public Administrations) and consumers of Public Services (Public Administration or businesses), as stated in the EIF: &quot;A European public service comprises any public sector service exposed to a cross-border dimension and supplied by public administrations, either to one another or to businesses and citizens in the Union.&quot;

EXAMPLES:
The following implementation is an example on how this specific Architecture Building Block (ABB) can be instantiated as a Solution Building Block (SBB):

AFIS - Europol organisation
Europol is the European Unions law enforcement agency. Its main goal is to achieve a safer Europe for the benefit of all the EU citizens.
https://www.europol.europa.eu/</skos:definition>
        <skos:narrower rdf:resource="http://data.europa.eu/dr8/PublicServiceAgent"/>
    </skos:Concept>

    <skos:Concept rdf:about="http://data.europa.eu/dr8/Citizen">
        <skos:notation>Citizen</skos:notation>
        <skos:prefLabel xml:lang="en">[ABB8] Citizen</skos:prefLabel>
        <skos:definition xml:lang="en">DESCRIPTION:
An individual is a principal that provides and/or consumes Public Services. A citizen is a member of a particular country and who has rights because of being born there or because of being given rights.
Every national of a Member State shall be a citizen of the Union. Citizenship of the Union shall be additional to national citizenship and shall not replace it (Treaty of Maastricht on European Union, Title II Provisions on democratic principles, article 8).
The main difference between the two (European citizenship and citizenship of a Member State) is that the rights that citizens enjoy as a result of European citizenship are not matched with duties. Legal basis: Articles 9 to 12 TEU and 18 to 25 TFEU (European Parliament).
The additional rights EU citizenship confers are detailed at http://ec.europa.eu/justice/citizen/index_en.htm (European Commission).

INTEROPERABILITY SALIENCY:
IoP Dimension: Governance IoP
The Citizen ABB is salient for organisation interoperability because citizens can play the role of consumers of Public Services, as stated in the EIF: &quot;A European public service comprises any public sector service exposed to a cross-border dimension and supplied by public administrations, either to one another or to businesses and citizens in the Union.&quot;

Based on EUR-Lex, Europa web site and the Cambridge Dictionary
http://eur-lex.europa.eu/legal-content/EN/TXT/PDF/?uri=OJ:C:2007:306:FULL&amp;from=EN
http://www.europarl.europa.eu/atyourservice/en/displayFtu.html?ftuId=FTU_2.1.1.html
http://dictionary.cambridge.org/dictionary/english/citizen

EXAMPLES:
The following implementation is an example on how this specific Architecture Building Block (ABB) can be instantiated as a Solution Building Block (SBB):

EUROPASS2 - EU citizen
Every national of a Member State shall be a citizen of the Union.
http://europass.cedefop.europa.eu/europass-and-you</skos:definition>
        <skos:narrower rdf:resource="http://data.europa.eu/dr8/PublicServiceAgent"/>
    </skos:Concept>

    <skos:Concept rdf:about="http://data.europa.eu/dr8/PublicServiceAgent">
        <skos:notation>PublicServiceAgent</skos:notation>
        <skos:prefLabel xml:lang="en">[ABB229] Public Service Agent</skos:prefLabel>
        <skos:definition xml:lang="en">DESCRIPTION:
An agent that consumes or delivers a public service on behalf of a principal.

Source:
https://joinup.ec.europa.eu/rdf_entity/http_e_f_fdata_ceuropa_ceu_fw21_f7661a4a0_bbdf9_b4e98_bb04a_b967c6a1053f9

INTEROPERABILITY SALIENCY:
IoP Dimension: Governance IoP
The Public Service Agent is salient for organisational interoperability because it acts on behalf of a Public Service Consumer Agent to consume a Public Service and Public Service Provider Agent to deliver a Publice Service.

EXAMPLES:
Your Europe Advice  ECAS
Your Europe Advice is an EU advice service provided by legal experts from ECAS (European Citizen Action Service) operating under contract with the European Commission. It consists of a team of about 60 lawyers who cover all 24 official EU languages and are familiar both with EU law and national laws in all EU countries. Your Europe Advice replies to questions from citizens or businesses on their personal EU rights. The experts respond to the questions within one week, free of charge and in the language chosen by the user. ECAS mission is to empower citizens to exercise their rights and promote open and inclusive decision-making through the provision of high quality advice, research and advocacy, as well as capacity building for civil society organisations.
http://ecas.org/services/your-europe-advice-yea/ &quot;</skos:definition>
        <skos:topConceptOf rdf:resource="http://data.europa.eu/dr8"/>
    </skos:Concept>

    <skos:Concept rdf:about="http://data.europa.eu/dr8/PublicServiceConsumerAgent">
        <skos:notation>PublicServiceConsumerAgent</skos:notation>
        <skos:prefLabel xml:lang="en">[ABB230] Public Service Consumer Agent</skos:prefLabel>
        <skos:definition xml:lang="en">DESCRIPTION:
Any agent that consumes a public service on behalf of a principal.

Source:
https://joinup.ec.europa.eu/rdf_entity/http_e_f_fdata_ceuropa_ceu_fw21_f7661a4a0_bbdf9_b4e98_bb04a_b967c6a1053f9&quot;

INTEROPERABILITY SALIENCY:
IoP Dimension: Governance IoP
The Public Service Consumer Agent is salient for organisational interoperability because it acts on behalf of a Public Service Consumer (the &quot;Principal&quot;) to consume a Public Service. An agent is described by the tuple &lt;agent_type, principal_type&gt;, where agent_type belongs to {human, machine}, and principal_type belongs to {citizen, business, PA}.

EXAMPLES:
Your Europe Advice  ECAS
Your Europe Advice is an EU advice service provided by legal experts from ECAS (European Citizen Action Service) operating under contract with the European Commission. It consists of a team of about 60 lawyers who cover all 24 official EU languages and are familiar both with EU law and national laws in all EU countries. Your Europe Advice replies to questions from citizens or businesses on their personal EU rights. The experts respond to the questions within one week, free of charge and in the language chosen by the user. ECAS mission is to empower citizens to exercise their rights and promote open and inclusive decision-making through the provision of high quality advice, research and advocacy, as well as capacity building for civil society organisations.
http://ecas.org/services/your-europe-advice-yea/ &quot;</skos:definition>
        <skos:topConceptOf rdf:resource="http://data.europa.eu/dr8"/>
    </skos:Concept>

    <skos:Concept rdf:about="http://data.europa.eu/dr8/PublicServiceConsumer">
        <skos:notation>PublicServiceConsumer</skos:notation>
        <skos:prefLabel xml:lang="en">[ABB5] Public Service Consumer</skos:prefLabel>
        <skos:definition xml:lang="en">DESCRIPTION:
A principal consuming public services.

Source: Based on EIF 2.0
http://ec.europa.eu/isa/documents/isa_annex_ii_eif_en.pdf

INTEROPERABILITY SALIENCY:
IoP Dimension: Governance IoP
The Public Service Consumer ABB is salient for organisational interoperability because it is one of the main actors involved in the interoperability of the public service as stated in the EIF: &quot;Service orientation, upon which the conceptual model for public services is conceived, means that the relationship between service providers and service consumers must be clearly defined&quot;. EIF Recommendation n.29 also suggests:
&quot;Clarify and formalise your organisational relationships for establishing and operating European public services.&quot;

EXAMPLES:
The following implementation is an example on how this specific Architecture Building Block (ABB) can be instantiated as a Solution Building Block (SBB):

Cosmetic Product Notification Portal CPNP - Poison centre, Responsible person, Market surveillance authority, Distributor, Health advisor, Administrations
The CPNP is making this information available electronically to:

	Competent Authorities (for the purposes of market surveillance, market analysis, evaluation and consumer information)
	Poison Centres or similar bodies established by EU countries (for the purposes of medical treatment).

The CPNP is accessible to:

	Competent Authorities
	European Poison Centres
	Cosmetic products responsible persons
	Distributors of cosmetic products

https://ec.europa.eu/growth/sectors/cosmetics/cpnp_fr</skos:definition>
        <skos:topConceptOf rdf:resource="http://data.europa.eu/dr8"/>
    </skos:Concept>

    <skos:Concept rdf:about="http://data.europa.eu/dr8/OrganisationalInteroperabilityAgreement">
        <skos:notation>OrganisationalInteroperabilityAgreement</skos:notation>
        <skos:prefLabel xml:lang="en">[ABB119] Organisational Interoperability Agreement</skos:prefLabel>
        <skos:definition xml:lang="en">DESCRIPTION:
An organisational interoperability agreement is a resource of private nature formalizing governance rules enabling collaboration between digital public services with enabling seamless functioning  value
The Organisational Interoperability Agreement ABB  is a key interoperability enabler because it supports organisational governance interoperability by enabling collaboration between digital public services.

Source ISA2, EIFv2
https://ec.europa.eu/isa2/isa2_en

(*)DECISION (EU) 2015/2240 OF THE EUROPEAN PARLIAMENT AND OF THE COUNCIL of 25 November 2015 establishing a programme on interoperability solutions and common frameworks for European public administrations, businesses and citizens (ISA2 programme) as a means for modernising the public sector.

The agreement should include purposes and goals, terms and conditions, governance, and the description of the channel(s). The EIRA differentiates the following Interoperability Agreements:

	Interoperability Service Agreement (between Public Service Consumers and Public Service Providers;
	Interoperability Collaboration Agreement (between Organisations); or
	Interoperability Provider Agreement (between Public Service Providers).

INTEROPERABILITY SALIENCY:
IoP Dimension: Governance IoP
Concrete and binding documents which set out the precise obligations of two parties cooperating across an interface to achieve interoperability.

EXAMPLES:
The following implementation is an example on how this specific Architecture Building Block (ABB) can be instantiated as a Solution Building Block (SBB):

ICAO Service Level Agreement Template
A Service Level Agreement (SLA) is an example of Interoperability Agreement in which parties agree on the description of the services to be provided by one or several parties to the other one(s). The SLA tackles topics like: service description, optional services, exclusions, limitations, service levels, service credits, escalation procedure, reporting and points of contact.
https://www.icao.int/ESAF/Documents/APIRG/APIRG18/Docs/wp17_appendices_en.pdf</skos:definition>
        <skos:topConceptOf rdf:resource="http://data.europa.eu/dr8"/>
    </skos:Concept>

    <skos:Concept rdf:about="http://data.europa.eu/dr8/PublicServiceProvider">
        <skos:notation>PublicServiceProvider</skos:notation>
        <skos:prefLabel xml:lang="en">[ABB174] Public Service Provider</skos:prefLabel>
        <skos:definition xml:lang="en">DESCRIPTION:
A principal deliverying public services.

Based on IATE definition (definition of service producer, entry Economics, Taxation [Council])
http://iate.europa.eu/

INTEROPERABILITY SALIENCY:
IoP Dimension: Governance IoP
The Public Service Provider ABB is salient for organisational interoperability because it is one of the main actors involved in the interoperability of the public service as stated in the EIF: &quot;&quot;Service orientation, upon which the conceptual model for public services is conceived, means that the relationship between service providers and service consumers must be clearly defined. EIF Recommendation 29 also suggests:
&quot;Clarify and formalise your organisational relationships for establishing and operating European public services.&quot;

EXAMPLES:
The following implementation is an example on how this specific Architecture Building Block (ABB) can be instantiated as a Solution Building Block (SBB):

Ecolabel - Member State Competent Body
The Competent Body is the independent organisation responsible for assessing, awarding, and managing EU Ecolabel applications and licences on the national level. The Competent Body provides guidance on the documents needed for the dossier, such as declarations, data sheets, and test results. Recommendations on product testing laboratories that are ISO 17025 accredited or equivalent are shared, along with any relevant technical expertise needed to complete the application.
Upon application approval, the Competent Body issues the contract and licence upon approving the application. This contract sets out the services or range of products covered within the licence, including any trade names or manufacturers internal reference numbers. It will also lay out the terms of use of the EU Ecolabel, following the standard contract in Annex IV of the Regulation (EC) No 66/2010 of 25 November 2009. Once the contract has been signed, a certificate can be asked for/will be sent, depending on the Competent Body. This certificate will detail: the licence number that can be used with the EU Ecolabel logo; the legal name of the applicant; the services or range of products awarded the EU Ecolabel; all relevant trade names under which the product is sold or the service is marketed. The Competent Body will give the final validation on when the EU Ecolabel logo and the licence number can be used on the EU Ecolabel services and products that have met the criteria.
http://ec.europa.eu/environment/ecolabel/how-to-apply-for-eu-ecolabel.html
http://ec.europa.eu/environment/ecolabel/competent-bodies.html#be</skos:definition>
        <skos:topConceptOf rdf:resource="http://data.europa.eu/dr8"/>
    </skos:Concept>

    <skos:Concept rdf:about="http://data.europa.eu/dr8/PublicServiceDeliveryAgent">
        <skos:notation>PublicServiceDeliveryAgent</skos:notation>
        <skos:prefLabel xml:lang="en">[ABB173] Public Service Delivery Agent</skos:prefLabel>
        <skos:definition xml:lang="en">DESCRIPTION:
Any agent that delivers a public service on behalf of a principal.

Based on definition of Agent class in ISA2 Core Vocabularies
https://joinup.ec.europa.eu/catalogue/distribution/cpsv-ap-specification-v20-pdf

INTEROPERABILITY SALIENCY:
IoP Dimension: Governance IoP
The Public Service Delivery Agent is salient for organisational interoperability because it acts on behalf of a Public Service Provider (the &quot;Principal&quot;) to deliver a Public Service. An agent is described by the tuple &lt;agent_type, principal_type&gt;, where agent_type belongs to {human, machine}, and principal_type belongs to {citizen, business, PA}.

EXAMPLES:
The following implementation is an example on how this specific Architecture Building Block (ABB) can be instantiated as a Solution Building Block (SBB):

Your Europe Advice  ECAS
Your Europe Advice is an EU advice service provided by legal experts from ECAS (European Citizen Action Service) operating under contract with the European Commission. It consists of a team of about 60 lawyers who cover all 24 official EU languages and are familiar both with EU law and national laws in all EU countries. Your Europe Advice replies to questions from citizens or businesses on their personal EU rights. The experts respond to the questions within one week, free of charge and in the language chosen by the user. ECAS mission is to empower citizens to exercise their rights and promote open and inclusive decision-making through the provision of high quality advice, research and advocacy, as well as capacity building for civil society organisations.
http://ecas.org/services/your-europe-advice-yea/</skos:definition>
        <skos:topConceptOf rdf:resource="http://data.europa.eu/dr8"/>
    </skos:Concept>

    <skos:Concept rdf:about="http://data.europa.eu/dr8/ServiceDeliveryModel">
        <skos:notation>ServiceDeliveryModel</skos:notation>
        <skos:prefLabel xml:lang="en">[ABB15] Service Delivery Model</skos:prefLabel>
        <skos:definition xml:lang="en">DESCRIPTION:
The way of delivering to public service consumers, or otherwise interacting with them, for the purpose of supplying specific public services with accessibility value. This involves a number of management practices to ensure that the public services are provided as agreed between the public service provider and the consumer. The service delivery mode should also ensure a constant and stable access to public service in alarm and crisis situations (e.g., COVID 19 pandemic, natural disasters, etc.). Here some examples of service delivery mode: i) Mobile App; ii) Web Portal; iii) Web Services; iv) Contact Center, etc.

Based on the definitions in Innovation Policy Platform (World Bank and OECD)
https://www.innovationpolicyplatform.org/printpdf/12406

INTEROPERABILITY SALIENCY:
IoP Dimension: Behavioural IoP
The Service Delivery Model ABB is a key interoperability enabler because it supports to achieve organisational behavioral interoperability by   enabling the exchange of data, information, and knowledge between digital public services

EXAMPLES:
The following implementation is an example on how this specific Architecture Building Block (ABB) can be instantiated as a Solution Building Block (SBB):

Ecolabel - EU and Member State web sites
EU web site: permits to discover the types of products and services that can be awarded with the EU Ecolabel. Furthermore, the site permits to browse through the EU Ecolabel Product Catalogue and Tourist Accommodation Catalogue to find currently awarded products and services. Member State Competent Bodies provide information to businesses and consumers.
http://ec.europa.eu/environment/ecolabel/index_en.htm
https://www.ecolabel.be/fr
https://www.gov.uk/guidance/apply-for-an-eu-ecolabel</skos:definition>
        <skos:topConceptOf rdf:resource="http://data.europa.eu/dr8"/>
    </skos:Concept>

    <skos:Concept rdf:about="http://data.europa.eu/dr8/BusinessCapability">
        <skos:notation>BusinessCapability</skos:notation>
        <skos:prefLabel xml:lang="en">[ABB12] Business Capability</skos:prefLabel>
        <skos:definition xml:lang="en">DESCRIPTION:
A particular ability or capacity that an organisation may possess or exchange to achieve a specific purpose or outcome.
Defining a business capability involves identifying and describing what needs to be done by the business in support of its overall mission. Business capabilities provide an abstraction of the business reality in a way that helps to simplify conversations between interested stakeholders.

Based on TOGAF definition and description of business capability.
https://www2.opengroup.org/ogsys/catalog/g161

Syn. Business Ability

INTEROPERABILITY SALIENCY:
IoP Dimension: Structural IoP, Behavioral IoP
The Business Capability ABB is salient for organisational interoperability because it defines the main business reason for exchanging business information with other business capabilities in another organisation or in the same organisation.

EXAMPLES:
The following implementation is an example on how this specific Architecture Building Block (ABB) can be instantiated as a Solution Building Block (SBB):

Surveillance3 reporting and generation of data sets
The reporting and generation of data sets business capability brought by Surveillance3 enables the reporting and analysis of data by the end users, through integration mechanisms to other applications. Surveillance3 aggregates the declaration data and additional data such as Binding Tariff Information (BTI) decisions and Surveillance definitions in order to produce consolidated reports about:
1.	The BTI usage for the DG TAXUD BTI sector users and for Member State users and
2.	Surveillance statistical data

http://ec.europa.eu/taxation_customs/dds2/surv/surv_consultation.jsp?Lang=en</skos:definition>
        <skos:topConceptOf rdf:resource="http://data.europa.eu/dr8"/>
    </skos:Concept>

    <skos:Concept rdf:about="http://data.europa.eu/dr8/ExchangeOfBusinessInformation">
        <skos:notation>ExchangeOfBusinessInformation</skos:notation>
        <skos:prefLabel xml:lang="en">[ABB170] Exchange of Business Information</skos:prefLabel>
        <skos:definition xml:lang="en">DESCRIPTION:
Business capability on exchanging data, information, and Knowledge

Based on TOGAF definitions.
https://www2.opengroup.org/ogsys/catalog/g161
http://pubs.opengroup.org/architecture/togaf9-doc/arch/

(*)DECISION (EU) 2015/2240 OF THE EUROPEAN PARLIAMENT AND OF THE COUNCIL of 25 November 2015 establishing a programme on interoperability solutions and common frameworks for European public administrations, businesses and citizens (ISA2 programme) as a means for modernising the public sector.

Syn. Exchange of Business Facts, Exchange of Business Data, Exchange of Business Opinions

INTEROPERABILITY SALIENCY:
IoP Dimension: Structural IoP, Behavioral IoP
The Exchange of business Information ABB  is salient for interoperability because it helps achieve organisational interoperability by ensuring compatible interaction between organisations, as stated in the EIF: &quot;For the purpose of the EIF, interoperability is the ability of organisations to interact towards mutually beneficial goals, involving the sharing of information and knowledge between these organisations, through the business processes they support, by means of the exchange of data between their ICT systems&quot;.

EXAMPLES:
The following implementation is an example on how this specific Architecture Building Block (ABB) can be instantiated as a Solution Building Block (SBB):

Easi-MicPro - Agreement of Code of good conduct
Proof of transparency and usage of pan-European reporting standards.
https://webgate.ec.europa.eu/easi-micpro/application#!cogcPublicPage</skos:definition>
        <skos:topConceptOf rdf:resource="http://data.europa.eu/dr8"/>
    </skos:Concept>

    <skos:Concept rdf:about="http://data.europa.eu/dr8/BusinessInformation">
        <skos:notation>BusinessInformation</skos:notation>
        <skos:prefLabel xml:lang="en">[ABB13] Business Information</skos:prefLabel>
        <skos:definition xml:lang="en">DESCRIPTION:
Organizationally constructed meaning describing business facts, assets, or opinions that are exchanged in the context of a public service to support its delivery. Examples include an invoice, a medical prescription, a driving license.

Based on TOGAF guide about business capabilities and TOGAF definition of information.
https://www2.opengroup.org/ogsys/catalog/g161
http://pubs.opengroup.org/architecture/togaf9-doc/arch/

Syn. Business Facts, Business Data, Business Opinions

INTEROPERABILITY SALIENCY:
IoP Dimension: Behavioral IoP
The Business Information ABB is salient for organisational interoperability because it represents the entity being exchanged between organisations. Its interoperability needs to be guaranteed by means of organisational and semantic interoperability specifications.

EXAMPLES:
The following implementation is an example on how this specific Architecture Building Block (ABB) can be instantiated as a Solution Building Block (SBB):

Surveillance3 - Surveillance information
Published Surveillance information (Business Information) on Europa: Textile category 1 - Cotton yarn, not put up for retail sale [Council Regulation (EEC) No 3030/93] from Belarus in 2015: see URL for details.
http://ec.europa.eu/taxation_customs/dds2/surv/surv_data_list.jsp?Lang=en&amp;survNumber=670010&amp;survType=1&amp;startDate=20150101&amp;originCode=BY</skos:definition>
        <skos:topConceptOf rdf:resource="http://data.europa.eu/dr8"/>
    </skos:Concept>

    <skos:Concept rdf:about="http://data.europa.eu/dr8/PublicServiceCatalogue">
        <skos:notation>PublicServiceCatalogue</skos:notation>
        <skos:prefLabel xml:lang="en">[ABB124] Public Service Catalogue</skos:prefLabel>
        <skos:definition xml:lang="en">DESCRIPTION:
A catalogue of public services is a collection of descriptions of active public services that are provided by public administrations at any administrative level (i.e. local, regional, national or pan-European). All public service descriptions published in a catalogue of public services conform to a common data model for representing public services.
This ABB is a key interoperability enabler (*) for sharing/PROVISIONING and reusing/CONSUMING of front-office public services.

Source: ISA2 Core Vocabularies
https://joinup.ec.europa.eu/catalogue/distribution/cpsv-ap-specification-v20-pdf

(*)DECISION (EU) 2015/2240 OF THE EUROPEAN PARLIAMENT AND OF THE COUNCIL of 25 November 2015 establishing a programme on interoperability solutions and common frameworks for European public administrations, businesses and citizens (ISA2 programme) as a means for modernising the public sector.

Syn. Public Service Registry, Public Service Inventory

INTEROPERABILITY SALIENCY:
IoP Dimension: Structural IoP
The Public Service Catalogue ABB  is a key interoperability enabler because it supports to achieve organisational structural interoperability by ensuring the provision/consumption of  front-office digital public services. Catalogues are also key element of the EIF &quot;Integrated Public Service Governance&quot; conceptual model. According to EIF Recommendation 44: &quot;Put in place catalogues of public services, public data, and interoperability solutions and use common models for describing them.&quot;

EXAMPLES:
The following implementation is an example on how this specific Architecture Building Block (ABB) can be instantiated as a Solution Building Block (SBB):

FEDICT service catalogue
FEDICT, part of the Federal Public Service Policy and Support of Belgium, offers a public service catalogue. Here are a few examples of the offered services: Company data (company information and certificates), Digiflow (access to online certificates), E-mail Relay (relay of e-mail to and from the federal public services and institutions, as a protection to viruses and spam), eBirth (birth online notification and transfer of statistics), eDepot (for notaries), Federal Authentication Service (authentication of individuals for access to online government applications), etc.
http://www.fedict.belgium.be/en/service_catalogue</skos:definition>
        <skos:topConceptOf rdf:resource="http://data.europa.eu/dr8"/>
    </skos:Concept>

    <skos:Concept rdf:about="http://data.europa.eu/dr8/SharedGovernanceFramework">
        <skos:notation>SharedGovernanceFramework</skos:notation>
        <skos:prefLabel xml:lang="en">[ABB358] Shared Governance Framework</skos:prefLabel>
        <skos:definition xml:lang="en">DESCRIPTION:
A shared governance framework is formed by [re]usable governance resources, with  convergence power, in relation to public policy goals attainment, given by their functioning impact via communication and harmonization, across the levels of a public administration (central, regional, local) towards the achievement of the public policy goals, enabling :
i)	structural interoperability by organisational resources supporting reusing and/or sharing of digital public services (i.e. public services catalogue enabling provisioning/consuming public services cross public administrations and cross borders);
ii)	behavioural interoperability by organisational resources supporting exchanging capabilities of data, information or knowledge with internal/external peers (i.e. service delivery model enabling that data/information/knowledge be provisioned/consumed cross public administrations and cross borders); and
iii)	governance interoperability by governance resources supporting the collaboration with internal/external peers exchanging data, information or knowledge (i.e. Organisational Interoperability Agreements on organisational terms/conditions enabling sharing, reuse and exchange of data/information/knowledge cross public administrations and cross borders).

INTEROPERABILITY SALIENCY
IoP dimensions: Structural IoP, Behavioral IoP, Governance IoP
This ABB is a key interoperability enabler because it supports to achieve legal interoperability with public policy goals convergence value by  all in all enabling i) sharing/provisioning/reusing/consumption of legislation on digital public services,  ii) the exchange of data, information, and knowledge between digital public services, and iii) collaboration between digital public services</skos:definition>
        <skos:topConceptOf rdf:resource="http://data.europa.eu/dr8"/>
    </skos:Concept>

    <skos:Collection rdf:about="http://data.europa.eu/dr8/view/SemanticView">
        <skos:notation>SemanticView</skos:notation>
        <skos:prefLabel xml:lang="en">Semantic View</skos:prefLabel>
        <skos:member rdf:resource="http://data.europa.eu/dr8/DataPolicy"/>
        <skos:member rdf:resource="http://data.europa.eu/dr8/Representation"/>
        <skos:member rdf:resource="http://data.europa.eu/dr8/DataSetCatalogue"/>
        <skos:member rdf:resource="http://data.europa.eu/dr8/DataSet"/>
        <skos:member rdf:resource="http://data.europa.eu/dr8/Data"/>
        <skos:member rdf:resource="http://data.europa.eu/dr8/DescriptiveMetadataPolicy"/>
        <skos:member rdf:resource="http://data.europa.eu/dr8/MasterDataPolicy"/>
        <skos:member rdf:resource="http://data.europa.eu/dr8/OpenDataPolicy"/>
        <skos:member rdf:resource="http://data.europa.eu/dr8/BaseRegistryDataPolicy"/>
        <skos:member rdf:resource="http://data.europa.eu/dr8/DataPortabilityPolicy"/>
        <skos:member rdf:resource="http://data.europa.eu/dr8/ReferenceDataPolicy"/>
        <skos:member rdf:resource="http://data.europa.eu/dr8/DataEntity"/>
        <skos:member rdf:resource="http://data.europa.eu/dr8/CoreDataModel"/>
        <skos:member rdf:resource="http://data.europa.eu/dr8/DataSyntax"/>
        <skos:member rdf:resource="http://data.europa.eu/dr8/DataModel"/>
        <skos:member rdf:resource="http://data.europa.eu/dr8/ControlledVocabulary"/>
        <skos:member rdf:resource="http://data.europa.eu/dr8/SharedKnowledgeBase"/>
        <skos:member rdf:resource="http://data.europa.eu/dr8/DataMapping"/>
        <skos:member rdf:resource="http://data.europa.eu/dr8/OntologiesCatalogue"/>
        <skos:member rdf:resource="http://data.europa.eu/dr8/Ontology"/>
        <skos:member rdf:resource="http://data.europa.eu/dr8/DataOwner"/>
        <skos:member rdf:resource="http://data.europa.eu/dr8/SemanticInteroperabilityAgreement"/>
        <skos:member rdf:resource="http://data.europa.eu/dr8/DataMapping"/>
        <skos:member rdf:resource="http://data.europa.eu/dr8/DataMappingCatalogue"/>
        <skos:member rdf:resource="http://data.europa.eu/dr8/SemanticAgreement"/>
        <skos:member rdf:resource="http://data.europa.eu/dr8/SecurityPolicy"/>
        <skos:member rdf:resource="http://data.europa.eu/dr8/PrivacyPolicy"/>
    </skos:Collection>

    <skos:Concept rdf:about="http://data.europa.eu/dr8/DataPolicy">
        <skos:notation>DataPolicy</skos:notation>
        <skos:prefLabel xml:lang="en">[ABB30] Data Policy</skos:prefLabel>
        <skos:definition xml:lang="en">DESCRIPTION:
A set of broad, high level principles which form the guiding framework in which data management can operate.

Source: OECD
https://stats.oecd.org/glossary/detail.asp?ID=4454

INTEROPERABILITY SALIENCY:
IoP Dimension: Governance IoP
The Data Policy ABB is salient for semantic interoperability because it provides a guiding framework to manage data and information according to interoperability principles as stated in the EIF recommendation n 30: &quot;Perceive data and information as a public asset that should be appropriately generated, collected, managed, shared, protected and preserved.&quot;

EXAMPLES:
The following implementation is an example on how this specific Architecture Building Block (ABB) can be instantiated as a Solution Building Block (SBB):

EU SCIENCE HUB - The European Commission&apos;s science and knowledge service - JRC&apos;s Data policy
The JRC&apos;s data policy is driven by transparency with the aim of contributing to innovation. It is a pillar of the development and implementation of scientific knowledge management at the JRC. It follows the commitments and regulatory basis of the Commission Decision on the reuse of Commission documents (2011/833/EU).

The objectives for adopting and implementing the JRC data policy include:

	Share and use data on the basis of the JRC Open Data principles: fully, freely, openly and timely;
	To be transparent on the reasons for restricted access to certain data;
	Provide a coordinated approach to the acquisition of data by the JRC;
	Facilitate management, broaden access and use of JRC data;
	Reinforce goals of Horizon 2020;
	Support EU implementation of the G8 Open Data Charter;
	Continuously support evidence-based decision making and research;
	Ensure that JRC data is made available through the EU Open Data Portal.

For a successful implementation process, the JRC&apos;s data policy lays down implementation principles with respect to responsible entities, overall implementation guidelines, and their individual elements like data management plans, as well as the monitoring of its implementation.
https://ec.europa.eu/jrc/en/about/jrc-in-brief/data-policy
http://publications.jrc.ec.europa.eu/repository/bitstream/JRC95307/lb-na-27163-en-n%20.pdf</skos:definition>
        <skos:topConceptOf rdf:resource="http://data.europa.eu/dr8"/>
    </skos:Concept>

    <skos:Concept rdf:about="http://data.europa.eu/dr8/Representation">
        <skos:notation>Representation</skos:notation>
        <skos:prefLabel xml:lang="en">[ABB182] Representation</skos:prefLabel>
        <skos:definition xml:lang="en">DESCRIPTION:
The description of the perceptible configuration of business information or a Legal act. Representations can be classified in various ways; for example, in terms of medium (e.g. electronic or paper documents, audio, etc.) or format (HTML, ASCII, PDF, RTF, etc.).

Source: ArchiMate v3
http://pubs.opengroup.org/architecture/archimate3-doc/chap08.html

INTEROPERABILITY SALIENCY:
IoP Dimension: Behavioral IoP
The Representation ABB is a key interoperability enabler because it ensures a common and unambiguous interpretation of Data (*).

(*)DECISION (EU) 2015/2240 OF THE EUROPEAN PARLIAMENT AND OF THE COUNCIL of 25 November 2015 establishing a programme on interoperability solutions and common frameworks for European public administrations, businesses and citizens (ISA2 programme) as a means for modernising the public sector

EXAMPLES:
The following implementation is an example on how this specific Architecture Building Block (ABB) can be instantiated as a Solution Building Block (SBB):

ESPD data - XML representation
European Single Procurement Document (ESPD) is a self-declaration of the businesses&apos; financial status, abilities and suitability for a public procurement procedure. It is available in all EU languages and used as a preliminary evidence of fulfilment of the conditions required in public procurement procedures across the EU. Thanks to the ESPD, the tenderers no longer have to provide full documentary evidence and different forms previously used in the EU procurement, which means a significant simplification of access to cross-border tendering opportunities. [...] The online form can be filled in, printed and then sent to the buyer together with the rest of the bid.
https://ec.europa.eu/tools/espd/filter?lang=en</skos:definition>
        <skos:topConceptOf rdf:resource="http://data.europa.eu/dr8"/>
    </skos:Concept>

    <skos:Concept rdf:about="http://data.europa.eu/dr8/DataSetCatalogue">
        <skos:notation>DataSetCatalogue</skos:notation>
        <skos:prefLabel xml:lang="en">[ABB24] Data Set Catalogue</skos:prefLabel>
        <skos:definition xml:lang="en">DESCRIPTION:
Indexed inventory of data sets with comprehensiveness and trustiness value.
This ABB is a key interoperability enabler (*) for sharing/PROVISIONING and reusing/CONSUMING Data.

Based on W3C
http://www.w3.org/TR/vocab-dcat/#class-catalog

(*)DECISION (EU) 2015/2240 OF THE EUROPEAN PARLIAMENT AND OF THE COUNCIL of 25 November 2015 establishing a programme on interoperability solutions and common frameworks for European public administrations, businesses and citizens (ISA2 programme) as a means for modernising the public sector

Syn. Data Set Registry, Data Set Inventory

INTEROPERABILITY SALIENCY:
IoP Dimension: Structural IoP
The Data Set catalogue  ABB is a key interoperability enabler because it supports to achieve semantic structural interoperability by ensuring the provision/consumption of  data by digital public services.

EXAMPLES:
The following implementation is an example on how this specific Architecture Building Block (ABB) can be instantiated as a Solution Building Block (SBB):

Agricultural and Vegetable Catalogue
The seed of varieties of agricultural and plant species and varieties of vegetable species that are published in the EU level common catalogue is subject to no marketing restrictions with the Community. Publication in the catalogue must be approved as fulfilling minimum requirements laid down in legislation. Data is published on the contents of the catalogues for agricultural and vegetal species and maintainers with details of the reference list.
https://data.europa.eu/euodp/data/dataset/7A98oEqVa83q6L7tHQ</skos:definition>
        <skos:topConceptOf rdf:resource="http://data.europa.eu/dr8"/>
    </skos:Concept>

    <skos:Concept rdf:about="http://data.europa.eu/dr8/DataSet">
        <skos:notation>DataSet</skos:notation>
        <skos:prefLabel xml:lang="en">[ABB23] Data Set</skos:prefLabel>
        <skos:definition xml:lang="en">DESCRIPTION:
A Data Set is a collection of data, published or curated by a single agent, and available for access or download in one or more formats.

It is useful to remember that when a common interconnecting infrastructure for base registries is available, legislation is used to force its use. The use of interconnecting infrastructure prevents the proliferation of pointto-point interconnections. Stakeholders should be involved in developing the
legislation and be given enough time to prepare for implementation.

Source: W3C
http://www.w3.org/TR/vocab-dcat/#class-dataset

Other Source: ACCESS TO BASE REGISTRIES
https://ec.europa.eu/isa2/sites/isa/files/publications/access-to-base-registries-good-practices-on-building-successful-interconnections-of-base-registries.pdf

INTEROPERABILITY SALIENCY:
IoP Dimension: Structural IoP
The Data Set ABB is salient for semantic interoperability because it provides a collection of data to be shared or exchanged between ICT systmes as stated in the EIF recommendation n 30: &quot;Perceive data and information as a public asset that should be appropriately generated, collected, managed, shared, protected and preserved.&quot;

EXAMPLES:
The following implementation is an example on how this specific Architecture Building Block (ABB) can be instantiated as a Solution Building Block (SBB):

European Union Data Portal - The European Union Open Data Portal (EU ODP) gives you access to open data published by EU institutions and bodies. All the data you can find via this catalogue are free to use and reuse for commercial or non-commercial purposes.
https://data.europa.eu/euodp/data/dataset</skos:definition>
        <skos:topConceptOf rdf:resource="http://data.europa.eu/dr8"/>
    </skos:Concept>

    <skos:Concept rdf:about="http://data.europa.eu/dr8/Data">
        <skos:notation>Data</skos:notation>
        <skos:prefLabel xml:lang="en">[ABB22] Data</skos:prefLabel>
        <skos:definition xml:lang="en">DESCRIPTION:
Data are symbols obtained through an encoding process of business information or a legal act.

Source: ISO-IEC-2382-1 * 1993 *
https://www.iso.org/obp/ui/#iso:std:iso-iec:2382:ed-1:v1:en

(*)DECISION (EU) 2015/2240 OF THE EUROPEAN PARLIAMENT AND OF THE COUNCIL of 25 November 2015  establishing a programme on interoperability solutions and common frameworks for European public administrations, businesses and citizens (ISA2 programme) as a means for modernising the public sector

Syn. Information

INTEROPERABILITY SALIENCY:
IoP Dimension: Structural IoP
The Data ABB is salient for semantic interoperability because it represents the most important mean of interaction between ICT systems of organisations in order to ensure interoperability as stated in the EIF recommendation n 30: &quot;Perceive data and information as a public asset that should be appropriately generated, collected, managed, shared, protected and preserved.&quot;

EXAMPLES:
The following implementation is an example on how this specific Architecture Building Block (ABB) can be instantiated as a Solution Building Block (SBB):

Aggregated data of the Emission Trading System (ETS):
EU ETS data is aggregated by country, by main activity type and by year on the verified emissions, allowances and surrendered units of the more than 12 000 stationary installations reporting under the EU emission trading system, as well as 1400 aircraft operators. Aggregated data can be viewed with the EU ETS data viewer, which provides an easy access to emission trading data contained in the European Union Transaction Log (EUTL).
https://www.eea.europa.eu/data-and-maps/dashboards/emissions-trading-viewer-1</skos:definition>
        <skos:topConceptOf rdf:resource="http://data.europa.eu/dr8"/>
    </skos:Concept>

    <skos:Concept rdf:about="http://data.europa.eu/dr8/DescriptiveMetadataPolicy">
        <skos:notation>DescriptiveMetadataPolicy</skos:notation>
        <skos:prefLabel xml:lang="en">[ABB352] Descriptive Metadata Policy</skos:prefLabel>
        <skos:definition xml:lang="en">DESCRIPTION:
A Data Policy aiming at making data discoverable and identifiable. It may mandate elements such as title, abstract, author, and keywords.

Source:
http://www.niso.org/publications/press/UnderstandingMetadata.pdf

INTEROPERABILITY SALIENCY:
IoP Dimension: Governance IoP
The Descriptive Metadata Policy ABB is salient for semantic interoperability because metadata facilitates opening and sharing data by providing the appropriate format, description of the content, high level of quality in order to achieve interoperability as stated in the EIF recommendation n 42: &quot;[..] Ensure that open data is accompanied by high quality, machine-readable metadata in non-proprietary formats, including a description of their content, the way data is collected and its level of quality and the licence terms under which it is made available. The use of common vocabularies for expressing metadata is recommended.&quot;

EXAMPLES:
The following implementation is an example on how this specific Architecture Building Block (ABB) can be instantiated as a Solution Building Block (SBB):

Dublin Core Metadata Element Set, Version 1.1: Reference Description
The Dublin Core Metadata Element Set is a vocabulary of fifteen properties for use in resource description. The name &quot;Dublin&quot; is due to its origin at a 1995 invitational workshop in Dublin, Ohio; &quot;core&quot; because its elements are broad and generic, usable for describing a wide range of resources.
The fifteen element &quot;Dublin Core&quot; described in this standard is part of a larger set of metadata vocabularies and technical specifications maintained by the Dublin Core Metadata Initiative (DCMI). The full set of vocabularies, DCMI Metadata Terms [DCMI-TERMS], also includes sets of resource classes (including the DCMI Type Vocabulary [DCMI-TYPE]), vocabulary encoding schemes, and syntax encoding schemes. The terms in DCMI vocabularies are intended to be used in combination with terms from other, compatible vocabularies in the context of application profiles and on the basis of the DCMI Abstract Model [DCAM].
http://dublincore.org/documents/dces/</skos:definition>
        <skos:narrower rdf:resource="http://data.europa.eu/dr8/DataPolicy"/>
    </skos:Concept>

    <skos:Concept rdf:about="http://data.europa.eu/dr8/MasterDataPolicy">
        <skos:notation>MasterDataPolicy</skos:notation>
        <skos:prefLabel xml:lang="en">[ABB353] Master Data Policy</skos:prefLabel>
        <skos:definition xml:lang="en">DESCRIPTION:
A Data Policy applying to the authoritative, most accurate data that is available about key business entities, used to establish the context for business transactions and transactional data.

Source: DAMA DM_BOK
http://www.dama.org

INTEROPERABILITY SALIENCY:
IoP Dimension: Governance IoP
The Master Data Policy ABB is salient for semantic interoperability because Master Data is used to establish the context for business transactions and transactional data by providing accurate data usually stored and available for reuse by other parties. Its management should be prioritised as stated in the EIF recommendation n 31: &quot;Put in place an information management strategy at the highest possible level to avoid fragmentation and duplication. Management of metadata, master data and reference data should be prioritised.&quot;

EXAMPLES:
The following implementation is an example on how this specific Architecture Building Block (ABB) can be instantiated as a Solution Building Block (SBB):

EMVO: EMVS Master Data Guide
The EMVS (European Medicines Verification System) requires that OBPs (OnBoarding Partners) upload both product master data and product batch/pack data.
The aim of this guide is to clarify what data is expected to be used for the EMVS master data noting that the long-term goal is to source directly from the IDMP/SPOR system.

https://emvo-medicines.eu/new/wp-content/uploads/EMVO_0122_EMVS-Master-Data-Guide-1.pdf</skos:definition>
        <skos:narrower rdf:resource="http://data.europa.eu/dr8/DataPolicy"/>
    </skos:Concept>

    <skos:Concept rdf:about="http://data.europa.eu/dr8/OpenDataPolicy">
        <skos:notation>OpenDataPolicy</skos:notation>
        <skos:prefLabel xml:lang="en">[ABB354] Open Data Policy</skos:prefLabel>
        <skos:definition xml:lang="en">DESCRIPTION:
The rules and practice of publishing (raw) data in a way that is accessible, reusable, machine readable and licensed permissively. It can be generated by a wide range of parties, including public authorities, the semi-public sector, businesses and the public. In the case of public authorities, such as European Union organisations, making their data available for public reuse supports economic development, openness and transparency.

Source: EU Open Data guide
http://bookshop.europa.eu/en/eu-open-data-pbOA0416036/downloads/OA-04-16-036-EN-C/OA0416036ENC_002.pdf?FileName=OA0416036ENC_002.pdf&amp;SKU=OA0416036ENC_PDF&amp;CatalogueNumber=OA-04-16-036-EN-C

INTEROPERABILITY SALIENCY:
IoP Dimension: Governance IoP
The Open Data Policy ABB is salient for semantic interoperability because Open Data is a part of the basic components of the EIF&apos;s conceptual model for integrated public services. Opening of public sector datasets for sharing and reuse is encouraged by the Directive on the reuse of public sector information, which provides a common legal framework for reuse of public sector data as stated in the EIF recommendation n 2: &quot;Publish the data you own as open data unless certain restrictions apply.&quot;

EXAMPLES:
EU implementation of the G8 Open Data Charter
https://ec.europa.eu/digital-single-market/en/news/eu-implementation-g8-open-data-charter</skos:definition>
        <skos:narrower rdf:resource="http://data.europa.eu/dr8/DataPolicy"/>
    </skos:Concept>

    <skos:Concept rdf:about="http://data.europa.eu/dr8/BaseRegistryDataPolicy">
        <skos:notation>BaseRegistryDataPolicy</skos:notation>
        <skos:prefLabel xml:lang="en">[ABB351] Base Registry Data Policy</skos:prefLabel>
        <skos:definition xml:lang="en">DESCRIPTION:
A Data Policy applying to a trusted authentic source of information under the control of an appointed public administration or organisation appointed by government.

According to the European Interoperability Framework, base registries are: reliable sources of basic information on items such as persons, companies, vehicles, licenses, buildings, locations and roads and are authentic and authoritative and form, separately or in combination, the cornerstone of public services.

Source: the New EIF
http://eur-lex.europa.eu/resource.html?uri=cellar:2c2f2554-0faf-11e7-8a35-01aa75ed71a1.0017.02/DOC_3&amp;format=PDF

INTEROPERABILITY SALIENCY:
IoP Dimension: Governance IoP
The Base Registry Data Policy ABB is salient for semantic interoperability because base registries include &quot;authorative sources of information&quot;, that need to be properly governed and made available. EIF&apos;s includes base registries in the conceptual model for integrated public services, and describes it as &quot;the cornerstone of European public service delivery&quot;. EIF gives several recommendations on how to manage and interact with base registries (recommendation 37, 38, 39 and 40).

EXAMPLES:
The following implementation is an example on how this specific Architecture Building Block (ABB) can be instantiated as a Solution Building Block (SBB):

GOOD PRACTICES ON BUILDING SUCESSFUL INTERCONNECTIONS OF BASE REGISTRIES
In order to provide quick and user-friendly public services to citizens and businesses, public administrations are trying to adopt customer-centric approaches and readjust their ways of working.
One way to achieve efficiency and increase user-friendliness is through the once-only principle. Instead of asking the citizen for information that they have already provided, public administrations will reuse the information they already have. Much of this information is stored in authoritative databases called base registries. As the authentic sources of data for public administrations, base registries are one of the basic building blocks of public services and are the key to making the once-only principle a reality.
The document contains some good practices to foster access to the data contained in these base registries.
The good practices presented, are grouped according to the layered interoperability model proposed by the European Interoperability
Framework (EIF).
https://ec.europa.eu/isa2/sites/isa/files/publications/access-to-base-registries-good-practices-on-building-successful-interconnections-of-base-registries.pdf</skos:definition>
        <skos:narrower rdf:resource="http://data.europa.eu/dr8/MasterDataPolicy"/>
    </skos:Concept>

    <skos:Concept rdf:about="http://data.europa.eu/dr8/DataPortabilityPolicy">
        <skos:notation>DataPortabilityPolicy</skos:notation>
        <skos:prefLabel xml:lang="en">[ABB362] Data Portability Policy</skos:prefLabel>
        <skos:definition xml:lang="en">DESCRIPTION:
The data portability policy implements the right to data portability, which is one of eight rights enforced by the EU General Data Protection Regulation (GDPR). It regulates the exchange of data, allowing data subjects to obtain data that a data controller holds on them and to reuse it for their own purposes.
Accourding to GDPR, Individuals are free to either store the data for personal use or to transmit it to another data controller. The data must be received in a structured, commonly used and machine-readable format.

According to the Article 29 of the Data Protection Working Party (WP29), an advisory body made up of representatives from each EU member state, this right support[s] the free flow of personal data in the EU and foster[s] competition between controllers.
The right to data portability applies:
- To personal data that an individual has given to a data controller;
- When the processing is carried out by automated means; and
- Where the processing is based on the individuals consent or for the performance or a contract.

INTEROPERABILITY SALIENCY:
IoP Dimension: Governance IoP
The Data Portability Policy ABB is salient for semantic interoperability because it regulates how data can be exchanged and its reuse.

EXAMPLE:
The following implementation is an example on how this specific Architecture Building Block (ABB) can be instantiated as a Solution Building Block (SBB):</skos:definition>
        <skos:narrower rdf:resource="http://data.europa.eu/dr8/DataPolicy"/>
    </skos:Concept>

    <skos:Concept rdf:about="http://data.europa.eu/dr8/ReferenceDataPolicy">
        <skos:notation>ReferenceDataPolicy</skos:notation>
        <skos:prefLabel xml:lang="en">[ABB355] Reference Data Policy</skos:prefLabel>
        <skos:definition xml:lang="en">DESCRIPTION:
A Data Policy applying to data used to organise or categorise other data, or for relating data to information both within and beyond the boundaries of the enterprise. Usually it mandates the use of codes and descriptions, or definitions.

Source: DAMA DM_BOK
http://www.dama.org

Reference data consists typically of a small, discrete set of values that are not updated as part of business transactions but are usually used to impose consistent classication. Reference data normally has a low update frequency. Reference data is relevant across more than one business systems belonging to different organisations and sectors
[Source: J. Jordan &amp; C. Ellen (2009). Business need, data and business intelligence].

INTEROPERABILITY SALIENCY:
IoP Dimension: Governance IoP
The Reference Data Policy ABB is salient for semantic interoperability because Reference Data can be shared and reused (e.g. in the form of taxonomies or controlled vocabularies) between organisation to agree on some  basic information. Management of reference data is a priority as suggested by EIF&apos;s recommendation 31: &quot;Put in place an information management strategy at the highest possible level to avoid fragmentation and duplication. Management of metadata, master data and reference data should be prioritised.&quot;

EXAMPLES:
The following implementation is an example on how this specific Architecture Building Block (ABB) can be instantiated as a Solution Building Block (SBB):

FIRDS Reference Data System
The intended audience of this document is National Competent Authorities, Trading Venues
Systematic Internalisers and Data Reporting Service Provider (including Approved Publication
Arrangement and Consolidated Tape Providers), who are going to implement system interfaces
for the uploading of data to the Financial Instruments Reference Data System.

This document aims to specify the exchange of Reference Data Information (RDI) between NCAS,
Trading Venues, Systematic Internalisers and the Financial Instruments Reference System.

https://www.esma.europa.eu/sites/default/files/library/esma65-11-1193_firds_reference_data_reporting_instructions_v2.0.pdf</skos:definition>
        <skos:narrower rdf:resource="http://data.europa.eu/dr8/MasterDataPolicy"/>
    </skos:Concept>

    <skos:Concept rdf:about="http://data.europa.eu/dr8/DataEntity">
        <skos:notation>DataEntity</skos:notation>
        <skos:prefLabel xml:lang="en">[ABB20] Data Entity</skos:prefLabel>
        <skos:definition xml:lang="en">DESCRIPTION:
A classification of objects found in the real world described by the Noun part of speech  persons, places, things, concepts, and events  of interest to the enterprise.

Source: DAMA DM_BOK
http://www.dama.org

Syn. Coherent set of information

INTEROPERABILITY SALIENCY:
IoP Dimension: Structural IoP, Behavioral IoP, Governance IoP
The Data Entity ABB is salient for semantic interoperability because it represents a basic component of a Data Model ABB.

EXAMPLES:
The following implementation is an example on how this specific Architecture Building Block (ABB) can be instantiated as a Solution Building Block (SBB):

EURES - Job vacancy
Most of the jobs on the EURES Job Mobility Portal come from the job vacancies databases managed by the Public Employment Services of the countries participating in EURES. Using a technology called Web Services, the EURES search engine instantly, in real time, interrogates each national database for jobs. These jobs can be of two types:
EURES jobs&quot;, displayed with a blue flag, which are jobs where an employer has expressed an interest in recruiting from another country, or any other jobs advertised in the national jobs databases.
There is, in addition, a central database where EURES advisers can manually post jobs that will all be flagged as &quot;EURES jobs&quot;. This is for the time being the only way for those few countries that are not yet fully connected to Web Services to advertise jobs on the EURES portal. This solution can, however, also be used for other specific purposes, such as when an employer wishes to publish a vacancy in several languages etc., which may not always be possible in a national database.
https://ec.europa.eu/eures/public/en/advertise-a-job?lang=en&amp;app=1.8.1p6-build-0&amp;pageCode=advertise_job</skos:definition>
        <skos:narrower rdf:resource="http://data.europa.eu/dr8/DataModel"/>
    </skos:Concept>

    <skos:Concept rdf:about="http://data.europa.eu/dr8/CoreDataModel">
        <skos:notation>CoreDataModel</skos:notation>
        <skos:prefLabel xml:lang="en">[ABB194] Core Data Model</skos:prefLabel>
        <skos:definition xml:lang="en">DESCRIPTION:
A context-neutral data model that captures the fundamental characteristics of an entity or a core set of entities.

Based on Core Vocabularies Handbook
https://joinup.ec.europa.eu/site/core_vocabularies/Core_Vocabularies_user_handbook/

INTEROPERABILITY SALIENCY:
IoP Dimension: Structural IoP, Behavioral IoP, Governance IoP
The Core Data ABB is salient for semantic interoperability because it supports semantic interoperability by providing simplified, reusable and extensible data models that capture the fundamental characteristics of a data entity in a context-neutral and syntax-neutral fashion.

EXAMPLES:
The following implementation is an example on how this specific Architecture Building Block (ABB) can be instantiated as a Solution Building Block (SBB):

ISA2 Core Vocabularies

Core Vocabularies are simplified, re-usable and extensible data models that capture the fundamental characteristics of an entity in a context-neutral fashion.
Public administrations can use and extend the Core Vocabularies in the following contexts:
	Development of new systems: the Core Vocabularies can be used as a default starting point for designing the conceptual and logical data models in newly developed information systems.
	Information exchange between systems: the Core Vocabularies can become the basis of a context-specific data model used to exchange data among existing information systems.
	Data integration: the Core Vocabularies can be used to integrate data that comes from disparate data sources and create a data mash-up.
	Open data publishing: the Core Vocabularies can be used as the foundation of a common export format for data in base registries like cadastres, business registers and service portals.
	ISA has developed the Core Vocabularies for public administrations in an open process with the active involvement of specific working groups. The Core Vocabularies developed are the following:
-	Core Person: captures the fundamental characteristics of a person, e.g. name, gender, date of birth, location.
-	Registered organisation: captures the fundamental characteristics of a legal entity (e.g. its identifier, activities) which is created through a formal registration process, typically in a national or regional register.
-	Core Location: captures the fundamental characteristics of a location, represented as an address, a geographic name or geometry.
-	Core Public service: captures the fundamental characteristics of a service offered by a public administration.
-	Core Criterion and Core Evidence: describe the principles and the means that a private entity must fulfil to become eligible or qualified to perform public services. A Criterion is a rule or a principle that is used to judge, evaluate or test something. An Evidence is a means to prove a Criterion.
-	Core Public organisation: describes public organisations in the European Union.

https://ec.europa.eu/isa2/solutions/core-vocabularies_en</skos:definition>
        <skos:narrower rdf:resource="http://data.europa.eu/dr8/DataModel"/>
    </skos:Concept>

    <skos:Concept rdf:about="http://data.europa.eu/dr8/DataSyntax">
        <skos:notation>DataSyntax</skos:notation>
        <skos:prefLabel xml:lang="en">[ABB231] Data Syntax</skos:prefLabel>
        <skos:definition xml:lang="en">DESCRIPTION:
Data Syntax is a set of rules defining the way in which data is put together with appropriate identifiers, delimiters, separator character(s), and other non-data characters to form messages.

Source: reference: https://www.iso.org/obp/ui/#iso:std:iso:14817:-1:ed-1:v1:en:term:4.59

INTEROPERABILITY SALIENCY:
IoP Dimension: Structural IoP, Behavioral IoP, Governance IoP
The Data Syntax ABB is salient for semantic interoperability because it provides the rules establishing how data have to to be written.

EXAMPLES:
The following implementation is an example on how this specific Architecture Building Block (ABB) can be instantiated as a Solution Building Block (SBB):

XML syntax
XML syntax refers to the rules that determine how an XML application can be written. The XML syntax is very straight forward, and this makes XML very easy to learn. Below are the main points to remember when creating XML documents.
https://www.quackit.com/xml/tutorial/xml_syntax.cfm</skos:definition>
        <skos:narrower rdf:resource="http://data.europa.eu/dr8/SemanticInteroperabilitySpecification"/>
    </skos:Concept>

    <skos:Concept rdf:about="http://data.europa.eu/dr8/DataModel">
        <skos:notation>DataModel</skos:notation>
        <skos:prefLabel xml:lang="en">[ABB26] Data Model</skos:prefLabel>
        <skos:definition xml:lang="en">DESCRIPTION:
A collection of entities, their properties and the relationships among them, which aims at formally representing a domain, a concept or a real-world thing.

Source: ISA2 - SEMIC Action
https://joinup.ec.europa.eu/sites/default/files/methodology_and_tools_for_metadata_governance_and_management_for_eu_institutions.pdf

INTEROPERABILITY SALIENCY:
IoP Dimension: Structural IoP, Behavioral IoP, Governance IoP
The Data Model ABB is salient for semantic interoperability because it ensures compatible interpretations of data exchange as specified in the document &quot;Methodology and tools for metadata governance and management for EU Institutions&quot;, developed under the SEMIC action of the ISA Programme: &quot;Whilst technological developments offer various means to automate the exchange of information, technological developments alone cannot guarantee a greater interoperability between information systems. A fundamental aspect is the need for common data standards: primarily data models and reference data [...]&quot;.

EXAMPLES:
The following implementation is an example on how this specific Architecture Building Block (ABB) can be instantiated as a Solution Building Block (SBB):

ESPD - Exchange data model
The ESPD exchange data model (ESPD-EDM) is used for the ESPD service provided by the European Commission.
The ESPD Exchange Data Model was designed to implement the data requirements expressed in the Annex 2 of the COMMISSION IMPLEMENTING REGULATION (EU) 2016/7 of 5 January 2016 (from now on &quot;the Annex to the Regulation 2016/7&quot;), establishing the standard form for the European Single Document. Additionally to these requirements, the model took also into account the Information Requirements Model specified by the CEN/BII-Workshops.[3] (namely Workshop 3), and the latest developments relating to the Virtual Company Dossier (VCD) in e-Sens.[4].
One premise that has ruled the design and implementation life-cycle of the ESPD-EDM has been &apos;&apos;not to reinvent the wheel&apos;&apos;. Thus some very early key decisions were:

(i)	select a mature business language for the naming, design and implementation of the ESPD-EDM;
(ii)	reuse as much as possible existing information components and libraries &apos;&apos;as-they-are&apos;&apos;;
(iii)	for those entities that are not defined in any standard specification, design new components in such a way that they can be reused in other situations and domains, both in e-Procurement and beyond e-Procurement.

OASIS UBL-2.1 standard was chosen as the best candidate to base the ESPD-EDM upon. The main reasons for this decisions were:
i.	The European Commission is already using (and recommending) UBL-2.1 for e-Documents.[5] ;
ii.	Most of the concepts and components necessary for the ESPD documents were already defined by UBL specifically for e-Procurement; (3) Methodology and tools are available for the development of new documents, the extension of the existing UBL libraries, the semantic validation of XML instances, etc.

https://joinup.ec.europa.eu/release/espd-exchange-data-model-v101</skos:definition>
        <skos:narrower rdf:resource="http://data.europa.eu/dr8/SemanticInteroperabilitySpecification"/>
    </skos:Concept>

    <skos:Concept rdf:about="http://data.europa.eu/dr8/ControlledVocabulary">
        <skos:notation>ControlledVocabulary</skos:notation>
        <skos:prefLabel xml:lang="en">[ABB359] Controlled Vocabulary</skos:prefLabel>
        <skos:definition xml:lang="en">DESCRIPTION:
A controlled vocabulary is an organized arrangement of words and phrases used to index content and/or to retrieve content through browsing or searching. It typically includes preferred and variant terms and has a defined scope or describes a specific domain.

INTEROPERABILITY SALIENCY
IoP Dimension: Structural IoP, Behavioral IoP, Governance IoP
The Data Model ABB is salient for semantic interoperability because it ensures compatible interpretations of words and phrases used to index content and/or to retrieve content through browsing or searching.

EXAMPLES:
The following implementation is an example on how this specific Architecture Building Block (ABB) can be instantiated as a Solution Building Block (SBB):

EuroVoc
EuroVoc is a multilingual, multidisciplinary thesaurus covering the activities of the EU, the European Parliament in particular. It contains terms in 23 EU languages (Bulgarian, Croatian, Czech, Danish, Dutch, English, Estonian, Finnish, French, German, Greek, Hungarian, Italian, Latvian, Lithuanian, Maltese, Polish, Portuguese, Romanian, Slovak, Slovenian, Spanish and Swedish), plus in three languages of countries which are candidates for EU accession:  (mk), shqip (sq) and c (sr).
https://op.europa.eu/en/web/eu-vocabularies/th-dataset/-/resource/dataset/eurovoc</skos:definition>
        <skos:narrower rdf:resource="http://data.europa.eu/dr8/SemanticInteroperabilitySpecification"/>
    </skos:Concept>

    <skos:Concept rdf:about="http://data.europa.eu/dr8/SharedKnowledgeBase">
        <skos:notation>SharedKnowledgeBase</skos:notation>
        <skos:prefLabel xml:lang="en">[ABB366] Shared Knowledge Base</skos:prefLabel>
        <skos:definition xml:lang="en">DESCRIPTION:
A shared Knowledge Base is formed by usable data, information and knowledge resources, with  convergence power, in relation to public policy goals attainment, given by their impact in the enactment of common understanding from the existing organisational information, across the levels of a public administration (central, regional, local) towards the achievement of the public policy goals, enabling :
i)	structural interoperability by semantic resources supporting reusing and/or sharing of data, information and knowledge (i.e. data set catalogue enabling provisioning/consuming data, information and knowledge cross public administrations and cross borders);
ii)	behavioural interoperability by semantic resources supporting exchanging capabilities of data, information or knowledge with internal/external peers (i.e. Metadata mappings enabling that data/information/knowledge be provisioned/consumed cross public administrations and cross borders); and
iii)	governance interoperability by semantic resources supporting the collaboration with internal/external peers exchanging data, information or knowledge (i.e. Sematic Interoperability Agreements on interpretations enabling sharing, reuse and exchange of data/information/knowledge cross public administrations and cross borders).

INTEROPERABILITY SALIENCY:
IoP Dimension: Structural IoP, Behavioral IoP, Governance IoP
This ABB is a key interoperability enabler because it supports to achieve semantic interoperability with public policy goals convergence value by  all in all enabling i) the provision/consumption of  data by public services,  ii) the exchange of data, information, and knowledge between digital public services, and iii) collaboration between digital public services</skos:definition>
        <skos:topConceptOf rdf:resource="http://data.europa.eu/dr8"/>
    </skos:Concept>

    <skos:Concept rdf:about="http://data.europa.eu/dr8/DataMapping">
        <skos:notation>DataMapping</skos:notation>
        <skos:prefLabel xml:lang="en">[ABB360] Data mapping</skos:prefLabel>
        <skos:definition xml:lang="en">DESCRIPTION:
Data mapping is an equivalence relationship between two data items with ontological value. Data mapping is used for a wide variety of tasks, including:
- Data mediation between a data source and a destination;
- Data transformation
- Identification of data relationships as part of data lineage analysis;
- Discovery of hidden sensitive data such as the last four digits of a social security number hidden in another user id as part of a data masking or de-identification project;
- Consolidation of multiple databases into a single database and identifying redundant columns of data for consolidation or elimination.

INTEROPERABILITY SALIENCY
IoP Dimension: Behavioral  IoP
The Data Mapping ABB is a key interoperability enabler because it supports to achieve legal behavioral interoperability by   enabling the exchange of data, information, and knowledge between digital public services.

EXAMPLE
The following implementation is an example on how this specific Architecture Building Block (ABB) can be instantiated as a Solution Building Block (SBB):

Microsoft Dynamics CRM Mapping Schema:
Microsoft Dynamics CRM contains several data sets which comprise of different objects, such as Leads, Opportunities, and Competitors. Each of these data sets has several fields like Name, Account Owner, City, Country, Job Title, and more. The application has a defined schema along with attributes, enumerations, and mapping rules. Therefore, if a new record is to be added to the schema of a data object, a data map needs to be created from the data source to the Microsoft Dynamics CRM account.</skos:definition>
        <skos:topConceptOf rdf:resource="http://data.europa.eu/dr8"/>
    </skos:Concept>

    <skos:Concept rdf:about="http://data.europa.eu/dr8/OntologiesCatalogue">
        <skos:notation>OntologiesCatalogue</skos:notation>
        <skos:prefLabel xml:lang="en">[ABB365] Ontologies Catalogue</skos:prefLabel>
        <skos:definition xml:lang="en">DESCRIPTION:
Indexed inventory of ontologies with comprehensiveness and trustiness value.
This ABB is a key interoperability enabler (*) for sharing/PROVISIONING and reusing/CONSUMING Data.

INTEROPERABILITY SALIENCY:
IoP Dimension: Structural IoP
The Ontologies catalogue  ABB is a key interoperability enabler because it supports to achieve semantic structural interoperability by ensuring the provision/consumption of  ontologies by digital public services.

EXAMPLE:
The following implementation is an example on how this specific Architecture Building Block (ABB) can be instantiated as a Solution Building Block (SBB):
BioPortal
BioPortal is a repository of over 300 biomedical ontologies and includes tools for working with these ontologies. Holds most widely used Biomedical ontologies. Allows ontologies to be browsed, searched, and reviewed. Allows uses to create notes on ontologies terms. Allows arbitrary text to be annotated with ontology terms. Also supports search of biomedical resources (e.g. PubMed) for combinations of terms from ontologies. Allows programmatic access to ontologies through a REST interface.
http://bioportal.bioontology.org/</skos:definition>
        <skos:topConceptOf rdf:resource="http://data.europa.eu/dr8"/>
    </skos:Concept>

    <skos:Concept rdf:about="http://data.europa.eu/dr8/Ontology">
        <skos:notation>Ontology</skos:notation>
        <skos:prefLabel xml:lang="en">[ABB364] Ontology</skos:prefLabel>
        <skos:definition xml:lang="en">DESCRIPTION:
An Ontology is a formal description of knowledge as a set of concepts within a domain and the axioms connecting concepts and allowing for logic inferences. When speaking about an ontology, we do not refer only to the terminology (or T-Box) but also to all the assertions about the concepts and roles (the A-Box), i.e. all the individuals or instances of concepts and roles of the terminology and as important, the rules for logic inference: the semantics part.

INTEROPERABILITY SALIENCY:
IoP Dimension: Governance IoP
The Ontologies ABB is salient for semantic interoperability because it defined as a simplified, reusable and extensible data model that capture the fundamental characteristics of a data entity in a context-neutral and syntax-neutral fashion.

EXAMPLE:
The following implementation is an example on how this specific Architecture Building Block (ABB) can be instantiated as a Solution Building Block (SBB):
Medical Dictionary for Regulatory Activities Terminology (MedDRA)
The university ontology includes classes, e.g., :Staff, :Students, :Department or :Course. These classes denote natural concepts that are shared or at least understood by users familiar with universities all over the world.
Universities ontologies can be view in university portals.
http://bioportal.bioontology.org/ontologies/MEDDRA</skos:definition>
        <skos:topConceptOf rdf:resource="http://data.europa.eu/dr8"/>
    </skos:Concept>

    <skos:Concept rdf:about="http://data.europa.eu/dr8/DataOwner">
        <skos:notation>DataOwner</skos:notation>
        <skos:prefLabel xml:lang="en">[ABB361] Data Owner</skos:prefLabel>
        <skos:definition xml:lang="en">DESCRIPTION:
Data owners are either individuals or teams who make decisions such as who has the right to access and edit data and how its used. Owners may not work with their data every day, but are responsible for overseeing and protecting a data domain.
In the context of the GDPR, data owners are accountable for the quality, integrity, and protection of their data space.

INTEROPERABILITY SALIENCY:
IoP Dimension: Mainly Behavioural IoP
The Data Owner ABB is salient for organisational interoperability because it is responsible for the management of the data generated or consumed by the public service. The identification of Data Owners, as stated in the GDPR, is important for accountabilty since it clearly identifies a person/team repsonible to control the compliance of data, and for the defintiion of policies and standards for the alignment of public service data to GDPR.

EXAMPLE:
Uprava Subsidized Ticket for Students:
Slovenian portal eGovernment is the main point for e-services for citizens.
Students can buy subsidized tickets electronically on the eGovernment portal &quot;eUprava&quot;).
Data Owner - Ministry of Interior
The Ministry of Interior is the owner of the personal data from Central Population register.
https://e-uprava.gov.si/podrocja/izobrazevanje-kultura/visoka-in-visja-sola/subvencionirana-vozovnica.html</skos:definition>
        <skos:topConceptOf rdf:resource="http://data.europa.eu/dr8"/>
    </skos:Concept>

    <skos:Concept rdf:about="http://data.europa.eu/dr8/SemanticInteroperabilityAgreement">
        <skos:notation>SemanticInteroperabilityAgreement</skos:notation>
        <skos:prefLabel xml:lang="en">[ABB232] Semantic Interoperability Agreement</skos:prefLabel>
        <skos:definition xml:lang="en">DESCRIPTION:
A Semantic interoperability agreement is a semantic  resource formalizing governance rules enabling collaboration between digital public services with ontological value.

Source:
https://joinup.ec.europa.eu/sites/default/files/document/2015-03/Process

INTEROPERABILITY SALIENCY:
IoP Dimension: Governance IoP
The Semantic Interoperability Agreement ABB  is a key interoperability enabler because it supports semantic governance interoperability by enabling collaboration between digital public services.

EXAMPLES:
The following implementation is an example on how this specific Architecture Building Block (ABB) can be instantiated as a Solution Building Block (SBB):

e-Invoicing Semantic Data Model
The semantic data model includes only the essential information elements that an electronic invoice needs to ensure legal (including fiscal) compliance and to enable interoperability for cross-border, cross-sector and for domestic trade. The semantic data model may be used by public and private sector organisations for public procurement invoicing and took into account the physical and financial supply chain perspective, reflecting both private and public sector requirements, with a view to allowing the full straight-through processing of an electronic invoice.
https://ec.europa.eu/cefdigital/wiki/display/CEFDIGITAL/2017/06/28/CEN+Publishes+eInvoicing+Semantic+Data+Model</skos:definition>
        <skos:topConceptOf rdf:resource="http://data.europa.eu/dr8"/>
    </skos:Concept>

    <skos:Concept rdf:about="http://data.europa.eu/dr8/DataMapping">
        <skos:notation>DataMapping</skos:notation>
        <skos:prefLabel xml:lang="en">[ABB375] Data mapping</skos:prefLabel>
        <skos:definition xml:lang="en">DESCRIPTION:
Data mapping is an equivalence relationship between two data items with ontological value. Data mapping is used for a wide variety of tasks, including:
- Data mediation between a data source and a destination;
- Data transformation
- Identification of data relationships as part of data lineage analysis;
- Discovery of hidden sensitive data such as the last four digits of a social security number hidden in another user id as part of a data masking or de-identification project;
- Consolidation of multiple databases into a single database and identifying redundant columns of data for consolidation or elimination.

INTEROPERABILITY SALIENCY
IoP Dimension: Behavioral  IoP
The Data Mapping ABB is a key interoperability enabler because it supports to achieve legal behavioral interoperability by enabling the exchange of data, information, and knowledge between digital public services.

EXAMPLE
The following implementation is an example on how this specific Architecture Building Block (ABB) can be instantiated as a Solution Building Block (SBB):

Microsoft Dynamics CRM Mapping Schema:
Microsoft Dynamics CRM contains several data sets which comprise of different objects, such as Leads, Opportunities, and Competitors. Each of these data sets has several fields like Name, Account Owner, City, Country, Job Title, and more. The application has a defined schema along with attributes, enumerations, and mapping rules. Therefore, if a new record is to be added to the schema of a data object, a data map needs to be created from the data source to the Microsoft Dynamics CRM account.</skos:definition>
        <skos:narrower rdf:resource="http://data.europa.eu/dr8/DataMapping"/>
    </skos:Concept>

    <skos:Concept rdf:about="http://data.europa.eu/dr8/DataMappingCatalogue">
        <skos:notation>DataMappingCatalogue</skos:notation>
        <skos:prefLabel xml:lang="en">[ABB376] Data Mapping Catalogue</skos:prefLabel>
        <skos:definition xml:lang="en">DESCRIPTION:
Indexed inventory of data mappings with comprehensiveness and trustiness value.
This ABB is a key interoperability enabler (*) for sharing/PROVISIONING and reusing/CONSUMING Data.

INTEROPERABILITY SALIENCY:


EXAMPLE:
CEMS Rapid Mapping - JRC
The Joint Research Centre (JRC) is the European Commission&apos;s science and knowledge service which employs scientists to carry out research in order to provide independent scientific advice and support to EU policy.
Rapid Mapping is one of the two on-demand mapping services under the Copernicus Emergency Management Service (CEMS). Rapid Mapping delivers geospatial information (in different vector and raster formats) in the midst of or immediately after catastrophic events or humanitarian crises. It is available 24/7/365. Supported disaster types range from natural hazards such as floods, fires, storms, tsunamis, volcanic eruptions, landslides, and earthquakes to industrial accidents and humanitarian crises.

https://data.jrc.ec.europa.eu/collection/id-0072</skos:definition>
        <skos:topConceptOf rdf:resource="http://data.europa.eu/dr8"/>
    </skos:Concept>

    <skos:Concept rdf:about="http://data.europa.eu/dr8/SemanticAgreement">
        <skos:notation>SemanticAgreement</skos:notation>
        <skos:prefLabel xml:lang="en">[ABB374] Semantic Agreement</skos:prefLabel>
        <skos:definition xml:lang="en">DESCRIPTION:
An agreement from a peer to the common ontology is the result of a matching or mapping process that is used to resolve their semantic discrepancies. The combination matching process consists of linguistic base, internal and external structure comparison. Result of matching combination will be used to develop agreement unit as component of agreement. There are some assumptions for the agreement, such as using same language to representation of schema/ontology, labels represent the meaning of concept, and there is no individual at the common ontology.

Source: Work Group Information System
http://ftp.gunadarma.ac.id/research/WorkGroupInformationSystem/ThesisPersonal/Thesis_IWayan_Final/MainThesisIWS/node78.html

INTEROPERABILITY SALIENCY:
Not applicable

EXAMPLES:
The following implementation is an example on how this specific Architecture Building Block (ABB) can be instantiated as a Solution Building Block (SBB):

SEMIC
&quot;Supporting alignments and agreements on common definitions and specifications at the semantic layer for the Member States and the EU institutions&quot;.
https://joinup.ec.europa.eu/collection/semantic-interoperability-community-semic/about</skos:definition>
        <skos:topConceptOf rdf:resource="http://data.europa.eu/dr8"/>
    </skos:Concept>

    <skos:Concept rdf:about="http://data.europa.eu/dr8/SecurityPolicy">
        <skos:notation>SecurityPolicy</skos:notation>
        <skos:prefLabel xml:lang="en">[ABB372] Security Policy</skos:prefLabel>
        <skos:definition xml:lang="en">DESCRIPTION:
A privacy or security policy is a statement or a legal document (in privacy law) that discloses some or all of the ways a party gathers, uses, discloses, and manages a customer or client&apos;s data.

INTEROPERABILITY SALIENCY:
IoP Dimension: Governance IoP
The Data Policy ABB is salient for semantic interoperability because it provides a guiding framework to ensure the security of data and information according to interoperability principles as stated in the EIF recommendation n 46 and 47: &quot;Consider the specific security and privacy requirements and identify measures for the provision of each public service according to risk management plans.&quot;

EXAMPLE:
The following implementation is an example on how this specific Architecture Building Block (ABB) can be instantiated as a Solution Building Block (SBB):

Common Foreign and Security Policy (CFSP)
The Common Foreign and Security Policy (CFSP) is the organised, agreed foreign policy of the European Union (EU) for mainly security and defence diplomacy and actions.
https://eeas.europa.eu/topics/common-foreign-security-policy-cfsp_en</skos:definition>
        <skos:topConceptOf rdf:resource="http://data.europa.eu/dr8"/>
    </skos:Concept>

    <skos:Concept rdf:about="http://data.europa.eu/dr8/PrivacyPolicy">
        <skos:notation>PrivacyPolicy</skos:notation>
        <skos:prefLabel xml:lang="en">[ABB373] Privacy Policy</skos:prefLabel>
        <skos:definition xml:lang="en">DESCRIPTION:
A privacy policy is a document that explains how an organization handles any customer, client or employee information gathered in its operations.

Source: Techtarget
https://whatis.techtarget.com/definition/privacy-policy

INTEROPERABILITY SALIENCY:
IoP Dimension: Governance IoP
The Data Policy ABB is salient for semantic interoperability because it provides a guiding framework to ensure the privacy of data and information according to interoperability principles as stated in the EIF recommendation n 46 and 47: &quot;Consider the specific security and privacy requirements and identify measures for the provision of each public service according to risk management plans.&quot;

EXAMPLES:
The following implementation is an example on how this specific Architecture Building Block (ABB) can be instantiated as a Solution Building Block (SBB):

Protection of individuals with regard to the processing of personal data
&quot;The policy on protection of individuals with regard to the processing of personal data by the European Union institutions is based on the Regulation (EU) 2018/1725 on the protection of personal data by the EU institutions, bodies, offices and agencies&quot;. https://ec.europa.eu/info/privacy-policy_en</skos:definition>
        <skos:topConceptOf rdf:resource="http://data.europa.eu/dr8"/>
    </skos:Concept>

    <skos:Collection rdf:about="http://data.europa.eu/dr8/view/TechnicalView-Application">
        <skos:notation>TechnicalView-Application</skos:notation>
        <skos:prefLabel xml:lang="en">Technical View - Application</skos:prefLabel>
        <skos:member rdf:resource="http://data.europa.eu/dr8/MachineToMachineInterface"/>
        <skos:member rdf:resource="http://data.europa.eu/dr8/HumanInterface"/>
        <skos:member rdf:resource="http://data.europa.eu/dr8/InteroperableEuropeanSolutionService"/>
        <skos:member rdf:resource="http://data.europa.eu/dr8/InteroperableEuropeanSolutionComponent"/>
        <skos:member rdf:resource="http://data.europa.eu/dr8/AccessManagementService"/>
        <skos:member rdf:resource="http://data.europa.eu/dr8/AccessManagementComponent"/>
        <skos:member rdf:resource="http://data.europa.eu/dr8/AuditService"/>
        <skos:member rdf:resource="http://data.europa.eu/dr8/AuditComponent"/>
        <skos:member rdf:resource="http://data.europa.eu/dr8/InteroperableEuropeanSolution"/>
        <skos:member rdf:resource="http://data.europa.eu/dr8/DataTransformationService"/>
        <skos:member rdf:resource="http://data.europa.eu/dr8/DataTransformationComponent"/>
        <skos:member rdf:resource="http://data.europa.eu/dr8/DataValidationService"/>
        <skos:member rdf:resource="http://data.europa.eu/dr8/DataValidationComponent"/>
        <skos:member rdf:resource="http://data.europa.eu/dr8/ServiceDiscoveryService"/>
        <skos:member rdf:resource="http://data.europa.eu/dr8/ServiceDiscoveryComponent"/>
        <skos:member rdf:resource="http://data.europa.eu/dr8/OrchestrationService"/>
        <skos:member rdf:resource="http://data.europa.eu/dr8/OrchestrationComponent"/>
        <skos:member rdf:resource="http://data.europa.eu/dr8/TechnicalSpecification"/>
        <skos:member rdf:resource="http://data.europa.eu/dr8/TechnicalInteroperabilityAgreement"/>
        <skos:member rdf:resource="http://data.europa.eu/dr8/SharedPlatform"/>
        <skos:member rdf:resource="http://data.europa.eu/dr8/ConformanceTestingService"/>
        <skos:member rdf:resource="http://data.europa.eu/dr8/ConformanceTestingComponent"/>
        <skos:member rdf:resource="http://data.europa.eu/dr8/ConformanceTestReport"/>
        <skos:member rdf:resource="http://data.europa.eu/dr8/ConformanceTestScenario"/>
        <skos:member rdf:resource="http://data.europa.eu/dr8/TechnicalAgreement"/>
    </skos:Collection>

    <skos:Concept rdf:about="http://data.europa.eu/dr8/MachineToMachineInterface">
        <skos:notation>MachineToMachineInterface</skos:notation>
        <skos:prefLabel xml:lang="en">[ABB38] Machine to Machine Interface</skos:prefLabel>
        <skos:definition xml:lang="en">DESCRIPTION:
A boundary set of means enabling the exchange of data between a service and other services.
This ABB is a key interoperability enabler (*) for assessing compatible interfaces.

Source: ISA2 - EIA Action

(*)DECISION (EU) 2015/2240 OF THE EUROPEAN PARLIAMENT AND OF THE COUNCIL of 25 November 2015 establishing a programme on interoperability solutions and common frameworks for European public administrations, businesses and citizens (ISA2 programme) as a means for modernising the public sector.

INTEROPERABILITY SALIENCY:
IoP Dimension: Behavioral IoP
The Machine to machine interface ABB  is a key interoperability enabler because it supports to achieve technical behavioral interoperability by   enabling the exchange of data, information, and knowledge between digital public services as stated in the EIF recommendation n5: &quot;&quot;Ensure internal visibility and provide external interfaces for European public services&quot; and recommendation n9:&quot;Ensure data portability, namely that data is easily transferable between systems and applications supporting the implementation and evolution of European public services without unjustified restrictions, if legally possible.&quot;


EXAMPLES:
The following implementation is an example on how this specific Architecture Building Block (ABB) can be instantiated as a Solution Building Block (SBB):

XMLGate TRACES Businesses (XTB)
Webservices enabling the management of organisations and cities registered in TRACES.
https://circabc.europa.eu/sd/a/dc77e52b-dfba-4dcc-aa39-6a54748db01d/XmlGate%20TRACES%20Businesses%20Manual.doc

In addition, the European Commission has publiched a study, called APIs4DGov, on Web Application Programming interfaces (APIs). The study identifies and describes a set of API standards and technical specification which can be used for Machine to Machine interfaces, as an example:

Advanced Message Queuing Protocol (AMQP);
Application Performance Index (APDEX);
HAL-FORMS.

The study lists 80 APIs standards, which can be consulted at the following link: https://ec.europa.eu/knowledge4policy/node/35863_el</skos:definition>
        <skos:topConceptOf rdf:resource="http://data.europa.eu/dr8"/>
    </skos:Concept>

    <skos:Concept rdf:about="http://data.europa.eu/dr8/HumanInterface">
        <skos:notation>HumanInterface</skos:notation>
        <skos:prefLabel xml:lang="en">[ABB37] Human Interface</skos:prefLabel>
        <skos:definition xml:lang="en">DESCRIPTION:
A boundary set of means enabling the exchange of data between an individual and a service.
This ABB is a key interoperability enabler (*) for assessing compatible interfaces.

Source: ISA2 - EIA Action

(*)DECISION (EU) 2015/2240 OF THE EUROPEAN PARLIAMENT AND OF THE COUNCIL of 25 November 2015 establishing a programme on interoperability solutions and common frameworks for European public administrations, businesses and citizens (ISA2 programme) as a means for modernising the public sector.

Syn. User interface, UI, Graphical User Interface, GUI

INTEROPERABILITY SALIENCY:
IoP Dimension: Behavioral IoP
The Human interface ABB  is a key interoperability enabler because it supports to achieve technical behavioral interoperability by   enabling the exchange of data, information, and knowledge between digital public services and individuals.

EXAMPLES:
The following implementation is an example on how this specific Architecture Building Block (ABB) can be instantiated as a Solution Building Block (SBB):

GrapesJS
GrapesJS is an open-source, multi-purpose, Web Builder Framework which combines different tools and features with the goal to help you (or users of your application) to build HTML templates without any knowledge of coding. It&apos;s a perfect solution to replace the common WYSIWYG editors, which are good for content editing but inappropriate for creating HTML structures. You can see it in action with the official demos, but using its API you&apos;re able to build your own editors.
https://grapesjs.com/</skos:definition>
        <skos:topConceptOf rdf:resource="http://data.europa.eu/dr8"/>
    </skos:Concept>

    <skos:Concept rdf:about="http://data.europa.eu/dr8/InteroperableEuropeanSolutionService">
        <skos:notation>InteroperableEuropeanSolutionService</skos:notation>
        <skos:prefLabel xml:lang="en">[ABB187] Interoperable European Solution Service</skos:prefLabel>
        <skos:definition xml:lang="en">DESCRIPTION:
Represents an explicitly defined shared application behavior of an Inteoperable European Solution.

Based on ArchiMate v3
http://pubs.opengroup.org/architecture/archimate3-doc/chap09.html

INTEROPERABILITY SALIENCY:
IoP Dimension: Behavioral IoP
The Interoperable European Solution service ABB is salient for technical interoperability because it is a central element the EIF&apos;s conceptual model for integrated public services. it represents the generalisation of all application services provided by an Interoperable European Solutionas as stated in the EIF: &quot;Technical interoperability the applications and infrastructures linking systems and services.&quot;

EXAMPLES:
The following implementation is an example on how this specific Architecture Building Block (ABB) can be instantiated as a Solution Building Block (SBB):

EU Login
EU Login is the European Commission&apos;s user authentication service. It allows authorised users to access a wide range of Commission web services and websites, using a single email address and password. EU Login implements the single sign-on functionality.
https://webgate.ec.europa.eu/cas/help.html</skos:definition>
        <skos:topConceptOf rdf:resource="http://data.europa.eu/dr8"/>
    </skos:Concept>

    <skos:Concept rdf:about="http://data.europa.eu/dr8/InteroperableEuropeanSolutionComponent">
        <skos:notation>InteroperableEuropeanSolutionComponent</skos:notation>
        <skos:prefLabel xml:lang="en">[ABB233] Interoperable European Solution Component</skos:prefLabel>
        <skos:definition xml:lang="en">DESCRIPTION:
Interoperable European Solution Component represents the encapsulation of a functionality provided by an Interoperable European Solution.

Based on ArchiMate v3
http://pubs.opengroup.org/architecture/archimate3-doc/chap09.html

INTEROPERABILITY SALIENCY:
IoP Dimension: Structural IoP
The Interoperable European Solution Component ABB is salient for technical interoperability because it is a central element the EIF&apos;s conceptual model for integrated public services. it represents all the functionalities provided by an Interoperable European Solutionas as stated in the EIF: &quot;Technical interoperability the applications and infrastructures linking systems and services.&quot;

EXAMPLES:
The following implementation is an example on how this specific Architecture Building Block (ABB) can be instantiated as a Solution Building Block (SBB):

EU Login
EU Login is the European Commission&apos;s user authentication service. It allows authorised users to access a wide range of Commission web services and websites, using a single email address and password. EU Login implements the single sign-on functionality.
https://webgate.ec.europa.eu/cas/help.html</skos:definition>
        <skos:topConceptOf rdf:resource="http://data.europa.eu/dr8"/>
    </skos:Concept>

    <skos:Concept rdf:about="http://data.europa.eu/dr8/AccessManagementService">
        <skos:notation>AccessManagementService</skos:notation>
        <skos:prefLabel xml:lang="en">[ABB57] Access Management Service</skos:prefLabel>
        <skos:definition xml:lang="en">DESCRIPTION:
Shares  the functionality of allowing users to make use of i) IT services, ii) data, and/or iii) other assets. Access management helps to protect the confidentiality, integrity and availability of assets by ensuring that only authorized users are able to access or modify the assets.

Based on ITIL v3
https://www.axelos.com/Corporate/media/Files/Glossaries/AXELOS-Common-Glossary.pdf

Syn. Role Management Service

INTEROPERABILITY SALIENCY:
IoP Dimension: Behavioral IoP
The Access Management Service ABB is salient for technical interoperability because it provides the functionality of allowing user to make an authorized  and trusted use of IT Services, data and other assets as stated in the EIF: &quot;Public administrations should ensure that a &apos;data access and authorisation plan which determines who has access to what data and under what conditions, to ensure privacy. Unauthorised access and security breaches should be monitored and appropriate actions should be taken to prevent any recurrence of breaches&quot;

EXAMPLES:
The following implementation is an example on how this specific Architecture Building Block (ABB) can be instantiated as a Solution Building Block (SBB):

Belgian Federal Public Service Policy and Support - Role Management service
The Role Management service gives access managers the possibility to manage roles. A role gives access to an online government application.

Characteristics:
	A federal access management platform for public e-gov applications
	Three separate contexts: Businesses, Officials and Independent
	Roles that can only be attributed by a specific group of managers for a specific application within one of the three contexts
	Two different security levels of the application depending on the sensitivity of the information: user name, password and token; and electronic identity card with associated PIN code
	Authentication when connecting to an application
	Support with the implementation of the service
	Support while the service is being used

Users: All public services and institutions that want a secure access management for their applications: federal public services and institutions; Communities and Regions; Provinces, municipalities and local public social welfare centres; businesses or persons implementing government contracts.
Requirements: application with Fedict Service Desk and signing up to a user agreement.
http://www.fedict.belgium.be/en/identificatie_beveiliging/rollenbeheer</skos:definition>
        <skos:topConceptOf rdf:resource="http://data.europa.eu/dr8"/>
    </skos:Concept>

    <skos:Concept rdf:about="http://data.europa.eu/dr8/AccessManagementComponent">
        <skos:notation>AccessManagementComponent</skos:notation>
        <skos:prefLabel xml:lang="en">[ABB70] Access Management Component</skos:prefLabel>
        <skos:definition xml:lang="en">DESCRIPTION:
Implements the functionalities of allowing users to make use of i) IT services, ii) data, and/or iii) other assets. Access management helps to protect the confidentiality, integrity and availability of assets by ensuring that only authorised users are able to access or modify the assets.

Based on ITIL v3
https://www.axelos.com/Corporate/media/Files/Glossaries/AXELOS-Common-Glossary.pdf

INTEROPERABILITY SALIENCY:
IoP Dimension: Structural IoP
The Access Management Component ABB is salient for technical interoperability because it provides the implementation the functionality of allowing user to make an authorized  and trusted use of IT Services, data and other assets as stated in the EIF: &quot;Public administrations should ensure that a &apos;data access and authorisation plan which determines who has access to what data and under what conditions, to ensure privacy. Unauthorised access and security breaches should be monitored and appropriate actions should be taken to prevent any recurrence of breaches&quot;

EXAMPLES:
The following implementation is an example on how this specific Architecture Building Block (ABB) can be instantiated as a Solution Building Block (SBB):

OpenIAM Access Manager
OpenIAM Access Management solution is based on a professional open source model. This is a robust, scalable solution built with Service Oriented Architecture. It integrates seamlessly with the OpenIAM Identity Manager product to provide a comprehensive solution that allows to take control of not only who can access the systems, but what they can do once they are in there. Corporate security policy is enforced across multiple points and managed centrally to improve effectiveness and reduce administrative costs.
http://www.openiam.com/products/access-manager/overview/</skos:definition>
        <skos:topConceptOf rdf:resource="http://data.europa.eu/dr8"/>
    </skos:Concept>

    <skos:Concept rdf:about="http://data.europa.eu/dr8/AuditService">
        <skos:notation>AuditService</skos:notation>
        <skos:prefLabel xml:lang="en">[ABB58] Audit Service</skos:prefLabel>
        <skos:definition xml:lang="en">DESCRIPTION:
Shares the audit functionality of providing support for the principle of accountability, which is holding users of a system accountable for their actions within the system, and detection of policy violations. The audit policy defines the elements of an information system which need to be traced, for example to assure traceability of actions: what, how, when, where and with what.

Based on The Open Group
http://www.opengroup.org/security/das/xdas_int.htm

INTEROPERABILITY SALIENCY:
IoP Dimension: Behavioral IoP
The Audit Service ABB is salient for technical interoperability because it defines the elements of an information system which need to be traced, for example to assure traceability of user actions as stated in the EIF: &quot;Public administrations should ensure that a &apos;data access and authorisation plan which determines who has access to what data and under what conditions, to ensure privacy. Unauthorised access and security breaches should be monitored and appropriate actions should be taken to prevent any recurrence of breaches&quot;

EXAMPLES:
The following implementation is an example on how this specific Architecture Building Block (ABB) can be instantiated as a Solution Building Block (SBB):

OpenIAM audit service
OpenIAM Auditing Service ensures that detailed information about events and activities associated with identities or resources are logged into a centralized repository and be tracked. It offers the following features:

	Sign-on, Sign-off
	User: create, update, delete or disable accounts
	Role: create, update, delete or disable accounts
	Resource: create, update, delete or disable accounts
	Password changes, resets, challenge response questions changes
	Synchronization events
	Reconciliation events

Several reporting templates are provided for a BIRT report writer for use in an Eclipse designer. Organizations can also generate their own reports in BIRT with SQL.
https://www.openiam.com/products/identity-manager/features/audit-compliance/</skos:definition>
        <skos:topConceptOf rdf:resource="http://data.europa.eu/dr8"/>
    </skos:Concept>

    <skos:Concept rdf:about="http://data.europa.eu/dr8/AuditComponent">
        <skos:notation>AuditComponent</skos:notation>
        <skos:prefLabel xml:lang="en">[ABB71] Audit Component</skos:prefLabel>
        <skos:definition xml:lang="en">DESCRIPTION:
Implements the functionality of providing support for the principle of accountability, which is holding users of a system accountable for their actions within the system, and detection of policy violations. The audit policy defines the elements of an information system which need to be traced, for example to assure traceability of actions: what, how, when, where and with what.

Based on The Open Group
http://www.opengroup.org/security/das/xdas_int.htm

INTEROPERABILITY SALIENCY:
IoP Dimension: Structural IoP
The Audit Component ABB is salient for technical interoperability because it allows the implementation of audit policies as stated in the EIF: &quot;Public administrations should ensure that a &apos;data access and authorisation plan which determines who has access to what data and under what conditions, to ensure privacy. Unauthorised access and security breaches should be monitored and appropriate actions should be taken to prevent any recurrence of breaches&quot;

EXAMPLES:
The following implementation is an example on how this specific Architecture Building Block (ABB) can be instantiated as a Solution Building Block (SBB):

Activiti audit feature
The audit feature of Activiti archives all process instances, activity instances, keeps variable values continuously in sync and all form properties that are submitted so that all user interaction through forms is traceable and can be audited.
Authenticated users who submitted the forms are accessible in the history as well as for start forms and task forms.
https://www.activiti.org/userguide/#historyFormAuditPurposes</skos:definition>
        <skos:topConceptOf rdf:resource="http://data.europa.eu/dr8"/>
    </skos:Concept>

    <skos:Concept rdf:about="http://data.europa.eu/dr8/InteroperableEuropeanSolution">
        <skos:notation>InteroperableEuropeanSolution</skos:notation>
        <skos:prefLabel xml:lang="en">[ABB60] Interoperable European Solution</skos:prefLabel>
        <skos:definition xml:lang="en">DESCRIPTION:
A solution, developed by Public Administrations that facilitate the delivery of electronic Public Services and cross-border exchange of information between Public Administrations (or Citizens) in support to the implementation and advancement of EU, national or local Public Policies.

Based on ISA TES definition
https://joinup.ec.europa.eu/node/149889

IoP Dimension: Structural IoP, Behavioral IoP

EXAMPLES:
The following implementation is an example on how this specific Architecture Building Block (ABB) can be instantiated as a Solution Building Block (SBB):

eDelivery
Supporting secure and reliable exchange of data and documents
eDelivery is a network of nodes for digital communications. It is based on a distributed model where every participant becomes a node using standard transport protocols and security policies. eDelivery helps public administrations to exchange electronic data and documents with other public administrations, businesses and citizens, in an interoperable, secure, reliable and trusted way. eDelivery is one of the building blocks of the European Commission&apos;s Connecting Europe Facility (CEF). These building blocks are reusable specifications, software and services that will form part of a wide variety of IT systems in different policy domains of the EU. The CEF eDelivery building block is based on the AS4 messaging protocol, open and free for all, developed by the OASIS standards development organisation. To ease its adoption in Europe, eDelivery uses the AS4 implementation guidelines defined by the Member States in the e-SENS Large Scale Pilot. Organisations must install an Access Point, or use a Service Provider, to exchange information with the AS4 messaging protocol.
https://ec.europa.eu/cefdigital/wiki/display/CEFDIGITAL/eDelivery</skos:definition>
        <skos:topConceptOf rdf:resource="http://data.europa.eu/dr8"/>
    </skos:Concept>

    <skos:Concept rdf:about="http://data.europa.eu/dr8/DataTransformationService">
        <skos:notation>DataTransformationService</skos:notation>
        <skos:prefLabel xml:lang="en">[ABB40] Data Transformation Service</skos:prefLabel>
        <skos:definition xml:lang="en">DESCRIPTION:
Shares the functionality of conversion of one data representation to another.

Source: ISA2  EIA Action

INTEROPERABILITY SALIENCY:
IoP Dimension: Behavioral IoP
The Data Transformation Service ABB is salient for technical interoperability  because it provides the functionalities to transform internal data structures to common and agreed interoperable formats as stated in the EIF recommendation n 41: &quot;Establish procedures and processes to integrate the opening of data in your common business processes, working routines, and in the development of new information systems.&quot;

EXAMPLES:
The following implementation is an example on how this specific Architecture Building Block (ABB) can be instantiated as a Solution Building Block (SBB):

Eurostat transformation service
The transformation service allows datasets to be converted from one file format to another, optionally performing additional tasks, such as mapping and transcoding.
The service is operational but is currently only available for internal consumption within Eurostat. However, the source code of both web service and software component is available in the SDMX webspace:
http://ec.europa.eu/eurostat/web/sdmx-infospace/validation-transformation/transformation-services</skos:definition>
        <skos:topConceptOf rdf:resource="http://data.europa.eu/dr8"/>
    </skos:Concept>

    <skos:Concept rdf:about="http://data.europa.eu/dr8/DataTransformationComponent">
        <skos:notation>DataTransformationComponent</skos:notation>
        <skos:prefLabel xml:lang="en">[ABB61] Data Transformation Component</skos:prefLabel>
        <skos:definition xml:lang="en">DESCRIPTION:
Implements the functionality of conversion of data from one data representation to another.

Source: ISA2  EIA Action

INTEROPERABILITY SALIENCY:
IoP Dimension: Structural IoP
The Data Transformation Component ABB is salient for technical interoperability  because it enables the implementation of the functionalities to transform internal data structures to common and agreed interoperable formats as stated in the EIF recommendation n 41: &quot;Establish procedures and processes to integrate the opening of data in your common business processes, working routines, and in the development of new information systems.&quot;

EXAMPLES:
The following implementation is an example on how this specific Architecture Building Block (ABB) can be instantiated as a Solution Building Block (SBB):

Eurostat SDMX converter
Eurostat SDMX converter
The SDMX Converter is a tool that converts statistical datasets between different formats. It is a Java application which is actively developed by Eurostat and is published as open source software.
http://ec.europa.eu/eurostat/web/sdmx-infospace/sdmx-it-tools/sdmx-converter</skos:definition>
        <skos:topConceptOf rdf:resource="http://data.europa.eu/dr8"/>
    </skos:Concept>

    <skos:Concept rdf:about="http://data.europa.eu/dr8/DataValidationService">
        <skos:notation>DataValidationService</skos:notation>
        <skos:prefLabel xml:lang="en">[ABB42] Data Validation Service</skos:prefLabel>
        <skos:definition xml:lang="en">DESCRIPTION:
Shares the functionality of referring to any activity aimed at verifying that the value of a data item comes from a given set of acceptable values. Data validation may be followed by corrective actions, such as data editing or data imputation.

Based on Eurostat Data Validation
http://ec.europa.eu/eurostat/data/data-validation

INTEROPERABILITY SALIENCY:
IoP Dimension: Behavioral IoP
The Data Validation Service ABB is salient for technical interoperability because it shares the functionality to validate if data received (or to be sent) is compliant with common and agreed interoperable formats as stated in the EIF recommendation n 41: &quot;Establish procedures and processes to integrate the opening of data in your common business processes, working routines, and in the development of new information systems.&quot;

EXAMPLES:
The following implementation is an example on how this specific Architecture Building Block (ABB) can be instantiated as a Solution Building Block (SBB):

Eurostat Struval
The Structural Validation service (called STRUVAL) performs structural validation of statistical data files following the SDMX Information Model for a given data flow. It ensures that a data file respects the following key elements:

	SDMX compliance in terms of checks on file format and completeness in terms of mandatory fields;
	SDMX compliance in terms of the structure and coding defined by the Data Structure Definition (DSD);
	The constraints defined for respective data flows.

The STRUVAL service returns a response containing a machine-readable message that is processed by the process manager. The invoker of the service receives a validation report, regardless of the result of the process (in case of no failures the reports hold no records).
http://ec.europa.eu/eurostat/web/sdmx-infospace/validation-transformation/structural-validation</skos:definition>
        <skos:topConceptOf rdf:resource="http://data.europa.eu/dr8"/>
    </skos:Concept>

    <skos:Concept rdf:about="http://data.europa.eu/dr8/DataValidationComponent">
        <skos:notation>DataValidationComponent</skos:notation>
        <skos:prefLabel xml:lang="en">[ABB63] Data Validation Component</skos:prefLabel>
        <skos:definition xml:lang="en">DESCRIPTION:
Implements the functionality of referring to any activity aimed at verifying that the value of a data item comes from a given set of acceptable values. Data validation may be followed by corrective actions, such as data editing or data imputation. In statistics, imputation is the process of replacing missing data with substituted values.

Based on Eurostat Data Validation
http://ec.europa.eu/eurostat/data/data-validation

INTEROPERABILITY SALIENCY:
IoP Dimension: Structural IoP
The Data Validation Component ABB is salient for technical interoperability because it allows the implementation of the functionality to validate if data received (or to be sent) is compliant with common and agreed interoperable formats as stated in the EIF recommendation n 41: &quot;Establish procedures and processes to integrate the opening of data in your common business processes, working routines, and in the development of new information systems.&quot;

EXAMPLES:
The following implementation is an example on how this specific Architecture Building Block (ABB) can be instantiated as a Solution Building Block (SBB):

Hibernate Validator
Express validation rules in a standardized way using annotation-based constraints and benefit from transparent integration with a wide variety of frameworks.
Application layer agnostic validation: Hibernate Validator allows to express and validate application constraints. The default metadata source are annotations, with the ability to override and extend through the use of XML. It is not tied to a specific application tier or programming model and is available for both server and client application programming.
Hibernate Validator presents the following characteristics:

	Extendable: Hibernate Validator offers a configurable bootstrap API as well as a range of built-in constraints. The latter can easily be extended by creating custom constraints.
	Rich metadata API: Hibernate Validator gives access to constraint configuration via a metadata API facilitating, for example, tooling integration.
	Reference implementation: Hibernate Validator 6.x is the reference implementation Bean Validation 2.0.
	Added value: Hibernate Validator offers additional value on top of the features required by Bean Validation. For example, a programmatic constraint configuration API as well as an annotation processor which plugs into the build process and raises compilation errors whenever constraint annotations are incorrectly used.

http://hibernate.org/validator/</skos:definition>
        <skos:topConceptOf rdf:resource="http://data.europa.eu/dr8"/>
    </skos:Concept>

    <skos:Concept rdf:about="http://data.europa.eu/dr8/ServiceDiscoveryService">
        <skos:notation>ServiceDiscoveryService</skos:notation>
        <skos:prefLabel xml:lang="en">[ABB159] Service Discovery Service</skos:prefLabel>
        <skos:definition xml:lang="en">DESCRIPTION:
Shares the functionality of locating a machine-processable description of a service-related resource that may have been previously unknown and that meets certain functional criteria. It involves matching a set of functional and other criteria with a set of resource descriptions. The goal is to find an appropriate service-related resource.

Based on W3C
https://www.w3.org/TR/2004/NOTE-ws-gloss-20040211/

INTEROPERABILITY SALIENCY:
IoP Dimension: Behavioral IoP
The Service Discovery Service ABB is salient for technical interoperability because it allows to discover service available for reuses as stated in the EIF recommendation n36: &quot;Develop a shared infrastructure of reusable services and information sources that can be used by all public administrations.&quot;

EXAMPLES:
The following implementation is an example on how this specific Architecture Building Block (ABB) can be instantiated as a Solution Building Block (SBB):

jUDDI
jUDDI is an open source Java implementation of OASIS the Universal Description, Discovery, and Integration (UDDI) specification for (Web) Services. The jUDDI project includes Scout. Scout is an implementation of the JSR 93 - JavaTM API for XML Registries 1.0 (JAXR).

Features:
	Platform Independent
	Use with any relational database that supports ANSI standard SQL (MySQL, Oracle, DB2, Sybase, Derby etc.)
	Deployable on any Java application server that supports the Servlet 2.3 specification
	jUDDI registry supports a clustered deployment configuration.
	Easy integration with existing authentication systems
	Supports InVM embeddable mode

jUDDIv3 Services:
	UDDI Specification version 3.0.2 compliant
	UDDI Specification version 2.0.4 interoperability services (BETA)
	Built on JAXB and JAX-WS standardized interfaces, tested on Apache CXF
	Built on JPA standardized interfaces, tested with Apache OpenJPA and Hibernate
	Pre-configured bundle deployed to Apache Tomcat
	Full featured user interface (based on Bootstrap)
	User, Administrative and Developer Documentation
	Includes extensive predefined tModels, such as Quality of Service Metrics

http://juddi.apache.org/</skos:definition>
        <skos:topConceptOf rdf:resource="http://data.europa.eu/dr8"/>
    </skos:Concept>

    <skos:Concept rdf:about="http://data.europa.eu/dr8/ServiceDiscoveryComponent">
        <skos:notation>ServiceDiscoveryComponent</skos:notation>
        <skos:prefLabel xml:lang="en">[ABB221] Service Discovery Component</skos:prefLabel>
        <skos:definition xml:lang="en">DESCRIPTION:
Implements the functionality of locating a machine-processable description of a service-related resource that may have been previously unknown and that meets certain functional criteria. It involves matching a set of functional and other criteria with a set of resource descriptions. The goal is to find an appropriate service-related resource.

Based on W3C
https://www.w3.org/TR/2004/NOTE-ws-gloss-20040211/

INTEROPERABILITY SALIENCY:
IoP Dimension: Structural IoP
The Service Discovery Component ABB is salient for technical interoperability because it allows to implement the funcionality of sharing services available for reuse as stated in the EIF recommendation n36: &quot;Develop a shared infrastructure of reusable services and information sources that can be used by all public administrations&quot;.

EXAMPLES:
The following implementation is an example on how this specific Architecture Building Block (ABB) can be instantiated as a Solution Building Block (SBB):

Consul
Consul has multiple components, but as a whole, it is a tool for discovering and configuring services in an infrastructure. It provides several key features:

	Service Discovery: Clients of Consul can provide a service, such as api or mysql, and other clients can use Consul to discover providers of a given service. Using either DNS or HTTP, applications can easily find the services they depend upon.
	Health Checking: Consul clients can provide any number of health checks, either associated with a given service (&quot;is the webserver returning 200 OK&quot;), or with the local node (&quot;is memory utilization below 90%&quot;). This information can be used by an operator to monitor cluster health, and it is used by the service discovery components to route traffic away from unhealthy hosts.
	KV Store: Applications can make use of Consul&apos;s hierarchical key/value store for any number of purposes, including dynamic configuration, feature flagging, coordination, leader election, and more. The simple HTTP API makes it easy to use.
	Multi Datacenter: Consul supports multiple datacenters out of the box. This means users of Consul do not have to worry about building additional layers of abstraction to grow to multiple regions.
https://www.consul.io/</skos:definition>
        <skos:topConceptOf rdf:resource="http://data.europa.eu/dr8"/>
    </skos:Concept>

    <skos:Concept rdf:about="http://data.europa.eu/dr8/OrchestrationService">
        <skos:notation>OrchestrationService</skos:notation>
        <skos:prefLabel xml:lang="en">[ABB45] Orchestration Service</skos:prefLabel>
        <skos:definition xml:lang="en">DESCRIPTION:
Shares the functionality of defining the sequence and conditions in which one service invokes other services in order to realize some useful function.

Based on W3C
https://www.w3.org/TR/ws-arch/

INTEROPERABILITY SALIENCY:
IoP Dimension: Behavioral IoP
The Orchestration Service ABB is salient for technical interoperability because it provides the functionality of &quot;automated&quot; business processes coordination.  The EIF&apos;s Conceptual model for integrated EU public services foresees the concept a Coordination for Integrated Service Delivery. The Model comprises an &quot;integrated service delivery&quot; is based on a &quot;coordination function&quot;, which is related to SOA principles such as choreography and orchestration, to manage internal business processes in order to remove complexity for the end-user, as stated in the EIF: &quot;The coordination function ensures that needs are identified and appropriate services are invoked and orchestrated to provide a European public service. This function should select the appropriate sources and services and integrate them. Coordination can be automated or manual.&quot;

EXAMPLES:
The following implementation is an example on how this specific Architecture Building Block (ABB) can be instantiated as a Solution Building Block (SBB):

Apache ODE
Apache ODE (Orchestration Director Engine) software executes business processes written following the WS-BPEL standard. It talks to web services, sending and receiving messages, handling data manipulation and error recovery as described by your process definition. It supports both long and short living process executions to orchestrate all the services that are part of your application.
http://ode.apache.org/</skos:definition>
        <skos:topConceptOf rdf:resource="http://data.europa.eu/dr8"/>
    </skos:Concept>

    <skos:Concept rdf:about="http://data.europa.eu/dr8/OrchestrationComponent">
        <skos:notation>OrchestrationComponent</skos:notation>
        <skos:prefLabel xml:lang="en">[ABB186] Orchestration Component</skos:prefLabel>
        <skos:definition xml:lang="en">DESCRIPTION:
Implements the functionality of defining the sequence and conditions in which one service invokes other services in order to realize some useful function.

Based on W3C
https://www.w3.org/TR/ws-arch/

INTEROPERABILITY SALIENCY:
IoP Dimension: Structural IoP
The Orchestration Component ABB is salient for technical interoperability because it provides a set of various methods to manage existing business processes or define and establish new ones. BPM components also execute business process documented through accepted modelling techniques, as recommended by the EIF n.28: &quot;Document your business processes using commonly accepted modelling techniques and agree on how these processes should be aligned to deliver a European public service.&quot;

EXAMPLES:
The following implementation is an example on how this specific Architecture Building Block (ABB) can be instantiated as a Solution Building Block (SBB):

Activiti
Activiti is an open-source workflow engine written in Java that can execute business processes described in BPMN 2.0. Activiti supports open standards such as BPMN and DMN with open REST APIs for demanding human- and system-centric processes. It provides business intelligence and audit logs features for free.  And with building the solution on business processes, Activiti help to structure the software, think about user tasks, external systems and timers that need to be managed, think about transaction boundaries of the application. Building that kind of features becomes easier when structuring an application around a business process. Managing wait states, timers and asynchronous continuations becomes easier. A business process can express that structure more compact than working with the fundamental instruments that the Java platform offers like JDBC and JMS. Activiti also makes possible to link in Java or scripting for jobs.
https://www.activiti.org/</skos:definition>
        <skos:topConceptOf rdf:resource="http://data.europa.eu/dr8"/>
    </skos:Concept>

    <skos:Concept rdf:about="http://data.europa.eu/dr8/TechnicalSpecification">
        <skos:notation>TechnicalSpecification</skos:notation>
        <skos:prefLabel xml:lang="en">[ABB125] Technical Specification</skos:prefLabel>
        <skos:definition xml:lang="en">DESCRIPTION:
A document that prescribes technical requirements to be fulfilled by a product, process or service.
- Note 1 to entry: A technical specification should indicate, whenever appropriate, the procedure(s) by means of which it may be determined whether the requirements given are fulfilled.
- Note 2 to entry: A technical specification may be a standard, a part of a standard or independent of a standard.

Source: https://www.iso.org/obp/ui/#iso:std:iso-iec:20944:-1:ed-1:v1:en:term:3.1.3.8]

INTEROPERABILITY SALIENCY:
IoP Dimension: Structural IoP, Behavioral IoP, Governance IoP
The Technical Specification ABB is salient for technical interoperability because it assesses the characteristics required of a product to support technical solutions.


EXAMPLES:
The following implementation is an example on how this specific Architecture Building Block (ABB) can be instantiated as a Solution Building Block (SBB):

AS4 Profile specification
The eDelivery AS4 Profile is a modular profile of the ebMS3 and AS4 OASIS specifications. Its core is a mandatory Common Profile that selects, extends and profiles the AS4 ebHandler Conformance Profile and AS4 Additional Features and provides a common Usage Profile. This Common Profile can be implemented using open source or closed source AS4 software implementations. It is aligned with, and corresponds to a subset of, the AS4 profile for TSOs (Transmission System Operators) developed by ENTSOG (the European Network of Transmission System Operators for Gas).
In addition to the Common Profile, this specification provides a number of optional Profile Enhancement modules that specify functionality enhancements covering AS4 message exchange in four corner topologies, the use of AS4 in conjunction with the UN/CEFACT Standard Business Document Header (SBDH) specification, and Dynamic Receiver and Dynamic Sender behavior.
https://ec.europa.eu/cefdigital/wiki/display/CEFDIGITAL/eDelivery+AS4+-+1.13</skos:definition>
        <skos:topConceptOf rdf:resource="http://data.europa.eu/dr8"/>
    </skos:Concept>

    <skos:Concept rdf:about="http://data.europa.eu/dr8/TechnicalInteroperabilityAgreement">
        <skos:notation>TechnicalInteroperabilityAgreement</skos:notation>
        <skos:prefLabel xml:lang="en">[ABB234] Technical Interoperability Agreement</skos:prefLabel>
        <skos:definition xml:lang="en">DESCRIPTION:
Technical Interoperability Agreement is the means through which Technical Authorities mandate specific Technical Interoperability Specifications, ensuring organisations (operating under different technical frameworks,
policies and strategies) are able to work together.

Based on EIF:
https://ec.europa.eu/isa2/sites/isa/files/eif_brochure_final.pdf#page=27

INTEROPERABILITY SALIENCY:
IoP dimensions: Governance IoP
The Technical Interoperability Agreement ABB  is a key interoperability enabler because it supports technical governance interoperability by enabling collaboration between digital public services.

EXAMPLES:
The following implementation is an example on how this specific Architecture Building Block (ABB) can be instantiated as a Solution Building Block (SBB):

ETA
The European Technical Assessment (ETA) is an alternative for construction products not covered by a harmonised standard. It is a document providing information on their performance assessment. The procedure is established in the Construction Products Regulation and offers a way for manufacturers to draw up the Declaration of Performance and affix the CE marking. It contributes to the free movement of construction products and the creation of a strong Single Market.
https://ec.europa.eu/growth/sectors/construction/product-regulation/european-assessment_en</skos:definition>
        <skos:topConceptOf rdf:resource="http://data.europa.eu/dr8"/>
    </skos:Concept>

    <skos:Concept rdf:about="http://data.europa.eu/dr8/SharedPlatform">
        <skos:notation>SharedPlatform</skos:notation>
        <skos:prefLabel xml:lang="en">[ABB367] Shared Platform</skos:prefLabel>
        <skos:definition xml:lang="en">DESCRIPTION:
A shared platform is formed by [re]usable ICT resources (i.e. the platform), with  convergence power, in relation to public policy goals attainment, given by the impact of the availability of common problem-solving instruments, across the levels of a public administration (central, regional, local) towards the achievement of the public policy goals, enabling :
i) structural interoperability by ICT resources  supporting reusing and/or sharing of data, information and knowledge (i.e. service registry service enabling provisioning/consuming [back-office] services cross public administrations and cross borders);
ii) behavioural interoperability by ICT resources supporting exchanging capabilities of data, information or knowledge with internal/external peers (i.e. technical interfaces enabling that data/information/knowledge be provisioned/consumed cross public administrations and cross borders); an
iii) governance interoperability by ICT resources supporting the collaboration with internal/external peers exchanging data, information or knowledge (i.e. Technical Interoperability Agreements on technical terms/conditions enabling sharing, reuse and exchange of data/information/knowledge cross public administrations and cross borders).

INTEROPERABILITY SALIENCY:
IoP dimensions: Structural  IoP  Behavioral IoP, Governance IoP
This ABB is a key interoperability enabler because it supports to achieve technical interoperability with public policy goals convergence value by  all in all enabling i) the provision/consumption of  back-office digital public services,  ii) the exchange of data, information, and knowledge between digital public services and individuals , and iii) collaboration between digital public services.</skos:definition>
        <skos:topConceptOf rdf:resource="http://data.europa.eu/dr8"/>
    </skos:Concept>

    <skos:Concept rdf:about="http://data.europa.eu/dr8/ConformanceTestingService">
        <skos:notation>ConformanceTestingService</skos:notation>
        <skos:prefLabel xml:lang="en">[ABB128] Conformance Testing Service</skos:prefLabel>
        <skos:definition xml:lang="en">DESCRIPTION:
Shares the functionality of verifying that several solutions can interoperate at one or more layers of the interoperability stack, while conforming to one or more specifications. This type of testing is executed by operating SUTs (System Under Test) and capturing their exchanges.
The logistics of interoperability testing is usually more costly (time, coordination, interoperability), and interoperability testing is no substitute for a conformance test suite. Experience shows that interoperability testing is more successful and less costly when conformance of implementations has been tested first.

Based on CEN/CENELC GITB
https://www.cen.eu/work/areas/ict/ebusiness/pages/ws-gitb.aspx

INTEROPERABILITY SALIENCY:
IoP Dimension: Behavioral IoP
The Conformance Testing Services ABB is salient for technical interoperability because it enables the validation and verification that several solutions at one or more layers of the interoperability stack and they satisfy certain interoperability requirements.

EXAMPLES:
The following implementation is an example on how this specific Architecture Building Block (ABB) can be instantiated as a Solution Building Block (SBB):

Interoperability Testbed
The Test Bed allows users to execute predefined test cases on their systems in order to test the conformance to standards and requirements, simulate a web-service, validate content and test a complete message exchange protocol. The Testbed manages test cases and users, and orchestrates domain-specific components, the domain-specific logic is in separate components that are used via web services.
Test results are provided in a standardised, machine-readable format. The Test Bed also offers a test registry and repository (TRR) to store test artefacts (assertions, test cases, validation schemas, etc.) and compile test services (validation services, simulator services, etc.).
Please visit the following website for more information:
https://ec.europa.eu/isa2/solutions/interoperability-test-bed_en</skos:definition>
        <skos:topConceptOf rdf:resource="http://data.europa.eu/dr8"/>
    </skos:Concept>

    <skos:Concept rdf:about="http://data.europa.eu/dr8/ConformanceTestingComponent">
        <skos:notation>ConformanceTestingComponent</skos:notation>
        <skos:prefLabel xml:lang="en">[ABB129] Conformance Testing Component</skos:prefLabel>
        <skos:definition xml:lang="en">DESCRIPTION:
Implements the functionality of allowing a structured and modular approach to implement test automation.

Based on ISTQB
http://glossary.istqb.org/search/test

INTEROPERABILITY SALIENCY:
IoP Dimension: Structural IoP
The Conformance Testing Component ABB is salient for technical interoperability because it enables the validation and verification that several solutions at one or more layers of the interoperability stack and they satisfy certain interoperability requirements.

EXAMPLES:
The following implementation is an example on how this specific Architecture Building Block (ABB) can be instantiated as a Solution Building Block (SBB):

Interoperability Testbed
The Test Bed allows users to execute predefined test cases on their systems in order to test the conformance to standards and requirements, simulate a web-service, validate content and test a complete message exchange protocol. The Testbed manages test cases and users, and orchestrates domain-specific components, the domain-specific logic is in separate components that are used via web services.
Test results are provided in a standardised, machine-readable format. The Test Bed also offers a test registry and repository (TRR) to store test artefacts (assertions, test cases, validation schemas, etc.) and compile test services (validation services, simulator services, etc.).
Please visit the following website for more information:
https://ec.europa.eu/isa2/solutions/interoperability-test-bed_en</skos:definition>
        <skos:topConceptOf rdf:resource="http://data.europa.eu/dr8"/>
    </skos:Concept>

    <skos:Concept rdf:about="http://data.europa.eu/dr8/ConformanceTestReport">
        <skos:notation>ConformanceTestReport</skos:notation>
        <skos:prefLabel xml:lang="en">[ABB131] Conformance Test Report</skos:prefLabel>
        <skos:definition xml:lang="en">DESCRIPTION:
Data from testing activities and subsequently consolidated in a report to inform stakeholders.

Based on ISTQB
http://glossary.istqb.org/search/test

Syn. Test results

INTEROPERABILITY SALIENCY:
IoP Dimension: Structural IoP
The Conformance Test Report ABB is salient for technical interoperability because it provides reports of data testing to inform stakeholders.

EXAMPLES:
The following implementation is an example on how this specific Architecture Building Block (ABB) can be instantiated as a Solution Building Block (SBB):

Jenkins jUnit plug-in

The JUnit plugin provides a publisher that consumes XML test reports generated during the builds and provides some graphical visualization of the historical test results (see JUnit graph for a sample) as well as a web UI for viewing test reports, tracking failures, and so on. Jenkins understands the JUnit test report XML format (which is also used by TestNG). When this option is configured, Jenkins can provide useful information about test results, such as trends.
https://wiki.jenkins.io/display/JENKINS/JUnit+Plugin</skos:definition>
        <skos:topConceptOf rdf:resource="http://data.europa.eu/dr8"/>
    </skos:Concept>

    <skos:Concept rdf:about="http://data.europa.eu/dr8/ConformanceTestScenario">
        <skos:notation>ConformanceTestScenario</skos:notation>
        <skos:prefLabel xml:lang="en">[ABB130] Conformance Test Scenario</skos:prefLabel>
        <skos:definition xml:lang="en">DESCRIPTION:
A document specifying a sequence of actions for the execution of a test. Also known as test script or manual test script.

Based on ISTQB
http://glossary.istqb.org/search/test

Syn. Test procedure

INTEROPERABILITY SALIENCY:
IoP Dimension: Structural IoP
The Conformance Testing Scenario ABB is salient for technical interoperability because it provides a document of a list of activities for the execution of interoperability tests.

EXAMPLES:
The following implementation is an example on how this specific Architecture Building Block (ABB) can be instantiated as a Solution Building Block (SBB):

SoapUI
SoapUI is the world&apos;s most widely-used open source API testing tool for SOAP and REST APIs. SoapUI offers SOAP Web Services functional testing, REST API functional testing, WSDL coverage, message assertion testing and test refactoring.
Scenario-based tests should be directly tied to user stories, which were probably provided by the product owner or some business stakeholder. Under ideal circumstances, these tests should be the user stories, so that business stakeholders can both easily help the tester develop the test cases and understand the results.
https://www.soapui.org/testing-dojo/best-practices/scenario-based-testing.html
https://www.soapui.org/testing-dojo/world-of-api-testing/test-first.html</skos:definition>
        <skos:topConceptOf rdf:resource="http://data.europa.eu/dr8"/>
    </skos:Concept>

    <skos:Concept rdf:about="http://data.europa.eu/dr8/TechnicalAgreement">
        <skos:notation>TechnicalAgreement</skos:notation>
        <skos:prefLabel xml:lang="en">[ABB377] Technical Agreement</skos:prefLabel>
        <skos:definition xml:lang="en">DESCRIPTION:
These agreements constitute a framework and a privileged forum to identify common interests, priorities, policy dialogue, and the necessary tools for Strategic &amp; Technological collaboration..

Based GMP Quality / Technical Agreements: https://ec.europa.eu/research/iscp/index.cfm?pg=countries

INTEROPERABILITY SALIENCY:
Not applicable

EXAMPLES:
The following implementation is an example on how this specific Architecture Building Block (ABB) can be instantiated as a Solution Building Block (SBB):

WTO Data Exchange technical agrement:
The agreement regulates the echange of data between systems and applications
https://olc.worldbank.org/sites/default/files/PMT-4.pdf</skos:definition>
        <skos:topConceptOf rdf:resource="http://data.europa.eu/dr8"/>
    </skos:Concept>

    <skos:Collection rdf:about="http://data.europa.eu/dr8/view/TechnicalView-Infrastructure">
        <skos:notation>TechnicalView-Infrastructure</skos:notation>
        <skos:prefLabel xml:lang="en">Technical View - Infrastructure</skos:prefLabel>
        <skos:member rdf:resource="http://data.europa.eu/dr8/DigitalServiceInfrastructure"/>
        <skos:member rdf:resource="http://data.europa.eu/dr8/MetadataManagementService"/>
        <skos:member rdf:resource="http://data.europa.eu/dr8/MetadataManagementComponent"/>
        <skos:member rdf:resource="http://data.europa.eu/dr8/E-archivingService"/>
        <skos:member rdf:resource="http://data.europa.eu/dr8/E-archivingComponent"/>
        <skos:member rdf:resource="http://data.europa.eu/dr8/FormsManagementService"/>
        <skos:member rdf:resource="http://data.europa.eu/dr8/FormsManagementComponent"/>
        <skos:member rdf:resource="http://data.europa.eu/dr8/DataPublicationService"/>
        <skos:member rdf:resource="http://data.europa.eu/dr8/DataPublicationComponent"/>
        <skos:member rdf:resource="http://data.europa.eu/dr8/PrivacyService"/>
        <skos:member rdf:resource="http://data.europa.eu/dr8/PrivacyComponent"/>
        <skos:member rdf:resource="http://data.europa.eu/dr8/ConfigurationAndSolutionCartographyService"/>
        <skos:member rdf:resource="http://data.europa.eu/dr8/ConfigurationAndSolutionCartographyServiceComponent"/>
        <skos:member rdf:resource="http://data.europa.eu/dr8/E-paymentService"/>
        <skos:member rdf:resource="http://data.europa.eu/dr8/E-paymentComponent"/>
        <skos:member rdf:resource="http://data.europa.eu/dr8/ServiceRegistrationService"/>
        <skos:member rdf:resource="http://data.europa.eu/dr8/ServiceRegistryComponent"/>
        <skos:member rdf:resource="http://data.europa.eu/dr8/MachineTranslationService"/>
        <skos:member rdf:resource="http://data.europa.eu/dr8/MachineTranslationComponent"/>
        <skos:member rdf:resource="http://data.europa.eu/dr8/E-signatureCreationService"/>
        <skos:member rdf:resource="http://data.europa.eu/dr8/E-signatureVerificationAndValidationService"/>
        <skos:member rdf:resource="http://data.europa.eu/dr8/E-signaturePreservationService"/>
        <skos:member rdf:resource="http://data.europa.eu/dr8/E-sealCreationService"/>
        <skos:member rdf:resource="http://data.europa.eu/dr8/E-sealVerificationAndValidationService"/>
        <skos:member rdf:resource="http://data.europa.eu/dr8/E-sealPreservationService"/>
        <skos:member rdf:resource="http://data.europa.eu/dr8/E-timestampCreationService"/>
        <skos:member rdf:resource="http://data.europa.eu/dr8/E-timestampVerificationAndValidationService"/>
        <skos:member rdf:resource="http://data.europa.eu/dr8/RegisteredElectronicDeliveryService"/>
        <skos:member rdf:resource="http://data.europa.eu/dr8/TrustServiceProvisioningComponent"/>
        <skos:member rdf:resource="http://data.europa.eu/dr8/IdentityManagementService"/>
        <skos:member rdf:resource="http://data.europa.eu/dr8/IdentityManagementComponent"/>
        <skos:member rdf:resource="http://data.europa.eu/dr8/TrustRegistryService"/>
        <skos:member rdf:resource="http://data.europa.eu/dr8/TrustRegistryComponent"/>
        <skos:member rdf:resource="http://data.europa.eu/dr8/DataExchangeService"/>
        <skos:member rdf:resource="http://data.europa.eu/dr8/DataExchangeComponent"/>
        <skos:member rdf:resource="http://data.europa.eu/dr8/HostingAndNetworkingInfrastructure"/>
        <skos:member rdf:resource="http://data.europa.eu/dr8/PublicNetwork"/>
        <skos:member rdf:resource="http://data.europa.eu/dr8/PrivateNetwork"/>
        <skos:member rdf:resource="http://data.europa.eu/dr8/Network"/>
        <skos:member rdf:resource="http://data.europa.eu/dr8/NetworkingService"/>
        <skos:member rdf:resource="http://data.europa.eu/dr8/HostingService"/>
        <skos:member rdf:resource="http://data.europa.eu/dr8/HostingFacility"/>
        <skos:member rdf:resource="http://data.europa.eu/dr8/PublicHostingFacility"/>
        <skos:member rdf:resource="http://data.europa.eu/dr8/PrivateHostingFacility"/>
        <skos:member rdf:resource="http://data.europa.eu/dr8/ContentManagementService"/>
        <skos:member rdf:resource="http://data.europa.eu/dr8/DataWarehouseService"/>
        <skos:member rdf:resource="http://data.europa.eu/dr8/DataWarehouseComponent"/>
        <skos:member rdf:resource="http://data.europa.eu/dr8/DataRepository"/>
        <skos:member rdf:resource="http://data.europa.eu/dr8/DataAnalyticsService"/>
        <skos:member rdf:resource="http://data.europa.eu/dr8/DataAnalyticsComponent"/>
        <skos:member rdf:resource="http://data.europa.eu/dr8/ArtificialIntelligenceService"/>
        <skos:member rdf:resource="http://data.europa.eu/dr8/ArtificialIntelligenceComponent"/>
        <skos:member rdf:resource="http://data.europa.eu/dr8/SmartDevices"/>
        <skos:member rdf:resource="http://data.europa.eu/dr8/HighPerformanceInfrastructure"/>
        <skos:member rdf:resource="http://data.europa.eu/dr8/DataInfrastructure"/>
        <skos:member rdf:resource="http://data.europa.eu/dr8/DataHub"/>
        <skos:member rdf:resource="http://data.europa.eu/dr8/DataLake"/>
        <skos:member rdf:resource="http://data.europa.eu/dr8/DataRepositoryExchangeService"/>
        <skos:member rdf:resource="http://data.europa.eu/dr8/DataRepositoryExchangeComponent"/>
    </skos:Collection>

    <skos:Concept rdf:about="http://data.europa.eu/dr8/DigitalServiceInfrastructure">
        <skos:notation>DigitalServiceInfrastructure</skos:notation>
        <skos:prefLabel xml:lang="en">[ABB188] Digital Service Infrastructure</skos:prefLabel>
        <skos:definition xml:lang="en">DESCRIPTION:
Infrastructure which enable networked services to be delivered electronically, typically over the internet, providing trans-European interoperable services of common interest for citizens, businesses  and/or public authorities, and which are composed of core service platforms and generic services

Source: Regulation (EU) No 283/2014
http://eur-lex.europa.eu/legal-content/EN/TXT/PDF/?uri=CELEX:32014R0283&amp;from=EN

INTEROPERABILITY SALIENCY:
IoP Dimension: Structural IoP, Behavioral IoP
The Digital Infrastructure Service ABB is salient for technical interoperability because it a central element through which interoperability is ensured and by definition, as intended in the EIRA, Digital Service Infrastructure provide trans-European interoperable services.

EXAMPLES:
The following implementation is an example on how this specific Architecture Building Block (ABB) can be instantiated as a Solution Building Block (SBB):
CEF Digital Service Infrastructure for eHealth
eHealth refers to tools and services using information and communication technologies (ICTs) that can improve prevention, diagnosis, treatment, monitoring and management. So far the Digital Service Infrastructure for eHealth is planned to support several services:
-	Cross-border patient summary service
-	ePrescriptions and eDispensations
In the future, two other services, the European Reference Networks and Interoperable Patient registries might be deployed.
https://webgate.ec.europa.eu/sanco-xmlgate/Login.jsp</skos:definition>
        <skos:topConceptOf rdf:resource="http://data.europa.eu/dr8"/>
    </skos:Concept>

    <skos:Concept rdf:about="http://data.europa.eu/dr8/MetadataManagementService">
        <skos:notation>MetadataManagementService</skos:notation>
        <skos:prefLabel xml:lang="en">[ABB52] Metadata Management Service</skos:prefLabel>
        <skos:definition xml:lang="en">DESCRIPTION:
Shares the functionalities for the i) creation, ii) storage, iii) categorisation and iv) retrieval of metadata.

Based on DAMA
http://www.dama.org/

INTEROPERABILITY SALIENCY:
IoP Dimension: Behavioral IoP
The Metadata management Service ABB is salient for interoperability  because it provides and shares the functionalities to manage metadata. EIF recommends to prioritise it: &quot;Put in place an information management strategy at the highest possible level to avoid fragmentation and duplication. Management of metadata, master data and reference data should be prioritised&quot;.

EXAMPLES:
The following implementation is an example on how this specific Architecture Building Block (ABB) can be instantiated as a Solution Building Block (SBB):
Eurostat SDMX repository
The Euro SDMX Registry is Eurostats implementation of an SDMX registry to facilitate the exchange of statistical data and metadata by serving as a metadata repository. It stores the SDMX artefacts needed for the parties to access and interpret the content of the exchanged statistical data and metadata sets.
http://ec.europa.eu/eurostat/web/sdmx-infospace/sdmx-it-tools/sdmx-registry</skos:definition>
        <skos:narrower rdf:resource="http://data.europa.eu/dr8/InteroperableEuropeanSolutionService"/>
    </skos:Concept>

    <skos:Concept rdf:about="http://data.europa.eu/dr8/MetadataManagementComponent">
        <skos:notation>MetadataManagementComponent</skos:notation>
        <skos:prefLabel xml:lang="en">[ABB74] Metadata Management Component</skos:prefLabel>
        <skos:definition xml:lang="en">DESCRIPTION:
Implements the functionalities for the i) creation, ii) storage, iii) categorisation and iv) retrieval of metadata.

Based on DAMA
http://www.dama.org/

INTEROPERABILITY SALIENCY:
IoP Dimension: Structural IoP
The Metadata management Component ABB is salient for interoperability  because it provides the implementation of the functionalities to manage metadata. EIF recommends to prioritise it: &quot;Put in place an information management strategy at the highest possible level to avoid fragmentation and duplication. Management of metadata, master data and reference data should be prioritised.&quot;

EXAMPLES:
The following implementation is an example on how this specific Architecture Building Block (ABB) can be instantiated as a Solution Building Block (SBB):
Eurostat SDMX repository
The Euro SDMX Registry is Eurostats implementation of an SDMX registry to facilitate the exchange of statistical data and metadata by serving as a metadata repository. It stores the SDMX artefacts needed for the parties to access and interpret the content of the exchanged statistical data and metadata sets.
http://ec.europa.eu/eurostat/web/sdmx-infospace/sdmx-it-tools/sdmx-registry</skos:definition>
        <skos:topConceptOf rdf:resource="http://data.europa.eu/dr8"/>
    </skos:Concept>

    <skos:Concept rdf:about="http://data.europa.eu/dr8/E-archivingService">
        <skos:notation>E-archivingService</skos:notation>
        <skos:prefLabel xml:lang="en">[ABB156] e-Archiving Service</skos:prefLabel>
        <skos:definition xml:lang="en">DESCRIPTION:
Shares the functionality of enabling the permanent or long-term storage of selected (by an authority) electronic documents or information for preservation purposes like their enduring research value and memory aid.

The EIRA(c) differentiates between document management, record management and e-archiving as follows:
- Document management is primarily about day-to-day use of electronic documents (create/update/delete/versioning) within the operational environment;
- Record management is primarily about ensuring that information (e.g. in form of an electronic document or database record) is available for business and legal purposes (e.g. to proof and track the handling of contracts). If an electronic document or information is becoming a record (an authority declares it as a record) that electronic document or information needs to be handled by the record management service (based on specific business or legal reasons (e.g. contract negotiation)).
- e-Archiving is primarily about storing records which have been selected (by an authority) for permanent or long-term preservation due to their enduring research value and as a memory aid. An electronic document or information which a) is managed by the document management service or the record management service and b) is no longer needed for business or legal purposes or day-to-day activities, and c) still has value for research purposes or as a memory aid, the electronic document should be managed by the e-archiving service.

Source: ISA2 - EIA Action

INTEROPERABILITY SALIENCY:
IoP Dimension: Behavioral IoP
The e-Archiving Service ABB is salient for technical interoperability because it provides and shares the functionality for the long-term or permanent preservation of records and information in electronic form in order to ensure their temporal egibility, reliability and integrity as stated in the EIF: &quot;Legislation requires that decisions and data are stored and can be accessed for a specified time. This means that records and information in electronic form held by public administrations for the purpose of documenting procedures and decisions must be preserved and be converted, where necessary, to new media when old media become obsolete. The goal is to ensure that records and other forms of information keep their legibility, reliability and integrity and can be accessed as long as needed subject to security and privacy provisions.&quot;

EXAMPLES:
The following implementation is an example on how this specific Architecture Building Block (ABB) can be instantiated as a Solution Building Block (SBB):

CEF eArchiving
eArchiving provides the core specifications, software, training and knowledge to tackle the challenge of short, medium and long-term data management and reuse in a sustainable, authentic, cost-efficient, manageable and interoperable way.
https://ec.europa.eu/cefdigital/wiki/display/CEFDIGITAL/eArchiving</skos:definition>
        <skos:narrower rdf:resource="http://data.europa.eu/dr8/InteroperableEuropeanSolutionService"/>
    </skos:Concept>

    <skos:Concept rdf:about="http://data.europa.eu/dr8/E-archivingComponent">
        <skos:notation>E-archivingComponent</skos:notation>
        <skos:prefLabel xml:lang="en">[ABB157] e-Archiving Component</skos:prefLabel>
        <skos:definition xml:lang="en">DESCRIPTION:
Shares the functionality of enabling the permanent or long-term storage of selected (by an authority) electronic documents or information for preservation purposes like their enduring research value and memory aid.

The EIRA differentiates between document management, record management and e-archiving as follows:
	Document management is primarily about day-to-day use of electronic documents (create/update/delete/versioning) within the operational environment;
	Record management is primarily about ensuring that information (e.g. in form of an electronic document or database record) is available for business and legal purposes (e.g. to proof and track the handling of contracts). If an electronic document or information is becoming a record (an authority declares it as a record) that electronic document or information needs to be handled by the record management service (based on specific business or legal reasons (e.g. contract negotiation)).
	e-Archiving is primarily about storing records which have been selected (by an authority) for permanent or long-term preservation due to their enduring research value and as a memory aid. An electronic document or information which a) is managed by the document management service or the record management service and b) is no longer needed for business or legal purposes or day-to-day activities, and c) still has value for research purposes or as a memory aid, the electronic document should be managed by the e-archiving service.
Source: ISA2 - EIA Action

Syn. Preservation Service

INTEROPERABILITY SALIENCY:
IoP Dimension: Structural IoP
The e-Archiving Component ABB is salient for technical interoperability because it provides the implementation of the functionalities for the long-term or permanent preservation of records and information in electronic form in order to ensure their temporal egibility, reliability and integrity as stated in the EIF: &quot;Legislation requires that decisions and data are stored and can be accessed for a specified time. This means that records and information in electronic form held by public administrations for the purpose of documenting procedures and decisions must be preserved and be converted, where necessary, to new media when old media become obsolete. The goal is to ensure that records and other forms of information keep their legibility, reliability and integrity and can be accessed as long as needed subject to security and privacy provisions.&quot;

EXAMPLES:
The following implementation is an example on how this specific Architecture Building Block (ABB) can be instantiated as a Solution Building Block (SBB):

CEF eArchiving
eArchiving provides the core specifications, software, training and knowledge to tackle the challenge of short, medium and long-term data management and reuse in a sustainable, authentic, cost-efficient, manageable and interoperable way.
https://ec.europa.eu/cefdigital/wiki/display/CEFDIGITAL/eArchiving</skos:definition>
        <skos:topConceptOf rdf:resource="http://data.europa.eu/dr8"/>
    </skos:Concept>

    <skos:Concept rdf:about="http://data.europa.eu/dr8/FormsManagementService">
        <skos:notation>FormsManagementService</skos:notation>
        <skos:prefLabel xml:lang="en">[ABB49] Forms Management Service</skos:prefLabel>
        <skos:definition xml:lang="en">DESCRIPTION:
Shares the functionalities of i) dynamic creation, ii) distribution and ii) analysis of forms and online surveys.

Source: ISA2 - EIA Action

Syn. e-Forms Service

INTEROPERABILITY SALIENCY:
IoP Dimension: Behavioral IoP
The Forms Management Service ABB is salient for technical interoperability because it provides and shares the functionalities  of dynamic creation, distribution and analysis of forms and online surveys as stated in the EIF: &quot; Catalogues help others to find reusable resources (e.g. services, data, software, data models). Various types of catalogue exist, e.g. directories of services, libraries of software components, open data portals, registries of base registries, metadata catalogues, catalogues of standards, specifications and guidelines. Commonly agreed descriptions of the services, data, registries and interoperable solutions published in catalogues are needed to enable interoperability between catalogues.&quot;

EXAMPLES:
The following implementation is an example on how this specific Architecture Building Block (ABB) can be instantiated as a Solution Building Block (SBB):

EACEA e-Forms
Electronic Application Forms - eForms
This page contains the resources and information required by applicants who wish to complete and submit an electronic application form (eForm) for a funding opportunity or for an accreditation.
The programmes and actions are listed for which electronic application forms are currently available. The Application eForm homepage is where applicants for funding and applicants for accreditation must follow a series of steps in order to create their new application.
https://eacea.ec.europa.eu/about-eacea/electronic-application-forms-eforms_en</skos:definition>
        <skos:narrower rdf:resource="http://data.europa.eu/dr8/InteroperableEuropeanSolutionService"/>
    </skos:Concept>

    <skos:Concept rdf:about="http://data.europa.eu/dr8/FormsManagementComponent">
        <skos:notation>FormsManagementComponent</skos:notation>
        <skos:prefLabel xml:lang="en">[ABB77] Forms Management Component</skos:prefLabel>
        <skos:definition xml:lang="en">DESCRIPTION:
Implements the functionalities of i) dynamic creation, ii) distribution and ii) analysis of forms and online surveys.

Source: ISA2 - EIA Action

Syn. e-Forms Component

INTEROPERABILITY SALIENCY:
IoP Dimension: Structural IoP

The Forms Management Component ABB is salient for technical interoperability because it provides  the implementation of the functionalities  of dynamic creation, distribution and analysis of forms and online surveys as stated in the EIF: &quot; Catalogues help others to find reusable resources (e.g. services, data, software, data models). Various types of catalogue exist, e.g. directories of services, libraries of software components, open data portals, registries of base registries, metadata catalogues, catalogues of standards, specifications and guidelines. Commonly agreed descriptions of the services, data, registries and interoperable solutions published in catalogues are needed to enable interoperability between catalogues.&quot;

EXAMPLES:
The following implementation is an example on how this specific Architecture Building Block (ABB) can be instantiated as a Solution Building Block (SBB):

Form Tools
Form Tools is a forms framework written in PHP and MySQL. You download and install the script on your own website. At its heart, Form Tools is a web form creator, processor, data storage and access script. It was originally designed to work with any existing web form, but has since been expanded to create forms automatically as well.
Form Tools is extremely versatile in how it integrates with your forms. You can use the bundled Form Builder module to create the forms automatically on your website (no programming or HTML skills necessary); you can use the PHP API to integrate your own custom form with the script; or you can simply POST your form to Form Tools, and just use it to store the form data. Anything goes! You can read about the different integration methods / form creation methods here.
Form Tools works by creating custom database tables to store your unique form data. It provides a range of functionality customized to your data set, such as allowing you to view, update, cross-reference and export your submission data, create subsets of your data for viewing/editing by client accounts, data visualizations, and much more.
https://formtools.org/</skos:definition>
        <skos:topConceptOf rdf:resource="http://data.europa.eu/dr8"/>
    </skos:Concept>

    <skos:Concept rdf:about="http://data.europa.eu/dr8/DataPublicationService">
        <skos:notation>DataPublicationService</skos:notation>
        <skos:prefLabel xml:lang="en">[ABB215] Data Publication Service</skos:prefLabel>
        <skos:definition xml:lang="en">DESCRIPTION:
Shares the functionality of making data available for common use.

Based on DAMA
http://www.dama.org/

INTEROPERABILITY SALIENCY:
IoP Dimension: Behavioral IoP
The Data Pubblication Service ABB is salient for technical interoperability because it provides the functionalities to make public data freely available for use and reuse by others unless restriction aoply as stated in the EIF recommendation n.2: &quot;Publish the data you own as open data unless certain restrictions apply.&quot;

EXAMPLES:
The following implementation is an example on how this specific Architecture Building Block (ABB) can be instantiated as a Solution Building Block (SBB):
European Data Portal
The European Data Portal harvests the metadata of Public Sector Information available on public data portals across European countries. Information regarding the provision of data and the benefits of re-using data is also included.
What is Open Data?
-	Open (Government) Data refers to the information collected, produced or paid for by the public bodies (also referred to as Public Sector Information) and made freely available for re-use for any purpose. The licence will specify the terms of use.
-	Public sector information is information held by the public sector. The Directive on the re-use of public sector information provides a common legal framework for a European market for government-held data. It is built around the key pillars of the internal market: free flow of data, transparency and fair competition. It is important to note that not all of the public sector information is Open Data.
Within the Portal, sections are dedicated to:
-	Searching datasets: Categories have been established to structure the metadata harvested from the various countries. These categories follow the revision of the DCAT Application Profile and have been mapped against the Eurovoc Thesaurus.
-	Providing Data: This section gives an insight into understanding Open Data from the perspective of a data provider. In addition, instructions are offered for those who wish their data portal to be harvested by the European Data Portal.
-	Using Data: How Open Data is being used, as well as the economic benefits of Open Data are detailed in this section.
-	Training and Library: eLearning modules about Open Data as well as training guides and a knowledge base referencing publications around Open Data and featured projects.
Portals can be national, regional, local or domain specific. They cover the 28 EU Member States, EEA, countries involved in the EU&apos;s neighbourhood policy and Switzerland.
https://www.europeandataportal.eu/

Belgian Data Portal
The Belgian Data Portal provides data (more than 6500 datasets), tools and resources.
Open Data is a driver for innovation, economic growth, transparency and participation. According to a European study (ref.COM (2011) 882) the cumulative economic benefits arising from the provision of public data would amount to  40 billion per year in the EU. These data lend themselves to reuse in the context of new products and services and can improve the efficiency of public authorities. Making public sector data accessible makes it possible to involve citizens more in political and social life and to make an active contribution to policy areas such as the environment, mobility, the economy, and so on.
The 2014-2018 Belgian government agreement states that the government will focus on opening public sector data (Open Data policy). Open public data is now the rule. Public services make available to citizens, researchers, companies and public authorities the reuse of data already available to them in the framework of their missions.
It is more specifically data that:
-	Public services have collected as part of their data collection missions;
-	Do not contain (more) privacy-sensitive information that is not protected by intellectual property rights held by third parties;
-	Are published in a format that is easy to reuse automatically (&quot;machine readable &quot;);
-	Can be reused for commercial and non-commercial purposes.
It is not only a matter of making public service data available, but also of building a community environment around these data. Companies can reuse some data and enrich it with their own information to market new products and services. Citizens benefit from more transparent public authorities and public services can help improve the quality of existing public data and services.
http://data.gov.be/en</skos:definition>
        <skos:narrower rdf:resource="http://data.europa.eu/dr8/InteroperableEuropeanSolutionService"/>
    </skos:Concept>

    <skos:Concept rdf:about="http://data.europa.eu/dr8/DataPublicationComponent">
        <skos:notation>DataPublicationComponent</skos:notation>
        <skos:prefLabel xml:lang="en">[ABB209] Data Publication Component</skos:prefLabel>
        <skos:definition xml:lang="en">DESCRIPTION:
Implements the functionality of making data available for common use.

Based on DAMA
http://www.dama.org/

INTEROPERABILITY SALIENCY:
IoP Dimension: Structural IoP
The Data Pubblication Component ABB is salient for technical interoperability because it provides the implementation of the functionalities to make public data freely available for use and reuse by others unless restriction aoply as stated in the EIF recommendation n.2: &quot;Publish the data you own as open data unless certain restrictions apply.&quot;

EXAMPLES:
The following implementation is an example on how this specific Architecture Building Block (ABB) can be instantiated as a Solution Building Block (SBB):
CKAN
CKAN is a data management system that makes data accessible by providing tools to streamline publishing, sharing, finding and using data.
This is a tool for making open data websites. It helps you manage and publish collections of data. It is used by national and local governments, research institutions, and other organizations who collect a lot of data.
Once your data is published, users can use its faceted search features to browse and find the data they need, and preview it using maps, graphs and tables  whether they are developers, journalists, researchers, NGOs, citizens, or even your own staff.
CKAN is open source and free software, with an active community of contributors who develop and maintain its core technology. CKAN is modified and extended by an even larger community of developers who contribute to a growing library of CKAN extensions.
https://ckan.org/

The following implementation is an example on how this specific Architecture Building Block (ABB) can be instantiated as a Solution Building Block (SBB):
Globus
Globus is a leading provider of research data management software application and platform services.
Globus publication capabilities are delivered through a hosted service. Published data is stored on campus, institutional, and group resources that are often managed and operated by different administrators. To associate storage resources with a data collection simply use Globus shared endpoints and associate them with the data repository to publish. Published datasets are organized by &quot;communities&quot; and their member &quot;collections&quot;. Globus users can create and manage their own communities and collections through the data publication service. A collection enables the submission of datasets with policies regarding access.
A dataset comprises data and metadata. Policies can be set on communities or collections to manage:
-	Metadata (schema, requirements)
-	Access control (user and group based)
-	Curation workflow
-	Submission and distribution licenses
-	Storage
Datasets undergo curation based on a workflow defined by the community that will publish the data. Workflows may be customized by each community to capture their specific metadata and to reflect the community&apos;s review process. After the dataset is published, it is discoverable using a faceted search that allows the researcher to progressively filter results and rapidly focus in on the data of interest. The data may then be transferred to a Globus endpoint where the investigator can inspect and further process the data.
Data publication is a premium feature available with a Globus Subscription
https://www.globus.org/data-publication</skos:definition>
        <skos:topConceptOf rdf:resource="http://data.europa.eu/dr8"/>
    </skos:Concept>

    <skos:Concept rdf:about="http://data.europa.eu/dr8/PrivacyService">
        <skos:notation>PrivacyService</skos:notation>
        <skos:prefLabel xml:lang="en">[ABB235] Privacy Service</skos:prefLabel>
        <skos:definition xml:lang="en">DESCRIPTION:
Privacy Service shares the functionalities of storing, securing, anonymising, pseudonymising, rectifying and erasing personal data.

INTEROPERABILITY SALIENCY:
IoP Dimension: Behavioral IoP
The Privacy Service ABB is salient for interoperability because &quot;security and privacy are primary concerns in the provision of public services&quot; (EIF) and, as stated in EIF Recommendation 15: &quot;Define a common security and privacy framework and establish processes for public services to ensure secure and trustworthy data exchange between public administrations and in interactions with citizens and businesses.&quot;

EXAMPLES:
The following implementation is an example on how this specific Architecture Building Block (ABB) can be instantiated as a Solution Building Block (SBB):

SOLVIT
Solvit is a mailbox service for the access, rectification or deletion of personal data.
http://ec.europa.eu/solvit/privacy-statement/#maincontentSec8</skos:definition>
        <skos:narrower rdf:resource="http://data.europa.eu/dr8/InteroperableEuropeanSolutionService"/>
    </skos:Concept>

    <skos:Concept rdf:about="http://data.europa.eu/dr8/PrivacyComponent">
        <skos:notation>PrivacyComponent</skos:notation>
        <skos:prefLabel xml:lang="en">[ABB236] Privacy Component</skos:prefLabel>
        <skos:definition xml:lang="en">DESCRIPTION:
Privacy Component implements the functionalities of storing, securing, anonymising, pseudonymising, rectifying and erasing personal data.

INTEROPERABILITY SALIENCY:
IoP Dimension: Structural IoP
The Privacy Service ABB is salient for interoperability because &quot;security and privacy are primary concerns in the provision of public services&quot; (EIF) and, as stated in EIF Recommendation 15: &quot;Define a common security and privacy framework and establish processes for public services to ensure secure and trustworthy data exchange between public administrations and in interactions with citizens and businesses.&quot;

EXAMPLES:
The following implementation is an example on how this specific Architecture Building Block (ABB) can be instantiated as a Solution Building Block (SBB):

SOLVIT
Solvit is a mailbox service for the access, rectification or deletion of personal data.
http://ec.europa.eu/solvit/privacy-statement/#maincontentSec8</skos:definition>
        <skos:topConceptOf rdf:resource="http://data.europa.eu/dr8"/>
    </skos:Concept>

    <skos:Concept rdf:about="http://data.europa.eu/dr8/ConfigurationAndSolutionCartographyService">
        <skos:notation>ConfigurationAndSolutionCartographyService</skos:notation>
        <skos:prefLabel xml:lang="en">[ABB210] Configuration and Solution Cartography Service</skos:prefLabel>
        <skos:definition xml:lang="en">DESCRIPTION:
Shares the functionality of documenting the configuration and architecture of solutions.

Source: ISA2 - EIA Action

INTEROPERABILITY SALIENCY:
The Configuration and Solution of Cartography Service ABB is salient for technical interoperability because it can be used to document the interoperabilty features of a solution or a set of solution/services.

EXAMPLES:
The following implementation is an example on how this specific Architecture Building Block (ABB) can be instantiated as a Solution Building Block (SBB):

Essential
The EA Essential tool provides with a semantically-rich meta-model. This means accurate modelling which allows for sophisticated reporting. Essential can be configured to import data from a wide range of sources such as CMDBs, Business Process Modelling tools, PMO tools, etc. The Essential Import Utility REST API allows to schedule automated imports from external data sources to keep the repository accurate and current. Complex queries can be built on the repository using the query wizard in Essential Open Source.
In addition to traditional the Enterprise Architecture assets, Essential also manages information about the entire organization including resources, skills, contracts, risk, security and more.
https://www.enterprise-architecture.org/features.php</skos:definition>
        <skos:narrower rdf:resource="http://data.europa.eu/dr8/InteroperableEuropeanSolutionService"/>
    </skos:Concept>

    <skos:Concept rdf:about="http://data.europa.eu/dr8/ConfigurationAndSolutionCartographyServiceComponent">
        <skos:notation>ConfigurationAndSolutionCartographyServiceComponent</skos:notation>
        <skos:prefLabel xml:lang="en">[ABB213] Configuration and Solution Cartography Service Component</skos:prefLabel>
        <skos:definition xml:lang="en">DESCRIPTION:
Implements the functionality of documenting the configuration and architecture of solutions.

Source: ISA2 - EIA Action

INTEROPERABILITY SALIENCY:
The Configuration and Solution of Cartography Component ABB is salient for technical interoperability because it provides the implementation of the functionalities which can be exploited to document the interoperabilty features of a solution or a set of solution/services.

EXAMPLES:
The following implementation is an example on how this specific Architecture Building Block (ABB) can be instantiated as a Solution Building Block (SBB):

Essential
The EA Essential tool provides with a semantically-rich meta-model. This means accurate modelling which allows for sophisticated reporting. Essential can be configured to import data from a wide range of sources such as CMDBs, Business Process Modelling tools, PMO tools, etc. The Essential Import Utility REST API allows to schedule automated imports from external data sources to keep the repository accurate and current. Complex queries can be built on the repository using the query wizard in Essential Open Source.
In addition to traditional the Enterprise Architecture assets, Essential also manages information about the entire organization including resources, skills, contracts, risk, security and more.
https://www.enterprise-architecture.org/features.php</skos:definition>
        <skos:topConceptOf rdf:resource="http://data.europa.eu/dr8"/>
    </skos:Concept>

    <skos:Concept rdf:about="http://data.europa.eu/dr8/E-paymentService">
        <skos:notation>E-paymentService</skos:notation>
        <skos:prefLabel xml:lang="en">[ABB48] e-Payment Service</skos:prefLabel>
        <skos:definition xml:lang="en">DESCRIPTION:
Shares the functionality of executing payment transactions where the consent of the payer to execute a payment transaction is given by means of any telecommunication, digital or IT device.

Source: Directive 2007/64/EC
http://eur-lex.europa.eu/LexUriServ/LexUriServ.do?uri=CELEX:32007L0064:EN:NOT

INTEROPERABILITY SALIENCY:
IoP Dimension: Behavioral IoP
The e-Payment Service ABBis salient for technical interoperability because it enables the possibility of executing payment transactions by any means of telecommunication, digital or IT device as stated in the EIF: &quot;Public administrations need to exploit services delivered outside their organisational boundaries by third parties, such as payment services provided by financial institutions or connectivity services provided by telecommunications providers.&quot;

EXAMPLES:
The following implementation is an example on how this specific Architecture Building Block (ABB) can be instantiated as a Solution Building Block (SBB):

SEPA
The single euro payments area (SEPA) harmonises the way cashless euro payments are made across Europe. It allows European consumers, businesses and public administrations to make and receive the following types of transactions under the same basic conditions:
-	credit transfers
-	direct debit payments
-	card payments
This makes all cross-border electronic payments in euro as easy as domestic payments.
https://ec.europa.eu/info/business-economy-euro/banking-and-finance/consumer-finance-and-payments/payment-services/single-euro-payments-area-sepa_en

UniPay Payment Gateway
The open source payment transactions processing platform UniPay Payment Gateway is a robust, flexible and scalable payment gateway software.
The platform has a powerful, processor-agnostic payment gateway at its foundation, which supplies numerous direct-to-processor backend integrations and includes a powerful routing engine configurable through web service calls. With unified API as your entry point (for both credit card transactions and ACH - Automated Clearing House), you gain access to numerous banks and credit card payment processors across the globe.
http://opensourcepaymentgateway.com/</skos:definition>
        <skos:narrower rdf:resource="http://data.europa.eu/dr8/InteroperableEuropeanSolutionService"/>
    </skos:Concept>

    <skos:Concept rdf:about="http://data.europa.eu/dr8/E-paymentComponent">
        <skos:notation>E-paymentComponent</skos:notation>
        <skos:prefLabel xml:lang="en">[ABB68] e-Payment Component</skos:prefLabel>
        <skos:definition xml:lang="en">DESCRIPTION:
Implements the functionality of executing payment transactions where the consent of the payer to execute a payment transaction is given by means of any telecommunication, digital or IT device.

Source: Directive 2007/64/EC
http://eur-lex.europa.eu/LexUriServ/LexUriServ.do?uri=CELEX:32007L0064:EN:NOT

INTEROPERABILITY SALIENCY:
IoP Dimension: Structural IoP

The e-Payment Component ABB is salient for technical interoperability because it provides the implementation of functionalities of executing payment transactions.

EXAMPLES:
The following implementation is an example on how this specific Architecture Building Block (ABB) can be instantiated as a Solution Building Block (SBB):

OpenACH
Introducing OpenACH, the world&apos;s first free, open-source, secure web-based ACH origination and payment processing platform.
ACH stands for &quot;Automated Clearing House&quot; and is a term that can be used very loosely in the banking and business industries. An originator is a business or organization initiating a transaction, either credit or debit.
OpenACH is several things:
-	An open source (GPLv3) ACH payment platform, written in PHP using Postgresql
-	An easy to use ACH payment gateway, using REST and JSON to put payments on the ACH network
-	A BYOB (Bring Your Own Bank) ACH processing platform
-	A third-party ACH originator, processing your payments on your behalf
https://openach.com/</skos:definition>
        <skos:topConceptOf rdf:resource="http://data.europa.eu/dr8"/>
    </skos:Concept>

    <skos:Concept rdf:about="http://data.europa.eu/dr8/ServiceRegistrationService">
        <skos:notation>ServiceRegistrationService</skos:notation>
        <skos:prefLabel xml:lang="en">[ABB189] Service Registration Service</skos:prefLabel>
        <skos:definition xml:lang="en">DESCRIPTION:
Shares the functionality of registering the system service within a catalogue to be discovered by other services.

Source ISA2 - EIA Action

Syn. Service Catalogue Service

INTEROPERABILITY SALIENCY:
IoP Dimension: Behavioral IoP
The  Service Registration Service ABB is a key interoperability enabler because it supports to achieve technical structural interoperability by ensuring the provision/consumption of  back-office digital public services.

EXAMPLES:
The following implementation is an example on how this specific Architecture Building Block (ABB) can be instantiated as a Solution Building Block (SBB):

Apache ZooKeeper
Apache ZooKeeper is an effort to develop and maintain an open-source server which enables highly reliable distributed coordination.
ZooKeeper is a centralized service for maintaining configuration information, naming, providing distributed synchronization, and providing group services. All of these kinds of services are used in some form or another by distributed applications. Each time they are implemented there is a lot of work that goes into fixing the bugs and race conditions that are inevitable. Because of the difficulty of implementing these kinds of services, applications initially usually skimp on them, which make them brittle in the presence of change and difficult to manage. Even when done correctly, different implementations of these services lead to management complexity when the applications are deployed.
ZooKeeper aims at distilling the essence of these different services into a very simple interface to a centralized coordination service. The service itself is distributed and highly reliable. Consensus, group management, and presence protocols will be implemented by the service so that the applications do not need to implement them on their own. Application specific uses of these will consist of a mixture of specific components of Zoo Keeper and application specific conventions. ZooKeeper Recipes shows how this simple service can be used to build much more powerful abstractions.
Apache have Java and C interfaces to Zoo Keeper for the applications themselves. A variety of client bindings is available for a number of languages including Python, Ruby and Go.
https://cwiki.apache.org/confluence/display/ZOOKEEPER/Index</skos:definition>
        <skos:narrower rdf:resource="http://data.europa.eu/dr8/InteroperableEuropeanSolutionService"/>
    </skos:Concept>

    <skos:Concept rdf:about="http://data.europa.eu/dr8/ServiceRegistryComponent">
        <skos:notation>ServiceRegistryComponent</skos:notation>
        <skos:prefLabel xml:lang="en">[ABB133] Service Registry Component</skos:prefLabel>
        <skos:definition xml:lang="en">DESCRIPTION:
Implements the functionality of registering the system service within a catalogue to be discovered by other services.
This ABB is a key interoperability enabler (*) for sharing/PROVISIONING and reusing/CONSUMING back-office services.

Source ISA2 - EIA Action

(*)DECISION (EU) 2015/2240 OF THE EUROPEAN PARLIAMENT AND OF THE COUNCIL of 25 November 2015 establishing a programme on interoperability solutions and common frameworks for European public administrations, businesses and citizens (ISA2 programme) as a means for modernising the public sector.

Syn. Service Catalogue Component

INTEROPERABILITY SALIENCY:
IoP Dimension: Structural IoP

The Service Registration Component ABB is a key interoperability enabler because it supports to achieve technical interoperability by provisioning and consuming back-office services as stated in the EIF recommendation n44: &quot;Put in place catalogues of public services, public data, and interoperability solutions and use common models for describing them.&quot;

EXAMPLES:
The following implementation is an example on how this specific Architecture Building Block (ABB) can be instantiated as a Solution Building Block (SBB):

jUDDI
jUDDI is an open source Java implementation of OASIS Universal Description, Discovery, and Integration (UDDI) specification for (Web) Services.
https://juddi.apache.org/</skos:definition>
        <skos:topConceptOf rdf:resource="http://data.europa.eu/dr8"/>
    </skos:Concept>

    <skos:Concept rdf:about="http://data.europa.eu/dr8/MachineTranslationService">
        <skos:notation>MachineTranslationService</skos:notation>
        <skos:prefLabel xml:lang="en">[ABB41] Machine Translation Service</skos:prefLabel>
        <skos:definition xml:lang="en">DESCRIPTION:
Shares the functionality of serving any current or future Digital Service Infrastructure (DSI) requiring cross-lingual functionality. The main functionality is automated translation of text, metadata and concept classes or nomenclatures.

Based on CEF Automated Translation
https://ec.europa.eu/digital-single-market/en/news/tools-and-resources-cef-automated-translation

INTEROPERABILITY SALIENCY:
IoP Dimension: Behavioral IoP
The Machine Translation Service ABB is salient for technical interoperability because it enables cross-lingual functionality by providing automated  translation of text, metadata and concept classes or nomenclatures as stated in the EIF recommendation n16: &quot;Use information systems and technical architectures that cater for multilingualism when establishing a European public service. Decide on the level of multilingualism support based on the needs of the expected users.&quot;

EXAMPLES:
The following implementation is an example on how this specific Architecture Building Block (ABB) can be instantiated as a Solution Building Block (SBB):

CEF Digital - eTranslation building block
eTranslation is a Connecting Europe Facility (CEF) building block provided by the European Commission (EC). eTranslation provides an online machine translation service.
https://ec.europa.eu/cefdigital/wiki/display/CEFDIGITAL/eTranslation &quot;</skos:definition>
        <skos:narrower rdf:resource="http://data.europa.eu/dr8/InteroperableEuropeanSolutionService"/>
    </skos:Concept>

    <skos:Concept rdf:about="http://data.europa.eu/dr8/MachineTranslationComponent">
        <skos:notation>MachineTranslationComponent</skos:notation>
        <skos:prefLabel xml:lang="en">[ABB62] Machine Translation Component</skos:prefLabel>
        <skos:definition xml:lang="en">DESCRIPTION:
Implements the functionality of serving any current or future Digital Service Infrastructure (DSI) requiring cross-lingual functionality. The main functionality is automated translation of text, metadata and concept classes or nomenclatures.

Based on CEF Automated Translation
https://ec.europa.eu/digital-single-market/en/news/tools-and-resources-cef-automated-translation

INTEROPERABILITY SALIENCY:
IoP Dimension: Structural IoP

The Machine Translation Component ABB is salient for technical interoperability because it provides the implementation of functionalities for cross-lingual functionality by providing automated  translation of text, metadata and concept classes or nomenclatures as stated in the EIF recommendation n16: &quot;Use information systems and technical architectures that cater for multilingualism when establishing a European public service. Decide on the level of multilingualism support based on the needs of the expected users.&quot;

EXAMPLES:
The following implementation is an example on how this specific Architecture Building Block (ABB) can be instantiated as a Solution Building Block (SBB):

&quot;CEF Digital - eTranslation building block
eTranslation is a Connecting Europe Facility (CEF) building block provided by the European Commission (EC). eTranslation provides a web-user interface for direct use by individuals (human-to-machine).
https://ec.europa.eu/cefdigital/wiki/display/CEFDIGITAL/eTranslation &quot;</skos:definition>
        <skos:topConceptOf rdf:resource="http://data.europa.eu/dr8"/>
    </skos:Concept>

    <skos:Concept rdf:about="http://data.europa.eu/dr8/E-signatureCreationService">
        <skos:notation>E-signatureCreationService</skos:notation>
        <skos:prefLabel xml:lang="en">[ABB55] e-Signature Creation Service</skos:prefLabel>
        <skos:definition xml:lang="en">DESCRIPTION:
Shares the functionality of signing data in electronic form by a natural person.
An electronic signature means data in electronic form which is attached to or logically associated with other data in electronic form and which is used by the signatory to sign.

Based on eIDAS - REGULATION (EU) No 910/2014 OF THE EUROPEAN PARLIAMENT AND OF THE COUNCIL of 23 July 2014 on electronic identification and trust services for electronic transactions in the internal market and repealing Directive 1999/93/EC.
http://eur-lex.europa.eu/legal-content/EN/TXT/?uri=uriserv%3AOJ.L_.2014.257.01.0073.01.ENG

INTEROPERABILITY SALIENCY:
IoP Dimension: Behavioral IoP
The e-Signature Creation Service ABB is salient for technical interoperability because it provides
the functionalities required for e-signature creation service.

EXAMPLES:
The following implementation is an example on how this specific Architecture Building Block (ABB) can be instantiated as a Solution Building Block (SBB):

CEF eSignature DSS
DSS (Digital Signature Services) is an open-source software library for electronic signature creation and validation. DSS supports the creation and verification of interoperable and secure electronic signatures in line with European legislation. In particular, DSS aims to follow the eIDAS Regulation and related standards closely.
DSS can be re-used in an IT solution for electronic signatures to ensure that signatures are created and verified in line with European legislation and standards. DSS allows re-use in a variety of different ways: in an applet, in a stand-alone application or in a server application. DSS can also be used as a reference implementation for IT solutions which do not directly re-use it.
CEF eSignature&apos;s DSS open-source library delivers the following benefits to its users:
	Open-source software under LGPL 2.1, a non-viral open source license;
	Interoperability of the e-signatures;
	Supports both e-signatures and e-seals;
	Validation of countersignatures and multiple signatures;
	Alignment with the eIDAS Regulation and related standards;
	Supports EU standards on:
o	Signature formats and packaging methods;
o	Signature validation procedures;
	Validation relying on Member States&apos; trusted lists:
o	Status of trust service providers/trust service, compensation of information, path validation.
https://ec.europa.eu/cefdigital/wiki/display/CEFDIGITAL/eSignature</skos:definition>
        <skos:narrower rdf:resource="http://data.europa.eu/dr8/InteroperableEuropeanSolutionService"/>
    </skos:Concept>

    <skos:Concept rdf:about="http://data.europa.eu/dr8/E-signatureVerificationAndValidationService">
        <skos:notation>E-signatureVerificationAndValidationService</skos:notation>
        <skos:prefLabel xml:lang="en">[ABB144] e-Signature Verification and Validation Service</skos:prefLabel>
        <skos:definition xml:lang="en">DESCRIPTION:
Shares the functionality of the verification of documents that are signed electronically.
An electronic signature means data in electronic form which is attached to or logically associated with other data in electronic form and which is used by the signatory to sign.
validation means the process of verifying and confirming that an electronic signature or a seal is valid.

Based on eIDAS - REGULATION (EU) No 910/2014 OF THE EUROPEAN PARLIAMENT AND OF THE COUNCIL of 23 July 2014 on electronic identification and trust services for electronic transactions in the internal market and repealing Directive 1999/93/EC.
http://eur-lex.europa.eu/legal-content/EN/TXT/?uri=uriserv%3AOJ.L_.2014.257.01.0073.01.ENG

INTEROPERABILITY SALIENCY:
IoP Dimension: Behavioral IoP
The e-Signature Verification and Validation Service ABB is salient for technical interoperability because it provides
the functionalities required for  e-signature verification and validation service.

EXAMPLES:
The following implementation is an example on how this specific Architecture Building Block (ABB) can be instantiated as a Solution Building Block (SBB):

CEF eSignature DSS
DSS (Digital Signature Services) is an open-source software library for electronic signature creation and validation. DSS supports the creation and verification of interoperable and secure electronic signatures in line with European legislation. In particular, DSS aims to follow the eIDAS Regulation and related standards closely.
DSS can be re-used in an IT solution for electronic signatures to ensure that signatures are created and verified in line with European legislation and standards. DSS allows re-use in a variety of different ways: in an applet, in a stand-alone application or in a server application. DSS can also be used as a reference implementation for IT solutions which do not directly re-use it.
CEF eSignature&apos;s DSS open-source library delivers the following benefits to its users:
	Open-source software under LGPL 2.1, a non-viral open source license;
	Interoperability of the e-signatures;
	Supports both e-signatures and e-seals;
	Validation of countersignatures and multiple signatures;
	Alignment with the eIDAS Regulation and related standards;
	Supports EU standards on:
o	Signature formats and packaging methods;
o	Signature validation procedures;
	Validation relying on Member States&apos; trusted lists:
o	Status of trust service providers/trust service, compensation of information, path validation.
https://ec.europa.eu/cefdigital/wiki/display/CEFDIGITAL/eSignature</skos:definition>
        <skos:narrower rdf:resource="http://data.europa.eu/dr8/InteroperableEuropeanSolutionService"/>
    </skos:Concept>

    <skos:Concept rdf:about="http://data.europa.eu/dr8/E-signaturePreservationService">
        <skos:notation>E-signaturePreservationService</skos:notation>
        <skos:prefLabel xml:lang="en">[ABB197] e-Signature Preservation Service</skos:prefLabel>
        <skos:definition xml:lang="en">DESCRIPTION:
Shares the functionality of extending the trustworthiness of the qualified electronic signature beyond the technological validity period.
An electronic signature means data in electronic form which is attached to or logically associated with other data in electronic form and which is used by the signatory to sign.

Based on eIDAS - REGULATION (EU) No 910/2014 OF THE EUROPEAN PARLIAMENT AND OF THE COUNCIL of 23 July 2014 on electronic identification and trust services for electronic transactions in the internal market and repealing Directive 1999/93/EC.
http://eur-lex.europa.eu/legal-content/EN/TXT/?uri=uriserv%3AOJ.L_.2014.257.01.0073.01.ENG

Syn. e-Signature Archiving Service

INTEROPERABILITY SALIENCY:
IoP Dimension: Behavioral IoP
The e-Signature Preservation Service ABB is salient for technical interoperability because it provides
the functionalities required for e-signature preservation service.

EXAMPLES:
The following implementation is an example on how this specific Architecture Building Block (ABB) can be instantiated as a Solution Building Block (SBB):

Namirial Spa Long term archiving solution
Namirial is a Trust Service Provider, focused on addressing the fast growing market of Digital Transaction Management (DTM), which includes legally compliant electronic signatures, managing and tracking documents flows, conducting secure transactions and ensuring secure storage of data.
It provides a long term archiving:
	Protect and preserve all documents generated while performing digital business transactions
	Make those documents easily searchable
	Accredited for Long-Term Archiving/Digital Preservation Services
	SaaS, high-availability, multi-company solution built to archive large volumes of documents
https://www.xyzmo.com/digital-signature/e-signature-products</skos:definition>
        <skos:narrower rdf:resource="http://data.europa.eu/dr8/InteroperableEuropeanSolutionService"/>
    </skos:Concept>

    <skos:Concept rdf:about="http://data.europa.eu/dr8/E-sealCreationService">
        <skos:notation>E-sealCreationService</skos:notation>
        <skos:prefLabel xml:lang="en">[ABB198] e-Seal Creation Service</skos:prefLabel>
        <skos:definition xml:lang="en">DESCRIPTION:
Shares the functionality of signing data in electronic forms on behalf of a legal person.
An electronic seal&apos; means data in electronic form, which is attached to or logically associated with other data in electronic form to ensure the latters origin and integrity. The creator of a seal is a legal person who creates an electronic seal.

Based on eIDAS - REGULATION (EU) No 910/2014 OF THE EUROPEAN PARLIAMENT AND OF THE COUNCIL of 23 July 2014 on electronic identification and trust services for electronic transactions in the internal market and repealing Directive 1999/93/EC.
http://eur-lex.europa.eu/legal-content/EN/TXT/?uri=uriserv%3AOJ.L_.2014.257.01.0073.01.ENG

INTEROPERABILITY SALIENCY:
IoP Dimension: Behavioral IoP
The e-Seal Creation Service ABB is salient for technical interoperability because it provides
the functionalities required for e-seal creation service.

EXAMPLES:
The following implementation is an example on how this specific Architecture Building Block (ABB) can be instantiated as a Solution Building Block (SBB):

CEF eSignature DSS
DSS (Digital Signature Services) is an open-source software library for electronic signature creation and validation. DSS supports the creation and verification of interoperable and secure electronic signatures in line with European legislation. In particular, DSS aims to follow the eIDAS Regulation and related standards closely.
DSS can be re-used in an IT solution for electronic signatures to ensure that signatures are created and verified in line with European legislation and standards. DSS allows re-use in a variety of different ways: in an applet, in a stand-alone application or in a server application. DSS can also be used as a reference implementation for IT solutions which do not directly re-use it.
CEF eSignature&apos;s DSS open-source library delivers the following benefits to its users:
	Open-source software under LGPL 2.1, a non-viral open source license;
	Interoperability of the e-signatures;
	Supports both e-signatures and e-seals;
	Validation of countersignatures and multiple signatures;
	Alignment with the eIDAS Regulation and related standards;
	Supports EU standards on:
o	Signature formats and packaging methods;
o	Signature validation procedures;
	Validation relying on Member States&apos; trusted lists:
o	Status of trust service providers/trust service, compensation of information, path validation.
https://ec.europa.eu/cefdigital/wiki/display/CEFDIGITAL/eSignaturefile:///C:/Users/bocquilp/Downloads/DSS(ServiceOfferingDescription)%20(v0.03)%20(5).pdf</skos:definition>
        <skos:narrower rdf:resource="http://data.europa.eu/dr8/InteroperableEuropeanSolutionService"/>
    </skos:Concept>

    <skos:Concept rdf:about="http://data.europa.eu/dr8/E-sealVerificationAndValidationService">
        <skos:notation>E-sealVerificationAndValidationService</skos:notation>
        <skos:prefLabel xml:lang="en">[ABB199] e-Seal Verification and Validation Service</skos:prefLabel>
        <skos:definition xml:lang="en">DESCRIPTION:
Shares the functionality of the verification of documents that are signed electronically.
An electronic seal&apos; means data in electronic form, which is attached to or logically associated with other data in electronic form to ensure the latters origin and integrity. The creator of a seal is a legal person who creates an electronic seal.

Based on eIDAS - REGULATION (EU) No 910/2014 OF THE EUROPEAN PARLIAMENT AND OF THE COUNCIL of 23 July 2014 on electronic identification and trust services for electronic transactions in the internal market and repealing Directive 1999/93/EC.
http://eur-lex.europa.eu/legal-content/EN/TXT/?uri=uriserv%3AOJ.L_.2014.257.01.0073.01.ENG

INTEROPERABILITY SALIENCY:
IoP Dimension: Behavioral IoP
The e-Seal Verification and Validation Service ABB is salient for technical interoperability because it provides
the functionalities required for e-seal verification and validation service.

EXAMPLES:
The following implementation is an example on how this specific Architecture Building Block (ABB) can be instantiated as a Solution Building Block (SBB):

CEF eSignature DSS
DSS (Digital Signature Services) is an open-source software library for electronic signature creation and validation. DSS supports the creation and verification of interoperable and secure electronic signatures in line with European legislation. In particular, DSS aims to follow the eIDAS Regulation and related standards closely.
DSS can be re-used in an IT solution for electronic signatures to ensure that signatures are created and verified in line with European legislation and standards. DSS allows re-use in a variety of different ways: in an applet, in a stand-alone application or in a server application. DSS can also be used as a reference implementation for IT solutions which do not directly re-use it.
CEF eSignature&apos;s DSS open-source library delivers the following benefits to its users:
	Open-source software under LGPL 2.1, a non-viral open source license;
	Interoperability of the e-signatures;
	Supports both e-signatures and e-seals;
	Validation of countersignatures and multiple signatures;
	Alignment with the eIDAS Regulation and related standards;
	Supports EU standards on:
o	Signature formats and packaging methods;
o	Signature validation procedures;
	Validation relying on Member States&apos; trusted lists:
o	Status of trust service providers/trust service, compensation of information, path validation.
https://ec.europa.eu/cefdigital/wiki/display/CEFDIGITAL/eSignaturefile:///C:/Users/bocquilp/Downloads/DSS(ServiceOfferingDescription)%20(v0.03)%20(5).pdf</skos:definition>
        <skos:narrower rdf:resource="http://data.europa.eu/dr8/InteroperableEuropeanSolutionService"/>
    </skos:Concept>

    <skos:Concept rdf:about="http://data.europa.eu/dr8/E-sealPreservationService">
        <skos:notation>E-sealPreservationService</skos:notation>
        <skos:prefLabel xml:lang="en">[ABB200] e-Seal Preservation Service</skos:prefLabel>
        <skos:definition xml:lang="en">DESCRIPTION:
Shares the functionality of extending the trustworthiness of the qualified electronic signature beyond the technological validity period.
An electronic seal&apos; means data in electronic form, which is attached to or logically associated with other data in electronic form to ensure the latters origin and integrity. The creator of a seal is a legal person who creates an electronic seal.

Based on eIDAS - REGULATION (EU) No 910/2014 OF THE EUROPEAN PARLIAMENT AND OF THE COUNCIL of 23 July 2014 on electronic identification and trust services for electronic transactions in the internal market and repealing Directive 1999/93/EC.
http://eur-lex.europa.eu/legal-content/EN/TXT/?uri=uriserv%3AOJ.L_.2014.257.01.0073.01.ENG

Syn. e-Seal Archiving Service

INTEROPERABILITY SALIENCY:
IoP Dimension: Behavioral IoP
The e-Seal Preservation Service ABB is salient for technical interoperability  because it provides
the functionalities required for e-seal preservation service.

EXAMPLES:
The following implementation is an example on how this specific Architecture Building Block (ABB) can be instantiated as a Solution Building Block (SBB):

CEF eSignature DSS
DSS (Digital Signature Services) is an open-source software library for electronic signature creation and validation. DSS supports the creation and verification of interoperable and secure electronic signatures in line with European legislation. In particular, DSS aims to follow the eIDAS Regulation and related standards closely.
DSS can be re-used in an IT solution for electronic signatures to ensure that signatures are created and verified in line with European legislation and standards. DSS allows re-use in a variety of different ways: in an applet, in a stand-alone application or in a server application. DSS can also be used as a reference implementation for IT solutions which do not directly re-use it.
CEF eSignature&apos;s DSS open-source library delivers the following benefits to its users:
	Open-source software under LGPL 2.1, a non-viral open source license;
	Interoperability of the e-signatures;
	Supports both e-signatures and e-seals;
	Validation of countersignatures and multiple signatures;
	Alignment with the eIDAS Regulation and related standards;
	Supports EU standards on:
o	Signature formats and packaging methods;
o	Signature validation procedures;
	Validation relying on Member States&apos; trusted lists:
o	Status of trust service providers/trust service, compensation of information, path validation.
https://ec.europa.eu/cefdigital/wiki/display/CEFDIGITAL/eSignaturefile:///C:/Users/bocquilp/Downloads/DSS(ServiceOfferingDescription)%20(v0.03)%20(5).pdf</skos:definition>
        <skos:narrower rdf:resource="http://data.europa.eu/dr8/InteroperableEuropeanSolutionService"/>
    </skos:Concept>

    <skos:Concept rdf:about="http://data.europa.eu/dr8/E-timestampCreationService">
        <skos:notation>E-timestampCreationService</skos:notation>
        <skos:prefLabel xml:lang="en">[ABB201] e-Timestamp Creation Service</skos:prefLabel>
        <skos:definition xml:lang="en">DESCRIPTION:
Shares the functionality of the verification of timestamps used for establishing evidence that a give piece of data existed at a given point in time.
An electronic time stamp means data in electronic form which binds other data in electronic form to a particular time establishing evidence that the latter data existed at that time.

Based on eIDAS - REGULATION (EU) No 910/2014 OF THE EUROPEAN PARLIAMENT AND OF THE COUNCIL of 23 July 2014 on electronic identification and trust services for electronic transactions in the internal market and repealing Directive 1999/93/EC.
http://eur-lex.europa.eu/legal-content/EN/TXT/?uri=uriserv%3AOJ.L_.2014.257.01.0073.01.ENG

Syn. eTS Creation Service

INTEROPERABILITY SALIENCY:
IoP Dimension: Behavioral IoP
The e-Timestamp Creation Service ABB is salient for technical interoperability because it provides
the functionalities required for e-Timestamp creation service.

EXAMPLES:
The following implementation is an example on how this specific Architecture Building Block (ABB) can be instantiated as a Solution Building Block (SBB):
DigiStamp eTimeStamp
DigiStamp eTimeStamp protects the intellectual property in any computer file:
	Use Desktop and Web applications for on-demand protection
	Plug the Timestamp Authority into the automated systems
Plug-in rigorous implementation of US &amp; EU standards:
	Secure, reliable, RFC 3161 timestamp cloud service
	Archiving and Hash Chaining keyless security
	Elliptic Curve Upgrade
Implementation of the Internet Engineering Task Force&apos;s RFC 3161 means DigiStamp timestamps are understood by data validation systems the world over:
	Implementation of ANSI X9.95 further increases the compatibility of our timestamps.
	Compliance with IETF RFC 3628 gives credence to the trustworthiness of our Time Stamp Authorities.
	Conformance to IETF RFC 3126 makes our timestamps usable for long-term, legally binding agreements.
https://www.digistamp.com/

freeTSA.org offers free NTP and DNSCRYPT services
freeTSA.org provides a free Time Stamp Authority. Adding a trusted timestamp to code or to an electronic signature provides a digital seal of data integrity and a trusted date and time of when the transaction took place.
Trusted timestamping is the process of securely keeping track of the creation and modification times of a document. Security here means that no one - not even the owner of the document - should be able to change it once it has been recorded provided that the timestamper&apos;s integrity is never compromised. FreeTSA trusted timestamping Software as a Service (SaaS) provides an easy method to apply RFC 3161 trusted timestamps to time-sensitive transactions through independently verified and auditable date and UTC (Coordinated Universal Time) sources.
https://www.freetsa.org/index_en.php</skos:definition>
        <skos:narrower rdf:resource="http://data.europa.eu/dr8/InteroperableEuropeanSolutionService"/>
    </skos:Concept>

    <skos:Concept rdf:about="http://data.europa.eu/dr8/E-timestampVerificationAndValidationService">
        <skos:notation>E-timestampVerificationAndValidationService</skos:notation>
        <skos:prefLabel xml:lang="en">[ABB202] e-Timestamp Verification and Validation Service</skos:prefLabel>
        <skos:definition xml:lang="en">DESCRIPTION:
Shares the functionality of the verification of timestamps used for establishing evidence that a give piece of data existed at a given point in time.
An electronic time stamp means data in electronic form which binds other data in electronic form to a particular time establishing evidence that the latter data existed at that time.

Based on eIDAS - REGULATION (EU) No 910/2014 OF THE EUROPEAN PARLIAMENT AND OF THE COUNCIL of 23 July 2014 on electronic identification and trust services for electronic transactions in the internal market and repealing Directive 1999/93/EC.
http://eur-lex.europa.eu/legal-content/EN/TXT/?uri=uriserv%3AOJ.L_.2014.257.01.0073.01.ENG

Syn. eTS Verification and Validation Service

INTEROPERABILITY SALIENCY:
IoP Dimension: Behavioral IoP
The e-Timestamp Verification and Validation Service ABB is salient for technical interoperability because it provides
the functionalities required for e-timestamp verification and validation service.

EXAMPLES:
The following implementation is an example on how this specific Architecture Building Block (ABB) can be instantiated as a Solution Building Block (SBB):
OpenSSL timestamp verification
OpenSSL is an open-source tool that can be used to retrieve and verify digital timestamps.
https://wiki.openssl.org/index.php/Manual:Ts(1)
https://www.digistamp.com/technical/software-alternatives/using-openssl-to-request-timestamps/</skos:definition>
        <skos:narrower rdf:resource="http://data.europa.eu/dr8/InteroperableEuropeanSolutionService"/>
    </skos:Concept>

    <skos:Concept rdf:about="http://data.europa.eu/dr8/RegisteredElectronicDeliveryService">
        <skos:notation>RegisteredElectronicDeliveryService</skos:notation>
        <skos:prefLabel xml:lang="en">[ABB203] Registered Electronic Delivery Service</skos:prefLabel>
        <skos:definition xml:lang="en">DESCRIPTION:
Shares the functionalities that i) makes it possible to transmit data between third parties by electronic means and ii) provides evidence relating to the handling of the transmitted data, including proof of sending and receiving the data, and iii) that protects transmitted data against the risk of loss, theft, damage or any unauthorised alterations;

Based on eIDAS - REGULATION (EU) No 910/2014 OF THE EUROPEAN PARLIAMENT AND OF THE COUNCIL of 23 July 2014 on electronic identification and trust services for electronic transactions in the internal market and repealing Directive 1999/93/EC.
http://eur-lex.europa.eu/legal-content/EN/TXT/?uri=uriserv%3AOJ.L_.2014.257.01.0073.01.ENG

INTEROPERABILITY SALIENCY:
IoP Dimension: Behavioral IoP
The Registered Electronic Delivery Service ABB is salient for technical interoperability because it provides  the functionalities related to the handling of data transmission.

EXAMPLES:
The following implementation is an example on how this specific Architecture Building Block (ABB) can be instantiated as a Solution Building Block (SBB):

Qualified electronic registered delivery services listed with CEF Trusted List Browser tool
Qualified electronic registered delivery services are listed on https://webgate.ec.europa.eu/tl-browser/#/search/1
https://webgate.ec.europa.eu/tl-browser/#/search/1</skos:definition>
        <skos:narrower rdf:resource="http://data.europa.eu/dr8/InteroperableEuropeanSolutionService"/>
    </skos:Concept>

    <skos:Concept rdf:about="http://data.europa.eu/dr8/TrustServiceProvisioningComponent">
        <skos:notation>TrustServiceProvisioningComponent</skos:notation>
        <skos:prefLabel xml:lang="en">[ABB69] Trust Service Provisioning Component</skos:prefLabel>
        <skos:definition xml:lang="en">DESCRIPTION:
Implements the functionalities encapsulating the trust services functionalities.
A trust service means an electronic service normally provided for remuneration which consists of these functionalities:
i) the creation, verification, and validation of electronic signatures, electronic seals or electronic time stamps, electronic registered delivery services and certificates related to those services, or
ii) the creation, verification and validation of certificates for website authentication; or
iii) the preservation of electronic signatures, seals or certificates related to those services.

Based on eIDAS - REGULATION (EU) No 910/2014 OF THE EUROPEAN PARLIAMENT AND OF THE COUNCIL of 23 July 2014 on electronic identification and trust services for electronic transactions in the internal market and repealing Directive 1999/93/EC.
http://eur-lex.europa.eu/legal-content/EN/TXT/?uri=uriserv%3AOJ.L_.2014.257.01.0073.01.ENG

INTEROPERABILITY SALIENCY:
IoP Dimension: Structural IoP
The Trust Service Provisioning Component ABB is salient for technical interoperability  because it provides
the implementation of the functionalities of information exchange between between administrations, businesses and citizens (e-signature and e-seal creation, verification,validation and preservation, timestamping  creation, verification and validation, identity management, etc.) as stated in the EIF recommendation n47: &quot;Use trust services according to the Regulation on eID and Trust Services as mechanisms that ensure secure and protected data exchange in public services.&quot;

EXAMPLES:
The following implementation is an example on how this specific Architecture Building Block (ABB) can be instantiated as a Solution Building Block (SBB):

e-TrustEx
Open e-TrustEx is a platform offered by the Directorate-General for Informatics of the European Commission to Public Administrations at European, national and regional level to set up secure exchange of natively digital documents from system to system via standardized interfaces. Open e-TrustEx provides a set of generic web services, which Public Administrations can use to connect heterogeneous applications, removing the need for complex point-to-point connections.
http://eur-lex.europa.eu/legal-content/DE/TXT/?uri=CELEX%3A52016SC0279
https://joinup.ec.europa.eu/solution/open-e-trustex</skos:definition>
        <skos:topConceptOf rdf:resource="http://data.europa.eu/dr8"/>
    </skos:Concept>

    <skos:Concept rdf:about="http://data.europa.eu/dr8/IdentityManagementService">
        <skos:notation>IdentityManagementService</skos:notation>
        <skos:prefLabel xml:lang="en">[ABB204] Identity Management Service</skos:prefLabel>
        <skos:definition xml:lang="en">DESCRIPTION:
Shares the functionality of user authentication.
Electronic identification means the process of using person identification data in electronic form uniquely representing either a natural or legal person, or a natural person representing a legal person;
Authentication means an electronic process that enables the electronic identification of a natural or legal person, or the origin and integrity of data in electronic form to be confirmed;

Based on eIDAS - REGULATION (EU) No 910/2014 OF THE EUROPEAN PARLIAMENT AND OF THE COUNCIL of 23 July 2014 on electronic identification and trust services for electronic transactions in the internal market and repealing Directive 1999/93/EC.
http://eur-lex.europa.eu/legal-content/EN/TXT/?uri=uriserv%3AOJ.L_.2014.257.01.0073.01.ENG

Syn. Authentication Service, eID

INTEROPERABILITY SALIENCY:
IoP Dimension: Behavioral IoP
The Identity Management Service ABB is salient for technical interoperability because it provides the functionalities of user authentication.

EXAMPLES:
The following implementation is an example on how this specific Architecture Building Block (ABB) can be instantiated as a Solution Building Block (SBB):

EU Login
EU Login is the European Commission&apos;s user authentication service. It allows authorised users to access a wide range of Commission web services. EU Login is the entry gate to sign in to different European Commission services and/or other systems. EU Login verifies your identity and allows recovering your personal settings, history and access rights in a secure way. You can sign in using social media accounts or the EU Login account.
EU Login supports a variety of verification methods:
	Password;
	ECAS Mobile App PIN code;
	ECAS Mobile App QR code;
	On mobile authentication;
	Mobile phone + SMS;
	Token and Token CRAM.
https://webgate.ec.europa.eu/cas/about.html
https://webgate.ec.europa.eu/cas/manuals/EU_Login_Tutorial_1.1.pdf

Federal Public Service Policy and Support - Federal Authentication Service (FAS)
Via the Federal Authentication Service (FAS) individuals are authenticated so that they can access secure online government applications.
Characteristics:
	Three different security levels depending on the sensitivity of the information: user name and password; user name, password and token; electronic identity card with associated PIN code.
	Authentication when connecting to an application
	Support with the implementation of the service
	Support while the service is being used
Attribute Publication Service:
	Collecting a users attributes from one or more reliable sources that are located in other government institutions (i.e., National Register, Crossroads Bank for Social Security and Crossroads Bank for Enterprises)
	Sending of the requested attributes to the requesting government application within the framework of a successful authentication
Users:
	All public services and institutions that want a secure authentication process for their applications: Federal public services and institutions; Communities and Regions; Provinces, municipalities and local public social welfare centres; businesses or persons implementing government contracts
Requirements:
	Application with Fedict Service Desk and signing up to a user agreement
http://www.fedict.belgium.be/en/identificatie_beveiliging/federal_authentication_service</skos:definition>
        <skos:narrower rdf:resource="http://data.europa.eu/dr8/InteroperableEuropeanSolutionService"/>
    </skos:Concept>

    <skos:Concept rdf:about="http://data.europa.eu/dr8/IdentityManagementComponent">
        <skos:notation>IdentityManagementComponent</skos:notation>
        <skos:prefLabel xml:lang="en">[ABB158] Identity Management Component</skos:prefLabel>
        <skos:definition xml:lang="en">DESCRIPTION:
Implements the functionality of user authentication.
Electronic identification means the process of using person identification data in electronic form uniquely representing either a natural or legal person, or a natural person representing a legal person;
Authentication means an electronic process that enables the electronic identification of a natural or legal person, or the origin and integrity of data in electronic form to be confirmed;

Based on eIDAS - REGULATION (EU) No 910/2014 OF THE EUROPEAN PARLIAMENT AND OF THE COUNCIL of 23 July 2014 on electronic identification and trust services for electronic transactions in the internal market and repealing Directive 1999/93/EC.
http://eur-lex.europa.eu/legal-content/EN/TXT/?uri=uriserv%3AOJ.L_.2014.257.01.0073.01.ENG

Syn. Authentication Component, eID

INTEROPERABILITY SALIENCY:
IoP Dimension: Structural IoP
The Identity Management Component ABB is salient for technical interoperability because it provides the functionalities of user authentication.

EXAMPLES:
The following implementation is an example on how this specific Architecture Building Block (ABB) can be instantiated as a Solution Building Block (SBB):

OpenIAM Identity Manager
The OpenIAM Identity Manager automates the task of managing identities across the various devices and applications used by the enterprise. This includes applications within the enterprise such as Active Directory and Exchange, and cloud based applications such as Google Apps.
OpenIAM Identity Manager provides capabilities such as:
	Provisioning, De-provisioning, Workflow
	Password Management, Password Policies, Synchronization
	Self-Service, allowing locked users to reset their accounts, manage their profiles, challenge response security questions
	Audit, Attestation, Reporting
	Delegated Administration
http://www.openiam.com/products/identity-manager/idm-overview/</skos:definition>
        <skos:topConceptOf rdf:resource="http://data.europa.eu/dr8"/>
    </skos:Concept>

    <skos:Concept rdf:about="http://data.europa.eu/dr8/TrustRegistryService">
        <skos:notation>TrustRegistryService</skos:notation>
        <skos:prefLabel xml:lang="en">[ABB145] Trust Registry Service</skos:prefLabel>
        <skos:definition xml:lang="en">DESCRIPTION:
Shares the functionality of the discovery of essential information about e.g. supervised/accredited trust service providers issuing certificates for electronic signatures, for electronic seals or for website authentication; supervised/accredited trust services for eSignature, eSeal or TimeStamp creation and validation; supervised/accredited trust services for eSignature or eSeal preservation; supervised/accredited trust services for electronic registered delivery.

Based on eIDAS - REGULATION (EU) No 910/2014 OF THE EUROPEAN PARLIAMENT AND OF THE COUNCIL of 23 July 2014 on electronic identification and trust services for electronic transactions in the internal market and repealing Directive 1999/93/EC.
http://eur-lex.europa.eu/legal-content/EN/TXT/?uri=uriserv%3AOJ.L_.2014.257.01.0073.01.ENG

Syn. Trusted List Service

INTEROPERABILITY SALIENCY:
IoP Dimension: Behavioral IoP
The Trust Registry Service ABB is salient for technical interoperability because it provides the functionalities of the discovery of essential information about accredited service providers.

EXAMPLES:
The following implementation is an example on how this specific Architecture Building Block (ABB) can be instantiated as a Solution Building Block (SBB):

BE:Trusted
BE:Trusted list including information related to the qualified trust service providers which are supervised by the issuing Member State, together with information related to the qualified trust services provided by them, in accordance with the relevant provisions laid down in Regulation (EU) No 910/2014 of the European Parliament and of the Council of 23 July 2014 on electronic identification and trust services for electronic transactions in the internal market.
https://tsl.belgium.be/archive/TSL-BE-2016-T3_vi5_sn27%20SPF%20Economie_signed.pdf</skos:definition>
        <skos:narrower rdf:resource="http://data.europa.eu/dr8/InteroperableEuropeanSolutionService"/>
    </skos:Concept>

    <skos:Concept rdf:about="http://data.europa.eu/dr8/TrustRegistryComponent">
        <skos:notation>TrustRegistryComponent</skos:notation>
        <skos:prefLabel xml:lang="en">[ABB146] Trust Registry Component</skos:prefLabel>
        <skos:definition xml:lang="en">DESCRIPTION:
Implements the functionality of the discovery of essential information about e.g. supervised/accredited trust service providers issuing certificates for electronic signatures, for electronic seals or for website authentication; supervised/accredited trust services for eSignature, eSeal or TimeStamp creation and validation; supervised/accredited trust services for eSignature or eSeal preservation; supervised/accredited trust services for electronic registered delivery.

Based on eIDAS - REGULATION (EU) No 910/2014 OF THE EUROPEAN PARLIAMENT AND OF THE COUNCIL of 23 July 2014 on electronic identification and trust services for electronic transactions in the internal market and repealing Directive 1999/93/EC.
http://eur-lex.europa.eu/legal-content/EN/TXT/?uri=uriserv%3AOJ.L_.2014.257.01.0073.01.ENG

Syn. Trusted List Component

INTEROPERABILITY SALIENCY:
IoP Dimension: Structural IoP
The Trust Registry Component ABB is salient for technical interoperability because it implements the functionalities of the discovery of essential information about accredited service providers.

EXAMPLES
The following implementation is an example on how this specific Architecture Building Block (ABB) can be instantiated as a Solution Building Block (SBB):

Trusted lists of all EU Member States
EU Member States have the obligation to establish, maintain and publish trusted lists of qualified trust service providers and the qualified trust services provided by them.
Under the Regulation (EC) No 910/2014/EU (eIDAS Regulation), national Trusted Lists have a constitutive effect. In other words, a trust service provider and the trust services it provides will be qualified only if it appears in the Trusted Lists. Consequently, the users (citizens, businesses or public administrations) will benefit from the legal effect associated with a given qualified trust service only if the latter is listed (as qualified) in the Trusted Lists.
Article 22 of the eIDAS Regulation provides indeed the obligation for Member States to establish, maintain and publish trusted lists, including information related to the qualified trust service providers for which they are responsible, together with information related to the qualified trust services provided by them. The lists are to be published in a secured manner, electronically signed or sealed in a form suitable for automated processing.
Trusted Lists are therefore essential in ensuring certainty and building trust among market operators as they indicate the status of the service provider and of the service at the moment of supervision, while aiming at fostering interoperability of qualified trust services by facilitating the validation of, among others, eSignatures and eSeals.
Member States may add trust services other than the qualified ones in the trusted lists, on a voluntary basis, at national level, provided that it is clearly indicated that they are not qualified according to Regulation (EU) No 910/2014.
In order to allow access to the trusted lists of all Member States, the Commission makes them available to the public, through a secure channel to an authenticated web server, the trusted lists as notified by Member States, in a signed or sealed form suitable for automated processing.
https://ec.europa.eu/digital-single-market/en/eu-trusted-lists-trust-service-providers
https://ec.europa.eu/information_society/policy/esignature/trusted-list/tl-mp.xml</skos:definition>
        <skos:topConceptOf rdf:resource="http://data.europa.eu/dr8"/>
    </skos:Concept>

    <skos:Concept rdf:about="http://data.europa.eu/dr8/DataExchangeService">
        <skos:notation>DataExchangeService</skos:notation>
        <skos:prefLabel xml:lang="en">[ABB43] Data Exchange Service</skos:prefLabel>
        <skos:definition xml:lang="en">DESCRIPTION:
Shares the functionality that enables the secure exchange of messages, records, forms and other kinds of data between different ICT systems. This includes data routing, except endpoint discovery.

Based on EIFv2
http://ec.europa.eu/isa/documents/isa_annex_ii_eif_en.pdf

INTEROPERABILITY SALIENCY:
IoP Dimension: Behavioral IoP
The Data Exchange Service ABB is salient for technical interoperability because it provides secure and trustworthy data exchange between different ICT systems as stated in the EIF: &quot;Define a common security and privacy framework and establish processes for public services to ensure secure and trustworthy data exchange between public administrations and in interactions with citizens and businesses.&quot;

EXAMPLES:
The following implementation is an example on how this specific Architecture Building Block (ABB) can be instantiated as a Solution Building Block (SBB):
XMLGate
XMLGate is a Web service application used to validate an XML instance against a well-defined schema. The XML flow is submitted either via a PDF form or by uploading the XML file.
https://webgate.ec.europa.eu/sanco-xmlgate/Login.jsp;jsessionid=2MPn_N5Wg9Dar4_W2-yVL_Xg-VlW3kn47PLVbNise9X5Kycx1yLI!-25226473</skos:definition>
        <skos:narrower rdf:resource="http://data.europa.eu/dr8/InteroperableEuropeanSolutionService"/>
    </skos:Concept>

    <skos:Concept rdf:about="http://data.europa.eu/dr8/DataExchangeComponent">
        <skos:notation>DataExchangeComponent</skos:notation>
        <skos:prefLabel xml:lang="en">[ABB64] Data Exchange Component</skos:prefLabel>
        <skos:definition xml:lang="en">DESCRIPTION:
Implements the functionality that enables the secure exchange of messages, records, forms and other kinds of data between different ICT systems. This includes data routing, except endpoint discovery.

Based on EIFv2
http://ec.europa.eu/isa/documents/isa_annex_ii_eif_en.pdf

INTEROPERABILITY SALIENCY:
IoP Dimension: Structural IoP
The Data Exchange Component ABB is salient for technical interoperability because it provides the implementation of the functionalities to enable a secure and trustworthy data exchange between different ICT systems as stated in the EIF: &quot;Define a common security and privacy framework and establish processes for public services to ensure secure and trustworthy data exchange between public administrations and in interactions with citizens and businesses.&quot;

EXAMPLES:
The following implementation is an example on how this specific Architecture Building Block (ABB) can be instantiated as a Solution Building Block (SBB):
Open e-TrustEx
Open e-TrustEx is a secure document exchange platform. Solution for European public administration that needs to electronically exchange information with other entities in a secure way. Open e-TrustEx is a cross-sector, open source tool that helps administrations to exchange structured and unstructured documents and to connect to pan-European e-delivery infrastructures with reduced investment. For Commission services, DG Informatics operates the e-TrustEx platform for a fee.
https://ec.europa.eu/isa2/solutions/open-e-trustex_en</skos:definition>
        <skos:topConceptOf rdf:resource="http://data.europa.eu/dr8"/>
    </skos:Concept>

    <skos:Concept rdf:about="http://data.europa.eu/dr8/HostingAndNetworkingInfrastructure">
        <skos:notation>HostingAndNetworkingInfrastructure</skos:notation>
        <skos:prefLabel xml:lang="en">[ABB190] Hosting and Networking Infrastructure</skos:prefLabel>
        <skos:definition xml:lang="en">DESCRIPTION:
Shares the functionalities for i) hosting Interoperable European Solutions and ii) providing the necessary networks for operating these solutions.

Source: ISA2 - EIA Action

INTEROPERABILITY SALIENCY:
IoP Dimension: Structural IoP
The Hosting and Infrastructure ABB is salient for technical interoperability because it provides all the functionalities to host the Interoperable European Solutions  (high availability and high performance hosting infrastructure) and the network where can operate these solutions (public and private network). Hosting and networking represent the lower level of the technical layer, but to be taken into account when design an interoperable solution, as it can create interoperability barriers. Interoperability technical specifications need to be used at this level to ensure interoperability of the levels above.

EXAMPLES:
The following implementation is an example on how this specific Architecture Building Block (ABB) can be instantiated as a Solution Building Block (SBB):

DIGIT Hosting and Networking Infrastructure Service
The mission of the Directorate General for Informatics (DIGIT) is to deliver digital services to enable EU policies and to support the Commission&apos;s internal administration.
Mission statement
With this goal in mind, DIGIT as trusted partner has the responsibility to:
	Provide the EC, and whenever appropriate other European Institutions and bodies, with high quality and innovative:
o	Workplace solutions  creating new ways of working and collaboration for staff;
o	Business solutions  delivering information systems supporting rationalised business processes within the framework of the corporate IT Governance strategy;
o	Infrastructure solutions  providing reliable, cost-effective and secure infrastructure and services;
o	Effective solutions  aligning IT investments with business priorities, facilitating relationships with our strategic partners, balancing risk with business value for the Institution.
	Support the modernisation of public administrations by promoting and facilitating interoperability so that European public administrations can work seamlessly together and with businesses and citizens across boundaries.
https://ec.europa.eu/info/sites/info/files/strategic-plan-2016-2020-dg-digit_march2016_en.pdf</skos:definition>
        <skos:topConceptOf rdf:resource="http://data.europa.eu/dr8"/>
    </skos:Concept>

    <skos:Concept rdf:about="http://data.europa.eu/dr8/PublicNetwork">
        <skos:notation>PublicNetwork</skos:notation>
        <skos:prefLabel xml:lang="en">[ABB94] Public Network</skos:prefLabel>
        <skos:definition xml:lang="en">DESCRIPTION:
A network that can be accessed by the public (public administrations, businesses and citizens) without specific authorisations. Interoperable European Solutions can rely on Public Networks (e.g. the Internet) to realise the physical communication between nodes.

Source: ISA2 - EIA Action

INTEROPERABILITY SALIENCY:
IoP Dimension: Structural IoP
The Public Network ABB is salient for technical interoperability because it provides  the public network where can operate interoperable solutions.

EXAMPLES:
The following implementation is an example on how this specific Architecture Building Block (ABB) can be instantiated as a Solution Building Block (SBB):

World-Wide-Web (WWW)
The WorldWideWeb (W3) is a wide-area hypermedia information retrieval initiative aiming to give universal access to a large universe of documents.
http://info.cern.ch/hypertext/WWW/TheProject.html</skos:definition>
        <skos:narrower rdf:resource="http://data.europa.eu/dr8/Network"/>
    </skos:Concept>

    <skos:Concept rdf:about="http://data.europa.eu/dr8/PrivateNetwork">
        <skos:notation>PrivateNetwork</skos:notation>
        <skos:prefLabel xml:lang="en">[ABB93] Private Network</skos:prefLabel>
        <skos:definition xml:lang="en">DESCRIPTION:
A network that is used for the only purpose of realising the physical communication among Interoperable European Solution (e.g. sTESTA), and cannot be accessed by the public.

Source: ISA2 - EIA Action

INTEROPERABILITY SALIENCY:
IoP Dimension: Structural IoP
The Private Network ABB is salient for technical interoperability because it provides  the private network where can operate interoperable solutions.

EXAMPLES:
The following implementation is an example on how this specific Architecture Building Block (ABB) can be instantiated as a Solution Building Block (SBB):

Any private network
Hosts within enterprises that use IP can be partitioned into two categories:
Category 1: hosts that do not require access to hosts in other enterprises or the Internet at large; hosts within this category may use IP addresses that are unambiguous within an enterprise, but may be ambiguous between enterprises.
Category 2: hosts that need access to a limited set of outside services (e.g., E-mail, FTP, netnews, remote login) which can be handled by mediating gateways (e.g., application layer gateways). For any hosts in this category an unrestricted external access (provided via IP connectivity) may be unnecessary and even undesirable for privacy/security reasons. Just like hosts within the first category, such hosts may use IP addresses that are unambiguous within an enterprise, but may be ambiguous between enterprises.
A third category is what is called a &apos;public network and consist of the following:
Category 3: hosts that need network layer access outside the enterprise (provided via IP connectivity); hosts in the last category require IP addresses that are globally unambiguous.
https://tools.ietf.org/html/rfc1918</skos:definition>
        <skos:narrower rdf:resource="http://data.europa.eu/dr8/Network"/>
    </skos:Concept>

    <skos:Concept rdf:about="http://data.europa.eu/dr8/Network">
        <skos:notation>Network</skos:notation>
        <skos:prefLabel xml:lang="en">[ABB92] Network</skos:prefLabel>
        <skos:definition xml:lang="en">DESCRIPTION:
Transmission systems and, where applicable, switching or routing equipment and other resources which permit the conveyance of signals by wire, by radio, by optical or by other electromagnetic means, including satellite networks, fixed (circuit- and packet- switched, including Internet) and mobile terrestrial networks, electricity cable systems, to the extent that they are used for the purpose of transmitting signals, networks used for radio and television broadcasting, and cable television networks, irrespective of the type of information conveyed.

Source: DIRECTIVE 2002/21/EC on a common regulatory framework for electronic communications networks and services
http://eur-lex.europa.eu/legal-content/EN/TXT/PDF/?uri=CELEX:32002L0021&amp;from=EN

INTEROPERABILITY SALIENCY:
IoP Dimension: Structural IoP
The Network ABB is salient for technical interoperability because it provides the network where can operate interoperable solutions (both public and private network).

EXAMPLES:
The following implementation is an example on how this specific Architecture Building Block (ABB) can be instantiated as a Solution Building Block (SBB):
sTESTA
The TESTA network service  which stands for Trans European Services for Telematics between Administrations  provides a European backbone network for data exchange between a wide variety of public administrations.
The network uses the Internet Protocols (IP) to ensure universal reach, but is operated by the EU Commission separately from the Internet. It provides guaranteed performance and a high level of security and has connections with all the EU Institutions and national networks. It caters for the exchange of both unclassified and classified information.
https://ec.europa.eu/isa2/solutions/testa_en</skos:definition>
        <skos:topConceptOf rdf:resource="http://data.europa.eu/dr8"/>
    </skos:Concept>

    <skos:Concept rdf:about="http://data.europa.eu/dr8/NetworkingService">
        <skos:notation>NetworkingService</skos:notation>
        <skos:prefLabel xml:lang="en">[ABB150] Networking Service</skos:prefLabel>
        <skos:definition xml:lang="en">DESCRIPTION:
Shares the functionalities provided by a network provider which is the combination of transmission systems and, where applicable, switching or routing equipment and other resources which permit the conveyance of signals by wire, by radio, by optical or by other electromagnetic means, including satellite networks, fixed (circuit- and packet- switched, including Internet) and mobile terrestrial networks, electricity cable systems, to the extent that they are used for the purpose of transmitting signals, networks used for radio and television broadcasting, and cable television networks, irrespective of the type of information conveyed.

Based on DIRECTIVE 2002/21/EC on a common regulatory framework for electronic communications networks and services
http://eur-lex.europa.eu/legal-content/EN/TXT/PDF/?uri=CELEX:32002L0021&amp;from=EN

INTEROPERABILITY SALIENCY:
IoP Dimension: Behavioural IoP
The Networking Service ABBis salient for technical interoperability because it provides all the required functionalities in order to create the suitable network underlayer    where can operate interoperable solutions.

EXAMPLES:
The following implementation is an example on how this specific Architecture Building Block (ABB) can be instantiated as a Solution Building Block (SBB):

sTESTA
The TESTA network service  which stands for Trans European Services for Telematics between Administrations  provides a European backbone network for data exchange between a wide variety of public administrations.
The network uses the Internet Protocols (IP) to ensure universal reach, but is operated by the EU Commission separately from the Internet. It provides guaranteed performance and a high level of security and has connections with all the EU Institutions and national networks. It caters for the exchange of both unclassified and classified information.
https://ec.europa.eu/isa2/solutions/testa_en</skos:definition>
        <skos:topConceptOf rdf:resource="http://data.europa.eu/dr8"/>
    </skos:Concept>

    <skos:Concept rdf:about="http://data.europa.eu/dr8/HostingService">
        <skos:notation>HostingService</skos:notation>
        <skos:prefLabel xml:lang="en">[ABB151] Hosting Service</skos:prefLabel>
        <skos:definition xml:lang="en">DESCRIPTION:
Shares the functionalities of a hosting provider, typically a high availability and high performance hosting infrastructure that is being comprised, among other elements, of back-end web server instances and application servers for hosting and serving both static and dynamic sites.

Based on DIGIT C Infrastructure Services Provision
http://ec.europa.eu/ipg/build/infrastructure/index_en.htm

INTEROPERABILITY SALIENCY:
IoP Dimension: Behavioural IoP
The Hosting Service ABB is salient for technical interoperability because it provides all the functionalities to host the Interoperable European Solutions  (high availability and high performance hosting infrastructure).

EXAMPLES:
The following implementation is an example on how this specific Architecture Building Block (ABB) can be instantiated as a Solution Building Block (SBB):

DIGIT/C Hosting Service
DIGIT/C offers a high availability and high performance hosting infrastructure that is being comprised, among other elements, of back-end web server instances and application servers for hosting and serving both static and dynamic sites.
http://ec.europa.eu/ipg/build/infrastructure/index_en.htm</skos:definition>
        <skos:topConceptOf rdf:resource="http://data.europa.eu/dr8"/>
    </skos:Concept>

    <skos:Concept rdf:about="http://data.europa.eu/dr8/HostingFacility">
        <skos:notation>HostingFacility</skos:notation>
        <skos:prefLabel xml:lang="en">[ABB191] Hosting Facility</skos:prefLabel>
        <skos:definition xml:lang="en">DESCRIPTION:
The equipment supporting the hosting of Interoperable European Solutions and their components, usually embodied in a building.

Based on DIGIT C Infrastructure Services Provision
http://ec.europa.eu/ipg/build/infrastructure/index_en.htm

INTEROPERABILITY SALIENCY:
IoP Dimension: Structural IoP
The Hosting Facility ABB is salient for technical interoperability because it provides all the equipment supporting the hosting of interaoperable solutions and their components.

EXAMPLES:
The following implementation is an example on how this specific Architecture Building Block (ABB) can be instantiated as a Solution Building Block (SBB):

DIGIT/C Hosting Facility
DIGIT/C offers a high availability and high performance hosting infrastructure that is being comprised, among other elements, of back-end web server instances and application servers for hosting and serving both static and dynamic sites.
The dynamic sites supported by the standard Apache web servers are mainly sites based on Coldfusion and in some cases also sites using CGI scripts.
Dynamic sites based on particular technologies (i.e. Weblogic) are being hosted on individual application servers and are being integrated with the other related sites using reverse proxy mappings.
Direct HTTP access to the back-end web servers hosting the static sites is denied by the standard web server configuration.
http://ec.europa.eu/ipg/build/infrastructure/index_en.htm</skos:definition>
        <skos:topConceptOf rdf:resource="http://data.europa.eu/dr8"/>
    </skos:Concept>

    <skos:Concept rdf:about="http://data.europa.eu/dr8/PublicHostingFacility">
        <skos:notation>PublicHostingFacility</skos:notation>
        <skos:prefLabel xml:lang="en">[ABB193] Public Hosting Facility</skos:prefLabel>
        <skos:definition xml:lang="en">DESCRIPTION:
The equipment supporting the hosting of Interoperable European Solutions and their components, usually embodied in a building, which is owned by a third party and shared between organizations (e.g. cloud services).

Based on DIGIT C Infrastructure Services Provision
http://ec.europa.eu/ipg/build/infrastructure/index_en.htm

INTEROPERABILITY SALIENCY:
IoP Dimension: Structural IoP
The Public Hosting Facility ABB is salient for technical interoperability because it provides all the equipment, shared between organizations, supporting the hosting of interaoperable solutions and their components.

EXAMPLES:

Amazon Web Services (AWS)
AWS provides a comprehensive suite of services and solutions to run sophisticated and scalable applications to help achieve better business outcomes. Running your applications in the AWS Cloud can help you move faster, operate more securely, and save substantial costs; all while benefitting from the agility, scale and performance of the cloud.
https://aws.amazon.com/solutions/?nc2=h_ql_sol</skos:definition>
        <skos:narrower rdf:resource="http://data.europa.eu/dr8/HostingFacility"/>
    </skos:Concept>

    <skos:Concept rdf:about="http://data.europa.eu/dr8/PrivateHostingFacility">
        <skos:notation>PrivateHostingFacility</skos:notation>
        <skos:prefLabel xml:lang="en">[ABB192] Private Hosting Facility</skos:prefLabel>
        <skos:definition xml:lang="en">DESCRIPTION:
A Hosting Facility, meaning the equipment supporting the hosting of Interoperable European Solutions and their components, usually embodied in a build-in, which is owned by or dedicated to one organization (e.g. data centre or private cloud).

Based on DIGIT C Infrastructure Services Provision
http://ec.europa.eu/ipg/build/infrastructure/index_en.htm

INTEROPERABILITY SALIENCY:
IoP Dimension: Structural IoP
The Private Hosting Facility ABB is salient for technical interoperability because it provides all the equipment, dedicated to one organization, supporting the hosting of interaoperable solutions and their components.

EXAMPLES:
The following implementation is an example on how this specific Architecture Building Block (ABB) can be instantiated as a Solution Building Block (SBB):

DG TAXUD Surveillance3 IES Datawarehouse servers hosted in DG TAXUD Data Centre
The Surveillance3 Data Warehouse plays multiple roles:
	The role of hub-and-spoke within the Surveillance3 system where data from different systems are integrated and linked and made available for report &amp; analytics as well as the central place from which other systems are fed with the correct information.
	The role of reporting environment offering all the required reporting, data analysis &amp; discovery and data mining functionality.
https://ec.europa.eu/assets/taxud/taxation_customs/tenders/2016ao02_a2_technical_en.pdf</skos:definition>
        <skos:narrower rdf:resource="http://data.europa.eu/dr8/HostingFacility"/>
    </skos:Concept>

    <skos:Concept rdf:about="http://data.europa.eu/dr8/ContentManagementService">
        <skos:notation>ContentManagementService</skos:notation>
        <skos:prefLabel xml:lang="en">[ABB380] Content Management Service</skos:prefLabel>
        <skos:definition xml:lang="en">DESCRIPTION:
A Content Management System (CMS) is responsible for:
- developing Website templates and functionalities
assigning appropriate user permissions and workflows
providing trainings to the web working group
- developing tools and web controls to speed up and facilitate the work of the web working group
-giving support and advice to the web working group
- ensuring continuity of service and performance
- ensuring security and accessibility on the website
- ensuring disaster recovery processes and backup procedures
- setting up the website information architecture within the CMS
- setting up alert procedures and analytics on usage of the platform.

Source: https://www.eui.eu/ServicesAndAdmin/CommunicationsService/WebUnit/Web-CMS

INTEROPERABILITY SALIENCY:
IoP Dimension: Behavioral IoP
The Content Management Service ABB is salient for technical interoperability because it provides and shares the functionalities of dynamic creation, distribution and analysis of contents (images, videos, etc.) as stated in the EIF: &quot; Catalogues help others to find reusable resources (e.g. services, data, software, data models). Various types of catalogue exist, e.g. directories of services, libraries of software components, open data portals, registries of base registries, metadata catalogues, catalogues of standards, specifications and guidelines. Commonly agreed descriptions of the services, data, registries and interoperable solutions published in catalogues are needed to enable interoperability between catalogues.&quot;

EXAMPLES:
FPFIS-CMS:
&quot;The European Commission announced in the Commission Internet strategy plans to transform the EUROPA web site from a source of one-way information into a tool for communication and interaction (i.e. provide modern interactive web sites for the citizens and stakeholders).
Web sites are a key tool for external communications. They are the institution&apos;s business card. Websites are a very cost-effective and efficient means of communication. EUROPA now hosts over 460 websites. EUROPA would benefit from fewer and better sites to respond to user needs. To address the shortcomings, as part of the Commission&apos;s IT governance process, the College on 30 November 2011, instructed Commission departments to rationalise the Institution&apos;s web presence.
Reduce the cost (human, financial, technical) of the Commission&apos;s web presence via exploiting economies of scale and eliminating redundancies by building corporate solutions. The European Commission should offer a corporate service which optimizes and harmonizes the use of different website tools, which speeds up the creation of new external dynamic and social websites (i.e. in days or weeks and not months) and which provides a common solid modern shared infrastructure to support the rapid deployment of these sites&quot;.

Source: https://webgate.ec.europa.eu/fpfis/mwikis/thinktank/index.php/Content_Management_System_of_the_Flexible_Platform</skos:definition>
        <skos:topConceptOf rdf:resource="http://data.europa.eu/dr8"/>
    </skos:Concept>

    <skos:Concept rdf:about="http://data.europa.eu/dr8/DataWarehouseService">
        <skos:notation>DataWarehouseService</skos:notation>
        <skos:prefLabel xml:lang="en">[ABB378] Data Warehouse Service</skos:prefLabel>
        <skos:definition xml:lang="en">DESCRIPTION:
A data warehouse is a central repository where raw data is transformed and stored in query-able forms. It is an information system that contains historical and commutative data from single or multiple sources. It simplifies reporting and analysis process of the organization.

INTEROPERABILITY SALIENCY:
IoP Dimension: Behavioral IoP
The Data Warehouse Service ABB is salient for technical interoperability because it provides and shares the functionality for the short-term or medium-term preservation of records and information in electronic form in order to ensure their temporal egibility, reliability and integrity and to ease their management as stated in the EIF: &quot;Legislation requires that decisions and data are stored and can be accessed for a specified time. This means that records and information in electronic form held by public administrations for the purpose of documenting procedures and decisions must be preserved and be converted, where necessary, to new media when old media become obsolete. The goal is to ensure that records and other forms of information keep their legibility, reliability and integrity and can be accessed as long as needed subject to security and privacy provisions.&quot;

EXAMPLES:
The following implementation is an example on how this specific Architecture Building Block (ABB) can be instantiated as a Solution Building Block (SBB):

ESSnet:
The overall objective of this ESSnet is to provide assistance in the development of more integrated databases and data production systems for business statistics in Member States. Therefore the ESSnet has to work on issues that are common for the majority of the ESS NSIs when applying a data warehousing approach for statistics.

Its general objectives are:
- Review of current best practices in integrated business data systems
- Identification of problems and solutions in current practices and the opportunities
that a data warehouse might provide
- Examination of ways in which data can be combined to support new outputs
- Provision of recommendations on how the ESS can improve data warehousing

Source: https://ec.europa.eu/eurostat/cros/content/data-warehouse-sga1_en</skos:definition>
        <skos:topConceptOf rdf:resource="http://data.europa.eu/dr8"/>
    </skos:Concept>

    <skos:Concept rdf:about="http://data.europa.eu/dr8/DataWarehouseComponent">
        <skos:notation>DataWarehouseComponent</skos:notation>
        <skos:prefLabel xml:lang="en">[ABB379] Data Warehouse Component</skos:prefLabel>
        <skos:definition xml:lang="en">DESCRIPTION:
A data warehouse Component is part of the central repository where raw data is transformed and stored in query-able forms. It is an information system that contains historical and commutative data from single or multiple sources. It simplifies reporting and analysis process of the organization.

INTEROPERABILITY SALIENCY:
IoP Dimension: Structural IoP
The Data Warehouse Component ABB is salient for technical interoperability because it provides and shares the functionality for the short-term or medium-term preservation of records and information in electronic form in order to ensure their temporal egibility, reliability and integrity and to ease their management as stated in the EIF: &quot;Legislation requires that decisions and data are stored and can be accessed for a specified time. This means that records and information in electronic form held by public administrations for the purpose of documenting procedures and decisions must be preserved and be converted, where necessary, to new media when old media become obsolete. The goal is to ensure that records and other forms of information keep their legibility, reliability and integrity and can be accessed as long as needed subject to security and privacy provisions.&quot;

EXAMPLES:
The following implementation is an example on how this specific Architecture Building Block (ABB) can be instantiated as a Solution Building Block (SBB):

ESSnet:
The overall objective of this ESSnet is to provide assistance in the development of more integrated databases and data production systems for business statistics in Member States. Therefore the ESSnet has to work on issues that are common for the majority of the ESS NSIs when applying a data warehousing approach for statistics.
Its general objectives are:
- Review of current best practices in integrated business data systems
- Identification of problems and solutions in current practices and the opportunities
that a data warehouse might provide
- Examination of ways in which data can be combined to support new outputs
- Provision of recommendations on how the ESS can improve data warehousing
Source: https://ec.europa.eu/eurostat/cros/content/data-warehouse-sga1_en</skos:definition>
        <skos:topConceptOf rdf:resource="http://data.europa.eu/dr8"/>
    </skos:Concept>

    <skos:Concept rdf:about="http://data.europa.eu/dr8/DataRepository">
        <skos:notation>DataRepository</skos:notation>
        <skos:prefLabel xml:lang="en">[ABB419] Data Repository</skos:prefLabel>
        <skos:definition xml:lang="en">DESCRIPTION:
A data repository can be defined as a place that holds data, makes data available to use, and organizes data in a logical manner. A data repository may also be defined as an appropriate, subject-specific location where researchers can submit their data. Data repositories may have specific requirements concerning subject or research domain; data re-use and access; file format and data structure; and the types of metadata that can be used.

Source: https://nnlm.gov/data/thesaurus/data-repository

INTEROPERABILITY SALIENCY:
IoP Dimension: Structural IoP
The Data Repository ABBis salient for technical interoperability because it provides a single trustworthy location to store and access the data. EIF recommendation 37 &quot;Make authoritative sources of information available to others while implementing access and control mechanisms to ensure security and privacy in accordance with the relevant legislation&quot;.

EXAMPLES:
The following implementation is an example on how this specific Architecture Building Block (ABB) can be instantiated as a Solution Building Block (SBB):

The Cancer Imanging Archive
TCIA is a service which de-identifies and hosts a large archive of medical images of cancer accessible for public download. The data are organized as collections; typically patients imaging related by a common disease (e.g. lung cancer), image modality or type (MRI, CT, digital histopathology, etc) or research focus. DICOM is the primary file format used by TCIA for radiology imaging. Supporting data related to the images such as patient outcomes, treatment details, genomics and expert analyses are also provided when available.

https://www.cancerimagingarchive.net/</skos:definition>
        <skos:topConceptOf rdf:resource="http://data.europa.eu/dr8"/>
    </skos:Concept>

    <skos:Concept rdf:about="http://data.europa.eu/dr8/DataAnalyticsService">
        <skos:notation>DataAnalyticsService</skos:notation>
        <skos:prefLabel xml:lang="en">[ABB420] Data Analytics Service</skos:prefLabel>
        <skos:definition xml:lang="en">DESCRIPTION:
Shares the functionalities of analysing a great amount of raw data in order to make conclusions about specific information. Data analytics services enable the automation of mechanical processes and algorithms that work over raw data for human consumption.

Source: https://www.investopedia.com/terms/d/data-analytics.asp

INTEROPERABILITY SALIENCY:
IoP Dimension: Behavioral IoP
The Data Analytics Service ABB is salient for technical interoperability because it enables the automated processing and analysis of different data source.

EXAMPLES:
The following implementation is an example on how this specific Architecture Building Block (ABB) can be instantiated as a Solution Building Block (SBB):

Microsoft Power BI
Power BI is a business analytics service by Microsoft. It aims to provide interactive visualizations and business intelligence capabilities with an interface simple enough for end users to create their own reports and dashboards. It is part of the Microsoft Power Platform.
https://powerbi.microsoft.com/it-it/what-is-power-bi/</skos:definition>
        <skos:topConceptOf rdf:resource="http://data.europa.eu/dr8"/>
    </skos:Concept>

    <skos:Concept rdf:about="http://data.europa.eu/dr8/DataAnalyticsComponent">
        <skos:notation>DataAnalyticsComponent</skos:notation>
        <skos:prefLabel xml:lang="en">[ABB421] Data Analytics Component</skos:prefLabel>
        <skos:definition xml:lang="en">DESCRIPTION:
Implements the functionality of serving any current or future Digital Service Infrastructure (DSI) requiring data analysis capabilities. Data analytics component enable the automation of mechanical processes and algorithms that work over raw data for human consumption.

INTEROPERABILITY SALIENCY:
IoP Dimension: Structural IoP
The Data Analytics Component ABB is salient for technical interoperability because it provides the implementation of functionalities for the automation of mechanical processes and algorithms that work over raw data for human consumption.

EXAMPLES:
The following implementation is an example on how this specific Architecture Building Block (ABB) can be instantiated as a Solution Building Block (SBB):

Microsoft Power BI
Power BI is a business analytics service by Microsoft. It aims to provide interactive visualizations and business intelligence capabilities with an interface simple enough for end users to create their own reports and dashboards. It is part of the Microsoft Power Platform.
https://powerbi.microsoft.com/it-it/what-is-power-bi/</skos:definition>
        <skos:topConceptOf rdf:resource="http://data.europa.eu/dr8"/>
    </skos:Concept>

    <skos:Concept rdf:about="http://data.europa.eu/dr8/ArtificialIntelligenceService">
        <skos:notation>ArtificialIntelligenceService</skos:notation>
        <skos:prefLabel xml:lang="en">[ABB422] Artificial Intelligence Service</skos:prefLabel>
        <skos:definition xml:lang="en">DESCRIPTION:
Shares the functionalities of appling advanced analysis and logic-based techniques, including machine learning, to interpret events, support and automate decisions, and take actions.

Source: https://www.gartner.com/en/information-technology/glossary/artificial-intelligence

INTEROPERABILITY SALIENCY:
IoP Dimension: Behavioral IoP
The Artificial intelligence Service ABB is salient for technical interoperability because it enables the application of advanced analysis and logic-based techniques, including machine learning, to interpret events, support and automate decisions, and take actions.

EXAMPLES:
The following implementation is an example on how this specific Architecture Building Block (ABB) can be instantiated as a Solution Building Block (SBB):

Google AI
A tool that enables scientists, data journalists, data geeks, or anyone else to easily find datasets stored in thousands of repositories across the web.
https://ai.google/#:~:text=A%20tool%20that%20enables%20scientists,of%20repositories%20across%20the%20web.&amp;text=We%20released%20a%20research%20framework,researchers%20to%20explore%20new%20ideas.</skos:definition>
        <skos:topConceptOf rdf:resource="http://data.europa.eu/dr8"/>
    </skos:Concept>

    <skos:Concept rdf:about="http://data.europa.eu/dr8/ArtificialIntelligenceComponent">
        <skos:notation>ArtificialIntelligenceComponent</skos:notation>
        <skos:prefLabel xml:lang="en">[ABB423] Artificial Intelligence Component</skos:prefLabel>
        <skos:definition xml:lang="en">DESCRIPTION:
Implements the functionality of serving any current or future Digital Service Infrastructure (DSI) requiring artificial intelligence capabilities. It enables the implementation of functionalities for appling advanced analysis and logic-based techniques, including machine learning, to interpret events, support and automate decisions, and take actions.

Source: https://www.gartner.com/en/information-technology/glossary/artificial-intelligence

INTEROPERABILITY SALIENCY:
IoP Dimension: Behavioral IoP
The Artificial intelligence Component ABB is salient for technical interoperability because it implements advanced analysis and logic-based techniques, including machine learning, to interpret events, support and automate decisions, and take actions.

EXAMPLES:
The following implementation is an example on how this specific Architecture Building Block (ABB) can be instantiated as a Solution Building Block (SBB):

Google AI
A tool that enables scientists, data journalists, data geeks, or anyone else to easily find datasets stored in thousands of repositories across the web.
https://ai.google/#:~:text=A%20tool%20that%20enables%20scientists,of%20repositories%20across%20the%20web.&amp;text=We%20released%20a%20research%20framework,researchers%20to%20explore%20new%20ideas.</skos:definition>
        <skos:topConceptOf rdf:resource="http://data.europa.eu/dr8"/>
    </skos:Concept>

    <skos:Concept rdf:about="http://data.europa.eu/dr8/SmartDevices">
        <skos:notation>SmartDevices</skos:notation>
        <skos:prefLabel xml:lang="en">[ABB424] Smart Devices</skos:prefLabel>
        <skos:definition xml:lang="en">DESCRIPTION:
Technological device means any computer, cellular phone, smartphone, digital camera, video camera, audio recording device, or other electronic device that can be used for creating, storing, or transmitting information in the form of electronic data.

Source: https://www.lawinsider.com/dictionary/technological-device

INTEROPERABILITY SALIENCY:
IoP Dimension: Not applicable

EXAMPLES:
The following implementation is an example on how this specific Architecture Building Block (ABB) can be instantiated as a Solution Building Block (SBB):

Digital blod pressures devices
Digital blood pressure monitors allow patients to seamlessly share their health data with physicians.</skos:definition>
        <skos:topConceptOf rdf:resource="http://data.europa.eu/dr8"/>
    </skos:Concept>

    <skos:Concept rdf:about="http://data.europa.eu/dr8/HighPerformanceInfrastructure">
        <skos:notation>HighPerformanceInfrastructure</skos:notation>
        <skos:prefLabel xml:lang="en">[ABB425] High Performance Infrastructure</skos:prefLabel>
        <skos:definition xml:lang="en">DESCRIPTION:
Shares the functionalities, through the use of computer clusters, to create computing systems capable of delivering very high performance in the range of PetaFLOPS, typically using parallel computing.

Source: Gartner

INTEROPERABILITY SALIENCY:
IoP Dimension: Structural IoP
The High Performance Infrastructure ABB is salient for technical interoperability because it provides all the functionalities to host the Interoperable European Solutions (high availability and high performance hosting infrastructure).

EXAMPLES:
The following implementation is an example on how this specific Architecture Building Block (ABB) can be instantiated as a Solution Building Block (SBB):

HPC AWS
The HPC of AWS provides the an elastic and scalable cloud infrastructure to run HPC applications.
https://aws.amazon.com/hpc/</skos:definition>
        <skos:topConceptOf rdf:resource="http://data.europa.eu/dr8"/>
    </skos:Concept>

    <skos:Concept rdf:about="http://data.europa.eu/dr8/DataInfrastructure">
        <skos:notation>DataInfrastructure</skos:notation>
        <skos:prefLabel xml:lang="en">[ABB426] Data Infrastructure</skos:prefLabel>
        <skos:definition xml:lang="en">DESCRIPTION:
Shares the functionalities to enable data sharing and consumption through the use of static and dynamic data repositories, data lakes and data hubs.

Source: Gartner

INTEROPERABILITY SALIENCY:
IoP Dimension: Structural IoP
The Data Hosting ABB is salient for technical interoperability because it provides all the functionalities to share and consume data.

EXAMPLES:
The following implementation is an example on how this specific Architecture Building Block (ABB) can be instantiated as a Solution Building Block (SBB):

D4Science
D4Science is an organisation operating a Data Hosting offering a rich array of services by community-driven virtual research environments. In particular, it supports communities of practice willing to implement open science practices. The infrastructure follows the system of systems approach, where the constituent systems (Service providers) offer resources (namely services and by them data, computing, storage) assembled together to implement the overall set of D4Science services.
https://www.d4science.org/</skos:definition>
        <skos:topConceptOf rdf:resource="http://data.europa.eu/dr8"/>
    </skos:Concept>

    <skos:Concept rdf:about="http://data.europa.eu/dr8/DataHub">
        <skos:notation>DataHub</skos:notation>
        <skos:prefLabel xml:lang="en">[ABB427] Data Hub</skos:prefLabel>
        <skos:definition xml:lang="en">DESCRIPTION:
A data hub is a collection of data from multiple sources organized for distribution, sharing, and often subsetting and sharing. Generally this data distribution is in the form of a hub and spoke architecture.

INTEROPERABILITY SALIENCY:
IoP Dimension: Structural IoP
The Data Hub ABBis salient for technical interoperability because it provides a single trustworthy location to store and access the data. EIF recommendation 37 &quot;Make authoritative sources of information available to others while implementing access and control mechanisms to ensure security and privacy in accordance with the relevant legislation&quot;.

EXAMPLES:
The following implementation is an example on how this specific Architecture Building Block (ABB) can be instantiated as a Solution Building Block (SBB):

Exprivia Data Hub:
The Exprivia Data Hub provides the tools needed to acquire, process and manage heterogeneous information from multiple sources.
https://www.exprivia.it/en/</skos:definition>
        <skos:topConceptOf rdf:resource="http://data.europa.eu/dr8"/>
    </skos:Concept>

    <skos:Concept rdf:about="http://data.europa.eu/dr8/DataLake">
        <skos:notation>DataLake</skos:notation>
        <skos:prefLabel xml:lang="en">[ABB428] Data Lake</skos:prefLabel>
        <skos:definition xml:lang="en">DESCRIPTION:
A data lake is usually a single store of data including raw copies of source system data, sensor data, social data etc., and transformed data used for tasks such as reporting, visualization, advanced analytics and machine learning. A data lake can include structured data from relational databases (rows and columns), semi-structured data (CSV, logs, XML, JSON), unstructured data (emails, documents, PDFs) and binary data (images, audio, video). A data lake can be established &quot;on premises&quot; (within an organization&apos;s data centers) or &quot;in the cloud&quot; (using cloud services from vendors such as Amazon, Microsoft, or Google).

INTEROPERABILITY SALIENCY:
IoP Dimension: Structural IoP
The Data Lake ABBis salient for technical interoperability because it provides a single trustworthy location to store and access the data. EIF recommendation 37 &quot;Make authoritative sources of information available to others while implementing access and control mechanisms to ensure security and privacy in accordance with the relevant legislation&quot;.

EXAMPLES:
The following implementation is an example on how this specific Architecture Building Block (ABB) can be instantiated as a Solution Building Block (SBB):

Google Cloud data lakes:
Google Cloud data lakes support any analysis on any type of data. This allows to import, store and analyse large volumes of heterogeneous, high-fidelity data securely and cost-effectively.
https://cloud.google.com/solutions/data-lake</skos:definition>
        <skos:topConceptOf rdf:resource="http://data.europa.eu/dr8"/>
    </skos:Concept>

    <skos:Concept rdf:about="http://data.europa.eu/dr8/DataRepositoryExchangeService">
        <skos:notation>DataRepositoryExchangeService</skos:notation>
        <skos:prefLabel xml:lang="en">[ABB429] Data Repository Exchange Service</skos:prefLabel>
        <skos:definition xml:lang="en">DESCRIPTION
Shares the functionalities of exchanging data structured under a source schema and transforming it into a target schema, so that the target data is an accurate representation of the source data. Data repository exchange service allows data to be shared between different application programs.

INTEROPERABILITY SALIENCY:
IoP Dimension: Structural IoP
The Data Repository Exchange Service ABB is salient for technical interoperability because it provides and shares the functionality for the share of data: &quot;Legislation requires that decisions and data are stored and can be accessed for a specified time. This means that records and information in electronic form held by public administrations for the purpose of documenting procedures and decisions must be preserved and be converted, where necessary, to new media when old media become obsolete. The goal is to ensure that records and other forms of information keep their legibility, reliability and integrity and can be accessed as long as needed subject to security and privacy provisions.&quot;

EXAMPLES:
The following implementation is an example on how this specific Architecture Building Block (ABB) can be instantiated as a Solution Building Block (SBB):

Oracle Data Exchange
The Data Exchange Service provides several access points to the Event Repository, allowing the user to perform queries on these events:
- The Query Subscription Administration Console configures the Data Exchange Service to create queries and periodically deliver query results to designated receivers (HTTP, JMS, and AS2). The Console can also test queries before subscribing, displaying user-readable events in XML format.
- A SOAP Web service allows programmatic queries. This SOAP service is based on the technically complete, but not formally ratified as of October 2006, EPCglobal EPC Information Services (EPCIS) Version 1.0 Specification.EPCglobal EPCIS 1.0 Working Draft.
https://docs.oracle.com/cd/E13197_01/rfid/enterprise_server/docs20/epcis/data-exchange.html</skos:definition>
        <skos:topConceptOf rdf:resource="http://data.europa.eu/dr8"/>
    </skos:Concept>

    <skos:Concept rdf:about="http://data.europa.eu/dr8/DataRepositoryExchangeComponent">
        <skos:notation>DataRepositoryExchangeComponent</skos:notation>
        <skos:prefLabel xml:lang="en">[ABB430] Data Repository Exchange Component</skos:prefLabel>
        <skos:definition xml:lang="en">DESCRIPTION
Shares the functionalities of exchanging data structured under a source schema and transforming it into a target schema, so that the target data is an accurate representation of the source data. Data repository exchange component allows data to be shared between different application programs.

INTEROPERABILITY SALIENCY:
IoP Dimension: Structural IoP
The Data Repository Exchange Component ABB is salient for technical interoperability because it provides and shares the functionality for the share of data: &quot;Legislation requires that decisions and data are stored and can be accessed for a specified time. This means that records and information in electronic form held by public administrations for the purpose of documenting procedures and decisions must be preserved and be converted, where necessary, to new media when old media become obsolete. The goal is to ensure that records and other forms of information keep their legibility, reliability and integrity and can be accessed as long as needed subject to security and privacy provisions.&quot;

EXAMPLES:
The following implementation is an example on how this specific Architecture Building Block (ABB) can be instantiated as a Solution Building Block (SBB):

Oracle Data Exchange
The Data Exchange Service provides several access points to the Event Repository, allowing the user to perform queries on these events:
- The Query Subscription Administration Console configures the Data Exchange Service to create queries and periodically deliver query results to designated receivers (HTTP, JMS, and AS2). The Console can also test queries before subscribing, displaying user-readable events in XML format.
- A SOAP Web service allows programmatic queries. This SOAP service is based on the technically complete, but not formally ratified as of October 2006, EPCglobal EPC Information Services (EPCIS) Version 1.0 Specification.EPCglobal EPCIS 1.0 Working Draft.
https://docs.oracle.com/cd/E13197_01/rfid/enterprise_server/docs20/epcis/data-exchange.html</skos:definition>
        <skos:topConceptOf rdf:resource="http://data.europa.eu/dr8"/>
    </skos:Concept>

    <skos:Collection rdf:about="http://data.europa.eu/dr8/view/IopSpecificationUnderpinningView">
        <skos:notation>IopSpecificationUnderpinningView</skos:notation>
        <skos:prefLabel xml:lang="en">IOP specification underpinning View</skos:prefLabel>
        <skos:member rdf:resource="http://data.europa.eu/dr8/InteroperabilitySpecification"/>
        <skos:member rdf:resource="http://data.europa.eu/dr8/LegalInteroperabilitySpecification"/>
        <skos:member rdf:resource="http://data.europa.eu/dr8/OrganisationalInteroperabilitySpecification"/>
        <skos:member rdf:resource="http://data.europa.eu/dr8/SemanticInteroperabilitySpecification"/>
        <skos:member rdf:resource="http://data.europa.eu/dr8/TechnicalInteroperabilitySpecification"/>
    </skos:Collection>

    <skos:Concept rdf:about="http://data.europa.eu/dr8/InteroperabilitySpecification">
        <skos:notation>InteroperabilitySpecification</skos:notation>
        <skos:prefLabel xml:lang="en">[ABB162] Interoperability Specification</skos:prefLabel>
        <skos:definition xml:lang="en">DESCRIPTION:
An Interoperability Specification is a document of the highest possible level of granularity on an EIRA SBB, formulated as an agreed normative statement in design terms on a legal, organisational, semantic, or technical attribute of an European Public Service.  It  can refer to existing  standards or  specifications

Source: ISA2  EIA Action

IoP dimensions: Structural IoP, Behavioral IoP, Governance IoP</skos:definition>
        <skos:narrower rdf:resource="http://data.europa.eu/dr8/KeyInteroperabilityEnabler"/>
    </skos:Concept>

    <skos:Concept rdf:about="http://data.europa.eu/dr8/LegalInteroperabilitySpecification">
        <skos:notation>LegalInteroperabilitySpecification</skos:notation>
        <skos:prefLabel xml:lang="en">[ABB175] Legal Interoperability Specification</skos:prefLabel>
        <skos:definition xml:lang="en">DESCRIPTION:
An Legal Interoperability Specification is a document of the highest possible level of granularity on an EIRA SBB, formulated as an agreed normative statement in design terms on a legal attribute of an European Public Service. It can refer to existing standards or specifications.

Source: How does the EIRA support interoperability?
https://joinup.ec.europa.eu/sites/default/files/how_does_eira_support_interoperability_v1_0_0.pdf

INTEROPERABILITY SALIENCY:
IoP Dimension: Structural IoP, Behavioral IoP, Governance IoP
The Legal Interoperability Specification ABB  is relevant for interoperability  a key interoperability enabler because it helps achieve legal interoperability by  addressing the core legal interoperability background for solutions.

EXAMPLES:
The following implementation is an example on how this specific Architecture Building Block (ABB) can be instantiated as a Solution Building Block (SBB):

e-procurement SAT - Directive 2014/24/EU on public procurement
DIRECTIVE 2014/24/EU OF THE EUROPEAN PARLIAMENT AND OF THE COUNCIL of 26 February 2014 on public procurement and repealing Directive 2004/18/EC (Text with EEA relevance). The directive sets out rules on the use of public contracts for the provision of works, supplies or services by companies or individuals and the exemptions which can be applied. The legislation specifies that when national authorities use public procurement to invite tenders to provide works, supplies or services, they must treat all applicants equally and not discriminate between them. They must also be transparent in their dealings. This Directive is considered as a Legal Interoperability Specification, as it shall be transposed in a National or Regional Binding Instrument when designing the solution using the e-procurement Solution Architecture Template.
https://joinup.ec.europa.eu/asset/eia/description</skos:definition>
        <skos:narrower rdf:resource="http://data.europa.eu/dr8/InteroperabilitySpecification"/>
    </skos:Concept>

    <skos:Concept rdf:about="http://data.europa.eu/dr8/OrganisationalInteroperabilitySpecification">
        <skos:notation>OrganisationalInteroperabilitySpecification</skos:notation>
        <skos:prefLabel xml:lang="en">[ABB176] Organisational Interoperability Specification</skos:prefLabel>
        <skos:definition xml:lang="en">DESCRIPTION:
This aspect of interoperability is concerned with how organisations, such as public administrations in different Member States, cooperate to achieve their mutually agreed goals. In practice, organisational interoperability implies integrating business processes and related data exchange. Organisational interoperability also aims to meet the requirements of the user community by making services available, easily identifiable, accessible and user-focused.

Organisation interoperability specifications support organisational interoperability by addressing the core organizational interoperability background for solutions.

Source: How does the EIRA support interoperability?
https://joinup.ec.europa.eu/sites/default/files/how_does_eira_support_interoperability_v1_0_0.pdf

EXAMPLES:
The following implementation is an example on how this specific Architecture Building Block (ABB) can be instantiated as a Solution Building Block (SBB):

Memorandum of Understanding on Economic and Financial Statistics between the DG Statistics of the European Central Bank and Eurostat
The purpose of this Memorandum of Understanding is to set out the respective areas of responsibility in economic and financial statistics at the Community level of the ECB (Directorate General Statistics) and the Commission (Eurostat); to provide a framework for the exchange and reproduction of data; to note the forms which co-operation between the Directorate General Statistics (DG Statistics) and Eurostat will take; and to set down a procedure for resolving disagreements.
https://www.ecb.europa.eu/ecb/legal/pdf/en_mou_with_eurostat1.pdf</skos:definition>
        <skos:narrower rdf:resource="http://data.europa.eu/dr8/InteroperabilitySpecification"/>
    </skos:Concept>

    <skos:Concept rdf:about="http://data.europa.eu/dr8/SemanticInteroperabilitySpecification">
        <skos:notation>SemanticInteroperabilitySpecification</skos:notation>
        <skos:prefLabel xml:lang="en">[ABB177] Semantic Interoperability Specification</skos:prefLabel>
        <skos:definition xml:lang="en">DESCRIPTION:
Semantic interoperability enables organisations to process information from external sources in a meaningful manner. It ensures that the precise meaning of exchanged information is understood and preserved throughout exchanges between parties. In the context of the EIF, semantic interoperability encompasses the following aspects:
	Semantic interoperability is about the meaning of data elements and the relationship between them. It includes developing vocabulary to describe data exchanges, and ensures that data elements are understood in the same way by communicating parties.
	Syntactic interoperability is about describing the exact format of the information to be exchanged in terms of grammar, format and schemas.
Semantic interoperability specifications support semantic interoperability by addressing the core semantic interoperability background for solutions.

Source: How does the EIRA support interoperability?
https://joinup.ec.europa.eu/sites/default/files/how_does_eira_support_interoperability_v1_0_0.pdf

INTEROPERABILITY SALIENCY:
IoP Dimension: Structural IoP, Behavioral IoP, Governance IoP
The Semantic Interoperability Specification ABB is salient for semantic interoperability because it enables organisations to process information from external sources in a meaningful manner and ensuring that the precise meaning of exchanged information is understood and preserved throughout exchanges between parties as stated in the EIF recommendation n32: &quot;Support the establishment of sector-specific and cross-sectoral communities that aim to create open information specifications and encourage relevant communities to share their results on national and European platforms.&quot;

EXAMPLES:
The following implementation is an example on how this specific Architecture Building Block (ABB) can be instantiated as a Solution Building Block (SBB):

United Nations Centre for Trade Facilitation and E-Business (UN/CEFACT) standard - International Plant Protection Convention (IPPC) SPSCertificate
Specification of phytosanitary certificates. These certificates are issued to indicate that consignments of plants, plant products or other regulated articles meet specified phytosanitary import requirements and are in conformity with the certifying statement of the appropriate model certificate.
https://www.ippc.int/en/ephyto/ephyto-technical-information/</skos:definition>
        <skos:narrower rdf:resource="http://data.europa.eu/dr8/InteroperabilitySpecification"/>
    </skos:Concept>

    <skos:Concept rdf:about="http://data.europa.eu/dr8/TechnicalInteroperabilitySpecification">
        <skos:notation>TechnicalInteroperabilitySpecification</skos:notation>
        <skos:prefLabel xml:lang="en">[ABB178] Technical Interoperability Specification</skos:prefLabel>
        <skos:definition xml:lang="en">DESCRIPTION:
A specification contained in a document which lays down the characteristics required of a product such as levels of quality, performance, safety or dimensions, including the requirements applicable to the product as regards the name under which the product is sold, terminology, symbols, testing and test methods, packaging, marking or labelling and conformity assessment procedures.

Source: Directive 98/34/EC laying down a procedure for the provision of information in the field of technical standards
and regulations and of rules on Information Society services;
http://eur-lex.europa.eu/LexUriServ/LexUriServ.do?uri=CONSLEG:1998L0034:20070101:EN:PDF

INTEROPERABILITY SALIENCY:
IoP dimensions: Structural IoP, Behavioral IoP, Governance IoP
The Technical Interoperability Specification ABB is salient for technical interoperability because it assesses the characteristics required of a product to support interoperability solutions.

EXAMPLES:
The following implementation is an example on how this specific Architecture Building Block (ABB) can be instantiated as a Solution Building Block (SBB):

HTTPS specification
HTTP [RFC2616] was originally used in the clear on the Internet. However, increased use of HTTP for sensitive applications has required security measures. SSL, and its successor TLS [RFC2246] were designed to provide channel-oriented security.
https://tools.ietf.org/html/rfc2818</skos:definition>
        <skos:narrower rdf:resource="http://data.europa.eu/dr8/InteroperabilitySpecification"/>
    </skos:Concept>

    <skos:Collection rdf:about="http://data.europa.eu/dr8/view/EiraOntologyViewpoint">
        <skos:notation>EiraOntologyViewpoint</skos:notation>
        <skos:prefLabel xml:lang="en">EIRA Ontology Viewpoint</skos:prefLabel>
        <skos:member rdf:resource="http://data.europa.eu/dr8/EiraViewpoint"/>
        <skos:member rdf:resource="http://data.europa.eu/dr8/ArchitectureBuildingBlock"/>
        <skos:member rdf:resource="http://data.europa.eu/dr8/SolutionBuildingBlock"/>
        <skos:member rdf:resource="http://data.europa.eu/dr8/EiraView"/>
        <skos:member rdf:resource="http://data.europa.eu/dr8/EiraArchitectureBuildingBlock"/>
        <skos:member rdf:resource="http://data.europa.eu/dr8/EiraSolutionBuildingBlock"/>
        <skos:member rdf:resource="http://data.europa.eu/dr8/Solution"/>
        <skos:member rdf:resource="http://data.europa.eu/dr8/EifInteroperabilityLevel"/>
        <skos:member rdf:resource="http://data.europa.eu/dr8/PublicServiceAgent"/>
        <skos:member rdf:resource="http://data.europa.eu/dr8/PublicServiceManifestation"/>
        <skos:member rdf:resource="http://data.europa.eu/dr8/PublicServiceComponent"/>
        <skos:member rdf:resource="http://data.europa.eu/dr8/KeyInteroperabilityEnabler"/>
        <skos:member rdf:resource="http://data.europa.eu/dr8/InteroperabilityAspect"/>
        <skos:member rdf:resource="http://data.europa.eu/dr8/InteroperabilityRequirement"/>
        <skos:member rdf:resource="http://data.europa.eu/dr8/LegalInteroperabilityRequirement"/>
        <skos:member rdf:resource="http://data.europa.eu/dr8/OrganisationalInteroperabilityRequirement"/>
        <skos:member rdf:resource="http://data.europa.eu/dr8/SemanticInteroperabilityRequirement"/>
        <skos:member rdf:resource="http://data.europa.eu/dr8/TechnicalInteroperabilityRequirement"/>
        <skos:member rdf:resource="http://data.europa.eu/dr8/EifPrinciple"/>
    </skos:Collection>

    <skos:Concept rdf:about="http://data.europa.eu/dr8/EiraViewpoint">
        <skos:notation>EiraViewpoint</skos:notation>
        <skos:prefLabel xml:lang="en">[ABB333] EIRA Viewpoint</skos:prefLabel>
        <skos:definition xml:lang="en">DESCRIPTION:
The EIRA provides several viewpoints (1) that conform to EIRA views. The viewpoints provide a perspective with specific stakeholders concern in mind.

(1) A specification of the conventions for a particular kind of architecture view.
Source: TOGAF
https://pubs.opengroup.org/architecture/togaf9-doc/arch/chap03.html#tag_03_18</skos:definition>
        <skos:topConceptOf rdf:resource="http://data.europa.eu/dr8"/>
    </skos:Concept>

    <skos:Concept rdf:about="http://data.europa.eu/dr8/ArchitectureBuildingBlock">
        <skos:notation>ArchitectureBuildingBlock</skos:notation>
        <skos:prefLabel xml:lang="en">[ABB334] Architecture Building Block</skos:prefLabel>
        <skos:definition xml:lang="en">DESCRIPTION:
An Architecture Building Block (ABB) is a constituent of the architecture model that describes a single aspect of the overall model. An Architecture Building Block describes generic characteristics and functionalities. Architecture Building Blocks are used to describe reference architectures, solution architecture templates or solution architectures of a specific solutions.

Source: TOGAF
https://pubs.opengroup.org/architecture/togaf9-doc/arch/chap03.html#tag_03_8</skos:definition>
        <skos:topConceptOf rdf:resource="http://data.europa.eu/dr8"/>
    </skos:Concept>

    <skos:Concept rdf:about="http://data.europa.eu/dr8/SolutionBuildingBlock">
        <skos:notation>SolutionBuildingBlock</skos:notation>
        <skos:prefLabel xml:lang="en">[ABB335] Solution Building Block</skos:prefLabel>
        <skos:definition xml:lang="en">DESCRIPTION:
A Solution Building Block (SBB) is a candidate solution which conforms to the specification of an Architecture Building Block (ABB).

Source: TOGAF
https://pubs.opengroup.org/architecture/togaf9-doc/arch/chap03.html#tag_03_70</skos:definition>
        <skos:topConceptOf rdf:resource="http://data.europa.eu/dr8"/>
    </skos:Concept>

    <skos:Concept rdf:about="http://data.europa.eu/dr8/EiraView">
        <skos:notation>EiraView</skos:notation>
        <skos:prefLabel xml:lang="en">[ABB336] EIRA View</skos:prefLabel>
        <skos:definition xml:lang="en">The EIRA consists of several architecture views(1), including one view for each of the EIF interoperability levels. The EIRA views contain a graphical notation of the EIRA ontology.

(1) An architecture view is a representation of a system from the perspective of a related set of concerns.
Source: TOGAF
https://pubs.opengroup.org/architecture/togaf9-doc/arch/chap03.html#tag_03_17</skos:definition>
        <skos:topConceptOf rdf:resource="http://data.europa.eu/dr8"/>
    </skos:Concept>

    <skos:Concept rdf:about="http://data.europa.eu/dr8/EiraArchitectureBuildingBlock">
        <skos:notation>EiraArchitectureBuildingBlock</skos:notation>
        <skos:prefLabel xml:lang="en">[ABB337] EIRA Architecture Building Block</skos:prefLabel>
        <skos:definition xml:lang="en">DESCRIPTION:
An EIRA Architecture Building Block is a requirement of an intermediate  level of granularity, in alignment with at least one EIF principle, formulated as an agreed normative statement in functional terms on a legal, organisational, semantic, or technical attribute of a To-Be European Public Service. An EIRA ABB might encapsulate several interoperability aspects</skos:definition>
        <skos:narrower rdf:resource="http://data.europa.eu/dr8/ArchitectureBuildingBlock"/>
    </skos:Concept>

    <skos:Concept rdf:about="http://data.europa.eu/dr8/EiraSolutionBuildingBlock">
        <skos:notation>EiraSolutionBuildingBlock</skos:notation>
        <skos:prefLabel xml:lang="en">[ABB338] EIRA Solution Building Block</skos:prefLabel>
        <skos:definition xml:lang="en">DESCRIPTION:
An EIRA Solution Building Block is a concrete component of an intermediate  level of granularity, that it implements one or more EIRA Architecture Building Blocks of an European Public Service, formulated as an agreed normative statement in design terms on a legal, organisational, semantic, or technical attribute of an European Public Service. On the technical view, a Solution Building Block is a specific software component that it might be either procured or developed of a To-Be Interoperable European Solution or that it is integrated in an As-Is Interoperable European Solution</skos:definition>
        <skos:narrower rdf:resource="http://data.europa.eu/dr8/SolutionBuildingBlock"/>
    </skos:Concept>

    <skos:Concept rdf:about="http://data.europa.eu/dr8/Solution">
        <skos:notation>Solution</skos:notation>
        <skos:prefLabel xml:lang="en">[ABB339] Solution</skos:prefLabel>
        <skos:definition xml:lang="en">DESCRIPTION:
A solution consists of one or more Solution Building Blocks to meet a certain stakeholder need. Within the context of the EIRA, a solution is usually an Interoperable European Solution developed by public administrations that facilitate the delivery of electronic Public Services and cross-border exchange of information between public administrations or Citizens in support to the implementation and advancement of EU, national or local public policies.

Inspired by TOGAF
https://pubs.opengroup.org/architecture/togaf9-doc/arch/chap03.html#tag_03_69</skos:definition>
        <skos:topConceptOf rdf:resource="http://data.europa.eu/dr8"/>
    </skos:Concept>

    <skos:Concept rdf:about="http://data.europa.eu/dr8/EifInteroperabilityLevel">
        <skos:notation>EifInteroperabilityLevel</skos:notation>
        <skos:prefLabel xml:lang="en">[ABB340] EIF Interoperability Level</skos:prefLabel>
        <skos:definition xml:lang="en">DESCRIPTION:
The New European Interoperability Framework (EIF) is a set of guidelines for developing public services. The EIF defines four interoperability levels, which cover legal, organisational, semantic and technical interoperability. Each level deserves special attention when a new European public service is established.

(1) European Commission, ISA Programme. The New European Interoperability Framework (EIF) for European public services. [Online] 2017. https://ec.europa.eu/isa2/eif_en.</skos:definition>
        <skos:topConceptOf rdf:resource="http://data.europa.eu/dr8"/>
    </skos:Concept>

    <skos:Concept rdf:about="http://data.europa.eu/dr8/PublicServiceAgent">
        <skos:notation>PublicServiceAgent</skos:notation>
        <skos:prefLabel xml:lang="en">[ABB341] Public Service Agent</skos:prefLabel>
        <skos:definition xml:lang="en"></skos:definition>
        <skos:narrower rdf:resource="http://data.europa.eu/dr8/EiraArchitectureBuildingBlock"/>
    </skos:Concept>

    <skos:Concept rdf:about="http://data.europa.eu/dr8/PublicServiceManifestation">
        <skos:notation>PublicServiceManifestation</skos:notation>
        <skos:prefLabel xml:lang="en">[ABB342] Public Service Manifestation</skos:prefLabel>
        <skos:definition xml:lang="en">A Public Service Manifestation is a behaviour EIRA Architecture Building Block, i.e. a unit of activity performed by one or more Public Service Components.</skos:definition>
        <skos:narrower rdf:resource="http://data.europa.eu/dr8/EiraArchitectureBuildingBlock"/>
    </skos:Concept>

    <skos:Concept rdf:about="http://data.europa.eu/dr8/PublicServiceComponent">
        <skos:notation>PublicServiceComponent</skos:notation>
        <skos:prefLabel xml:lang="en">[ABB343] Public Service Component</skos:prefLabel>
        <skos:definition xml:lang="en">A Public Service Component is a structural EIRA Architecture Building Block, i.e. an entity which can perform behaviour (active structure) or on which behaviour is performed (passive structure).</skos:definition>
        <skos:narrower rdf:resource="http://data.europa.eu/dr8/EiraArchitectureBuildingBlock"/>
    </skos:Concept>

    <skos:Concept rdf:about="http://data.europa.eu/dr8/KeyInteroperabilityEnabler">
        <skos:notation>KeyInteroperabilityEnabler</skos:notation>
        <skos:prefLabel xml:lang="en">[ABB344] Key Interoperability Enabler</skos:prefLabel>
        <skos:definition xml:lang="en">DESCRIPTION:
A Key Interoperability Enabler is an EIRA Architecture Building Block, which is necessary to enable the efficient and effective delivery of public services across administrations.</skos:definition>
        <skos:narrower rdf:resource="http://data.europa.eu/dr8/EiraArchitectureBuildingBlock"/>
    </skos:Concept>

    <skos:Concept rdf:about="http://data.europa.eu/dr8/InteroperabilityAspect">
        <skos:notation>InteroperabilityAspect</skos:notation>
        <skos:prefLabel xml:lang="en">[ABB345] Interoperability Aspect</skos:prefLabel>
        <skos:definition xml:lang="en">DESCRIPTION:
An Interoperability Aspect encapsulates a set of interoperability requirements to be provided/supported by an European Public Service</skos:definition>
        <skos:topConceptOf rdf:resource="http://data.europa.eu/dr8"/>
    </skos:Concept>

    <skos:Concept rdf:about="http://data.europa.eu/dr8/InteroperabilityRequirement">
        <skos:notation>InteroperabilityRequirement</skos:notation>
        <skos:prefLabel xml:lang="en">[ABB346] Interoperability Requirement</skos:prefLabel>
        <skos:definition xml:lang="en">DESCRIPTION:
An Interoperability Requirement is requirement of the highest possible level of granularity for an EIRA ABB, formulated as an agreed normative statement in functional terms on a legal, organisational, semantic, or technical attribute of a To-Be European Public Service</skos:definition>
        <skos:topConceptOf rdf:resource="http://data.europa.eu/dr8"/>
    </skos:Concept>

    <skos:Concept rdf:about="http://data.europa.eu/dr8/LegalInteroperabilityRequirement">
        <skos:notation>LegalInteroperabilityRequirement</skos:notation>
        <skos:prefLabel xml:lang="en">[ABB347] Legal Interoperability Requirement</skos:prefLabel>
        <skos:definition xml:lang="en">A legal interoperability requirement is an interoperability requirement that must be met to help achieve legal interoperability.</skos:definition>
        <skos:narrower rdf:resource="http://data.europa.eu/dr8/InteroperabilityRequirement"/>
    </skos:Concept>

    <skos:Concept rdf:about="http://data.europa.eu/dr8/OrganisationalInteroperabilityRequirement">
        <skos:notation>OrganisationalInteroperabilityRequirement</skos:notation>
        <skos:prefLabel xml:lang="en">[ABB348] Organisational Interoperability Requirement</skos:prefLabel>
        <skos:definition xml:lang="en">An organisational interoperability requirement is an interoperability requirement that must be met to help achieve organisational interoperability.</skos:definition>
        <skos:narrower rdf:resource="http://data.europa.eu/dr8/InteroperabilityRequirement"/>
    </skos:Concept>

    <skos:Concept rdf:about="http://data.europa.eu/dr8/SemanticInteroperabilityRequirement">
        <skos:notation>SemanticInteroperabilityRequirement</skos:notation>
        <skos:prefLabel xml:lang="en">[ABB349] Semantic Interoperability Requirement</skos:prefLabel>
        <skos:definition xml:lang="en">A semantical interoperability requirement is an interoperability requirement that must be met to help achieve semantic interoperability.</skos:definition>
        <skos:narrower rdf:resource="http://data.europa.eu/dr8/InteroperabilityRequirement"/>
    </skos:Concept>

    <skos:Concept rdf:about="http://data.europa.eu/dr8/TechnicalInteroperabilityRequirement">
        <skos:notation>TechnicalInteroperabilityRequirement</skos:notation>
        <skos:prefLabel xml:lang="en">[ABB350] Technical Interoperability Requirement</skos:prefLabel>
        <skos:definition xml:lang="en">A technical interoperability requirement is an interoperability requirement that must be met to help achieve technical interoperability.</skos:definition>
        <skos:narrower rdf:resource="http://data.europa.eu/dr8/InteroperabilityRequirement"/>
    </skos:Concept>

    <skos:Concept rdf:about="http://data.europa.eu/dr8/EifPrinciple">
        <skos:notation>EifPrinciple</skos:notation>
        <skos:prefLabel xml:lang="en">[ABB300] EIF Principle</skos:prefLabel>
        <skos:definition xml:lang="en">DESCRIPTION:
It is a requirement of the lowest possible level of granularity providing agreed orientation i) to analyse European public services by driving the identification and formulation of interoperability requirements with higher levels of granularity and ii) to design European public services by driving the identification and formulation of interoperability specifications

Source: The New EIF. https://ec.europa.eu/isa2/eif_en
The new European Interoperability Framework (EIF) is part of the Communication (COM(2017)134) from the European Commission adopted on 23 March 2017. The framework gives specific guidance on how to set up interoperable digital public services.</skos:definition>
        <skos:topConceptOf rdf:resource="http://data.europa.eu/dr8"/>
    </skos:Concept>

    <skos:Collection rdf:about="http://data.europa.eu/dr8/view/EiraOntologyViewpoint">
        <skos:notation>EiraOntologyViewpoint</skos:notation>
        <skos:prefLabel xml:lang="en">EIRA Ontology viewpoint</skos:prefLabel>
        <skos:member rdf:resource="http://data.europa.eu/dr8/ArchitecturePrinciple"/>
        <skos:member rdf:resource="http://data.europa.eu/dr8/ArchitectureRequirement"/>
        <skos:member rdf:resource="http://data.europa.eu/dr8/SolutionSpecification"/>
    </skos:Collection>

    <skos:Concept rdf:about="http://data.europa.eu/dr8/ArchitecturePrinciple">
        <skos:notation>ArchitecturePrinciple</skos:notation>
        <skos:prefLabel xml:lang="en">[ABB381] Architecture Principle</skos:prefLabel>
        <skos:definition xml:lang="en">DESCRIPTION:
Architecture Principles define the underlying general rules and guidelines for the use and deployment of all IT resources and assets across the enterprise. They reflect a level of consensus among the various elements of the enterprise, and form the basis for making future IT decisions.

Source: TOGAF 9.2 The Open Group
https://pubs.opengroup.org/architecture/togaf9-doc/arch/chap20.html#:~:text=Architecture%20Principles%20define%20the%20underlying,for%20making%20future%20IT%20decisions.</skos:definition>
        <skos:topConceptOf rdf:resource="http://data.europa.eu/dr8"/>
    </skos:Concept>

    <skos:Concept rdf:about="http://data.europa.eu/dr8/ArchitectureRequirement">
        <skos:notation>ArchitectureRequirement</skos:notation>
        <skos:prefLabel xml:lang="en">[ABB382] Architecture Requirement</skos:prefLabel>
        <skos:definition xml:lang="en">DESCRIPTION:
A Architectrure Requirement is requirement of the highest possible level of granularity for an Architectural Building Block, formulated as an agreed normative statement of a To-Be European Public Service</skos:definition>
        <skos:topConceptOf rdf:resource="http://data.europa.eu/dr8"/>
    </skos:Concept>

    <skos:Concept rdf:about="http://data.europa.eu/dr8/SolutionSpecification">
        <skos:notation>SolutionSpecification</skos:notation>
        <skos:prefLabel xml:lang="en">[ABB383] Solution Specification</skos:prefLabel>
        <skos:definition xml:lang="en">DESCRIPTION:
An Architecture Specification is a document of the highest possible level of granularity on an Solution Building Block, formulated as an agreed normative statement in design of an European Public Service.</skos:definition>
        <skos:topConceptOf rdf:resource="http://data.europa.eu/dr8"/>
    </skos:Concept>

    <skos:Collection rdf:about="http://data.europa.eu/dr8/view/ArchitecturalPrincipleView">
        <skos:notation>ArchitecturalPrincipleView</skos:notation>
        <skos:prefLabel xml:lang="en">Architectural Principle View</skos:prefLabel>
        <skos:member rdf:resource="http://data.europa.eu/dr8/EvidenceBasedPublicPolicy"/>
        <skos:member rdf:resource="http://data.europa.eu/dr8/Transparency"/>
        <skos:member rdf:resource="http://data.europa.eu/dr8/PublicValue"/>
        <skos:member rdf:resource="http://data.europa.eu/dr8/SuccessfulPublicServiceImplementationOrientation"/>
        <skos:member rdf:resource="http://data.europa.eu/dr8/SocialParticipation"/>
        <skos:member rdf:resource="http://data.europa.eu/dr8/Accountability"/>
        <skos:member rdf:resource="http://data.europa.eu/dr8/MarketCollaboration"/>
        <skos:member rdf:resource="http://data.europa.eu/dr8/DigitalInclusion"/>
        <skos:member rdf:resource="http://data.europa.eu/dr8/Accessibility"/>
        <skos:member rdf:resource="http://data.europa.eu/dr8/EuropeanDigitalSovereignty"/>
        <skos:member rdf:resource="http://data.europa.eu/dr8/EuLegislationCompliance"/>
        <skos:member rdf:resource="http://data.europa.eu/dr8/IntegratedHorizontalUserExperience"/>
        <skos:member rdf:resource="http://data.europa.eu/dr8/OnceOnly"/>
        <skos:member rdf:resource="http://data.europa.eu/dr8/CodeOfEthicsCompliance"/>
        <skos:member rdf:resource="http://data.europa.eu/dr8/Privacy"/>
        <skos:member rdf:resource="http://data.europa.eu/dr8/EulfCompliance"/>
        <skos:member rdf:resource="http://data.europa.eu/dr8/TechnologyNeutrality"/>
        <skos:member rdf:resource="http://data.europa.eu/dr8/ServiceOrientation"/>
        <skos:member rdf:resource="http://data.europa.eu/dr8/Proactiveness"/>
        <skos:member rdf:resource="http://data.europa.eu/dr8/AdministrativeSimplification"/>
        <skos:member rdf:resource="http://data.europa.eu/dr8/NewPublicManagementApproach"/>
        <skos:member rdf:resource="http://data.europa.eu/dr8/ConvergenceAssuranceOnPublicPolicyGoalsAttainment"/>
        <skos:member rdf:resource="http://data.europa.eu/dr8/Multilingulism"/>
        <skos:member rdf:resource="http://data.europa.eu/dr8/Openness"/>
        <skos:member rdf:resource="http://data.europa.eu/dr8/User-centricity"/>
        <skos:member rdf:resource="http://data.europa.eu/dr8/Reusability"/>
        <skos:member rdf:resource="http://data.europa.eu/dr8/SubsidiarityAndProportionality"/>
        <skos:member rdf:resource="http://data.europa.eu/dr8/DataPortability"/>
        <skos:member rdf:resource="http://data.europa.eu/dr8/Security"/>
        <skos:member rdf:resource="http://data.europa.eu/dr8/ConvergenceControlOnPublicPolicyGoalsAttainment"/>
        <skos:member rdf:resource="http://data.europa.eu/dr8/PreservationOfInformation"/>
        <skos:member rdf:resource="http://data.europa.eu/dr8/Trust"/>
        <skos:member rdf:resource="http://data.europa.eu/dr8/Innovation"/>
    </skos:Collection>

    <skos:Concept rdf:about="http://data.europa.eu/dr8/EvidenceBasedPublicPolicy">
        <skos:notation>EvidenceBasedPublicPolicy</skos:notation>
        <skos:prefLabel xml:lang="en">[ABB409] Evidence based Public Policy</skos:prefLabel>
        <skos:definition xml:lang="en">DESCRIPTION:
&quot;Evidence-based Public Policies are policies designed and periodically reviewed looking at experimental evidences and incontrovertible data.
The primary goal is to improve the reliability of advice concerning the efficiency and effectiveness of policy settings and possible alternatives.
There are three crucial enabling factors that underpin modern conceptions of evidence-based policy (EBP): high-quality information bases on relevant topic areas, cohorts of professionals with skills in data analysis and policy evaluation, and political incentives for utilising evidence-based analysis and advice in governmental decision-making processes.&quot;</skos:definition>
        <skos:topConceptOf rdf:resource="http://data.europa.eu/dr8"/>
    </skos:Concept>

    <skos:Concept rdf:about="http://data.europa.eu/dr8/Transparency">
        <skos:notation>Transparency</skos:notation>
        <skos:prefLabel xml:lang="en">[ABB410] Transparency</skos:prefLabel>
        <skos:definition xml:lang="en">DESCRIPTION:
&quot;Transparency in the EIF context refers to:
i. Enabling visibility inside the administrative environment of a public administration. This is about allowing other public administrations, citizens and businesses to view and understand administrative rules, processes,11 data, services and decision-making.
ii. Ensuring availability of interfaces with internal information systems. Public administrations operate a large number of what are often heterogeneous and disparate information systems in support of their internal processes. Interoperability depends on ensuring the availability of interfaces to these systems and the data they handle. In turn, interoperability facilitates reuse of systems and data, and enables these to be integrated into larger systems.
iii. Securing the right to the protection of personal data, by respecting the applicable legal framework for the large volumes of personal data of citizens, held and managed by Public administrations.&quot;</skos:definition>
        <skos:topConceptOf rdf:resource="http://data.europa.eu/dr8"/>
    </skos:Concept>

    <skos:Concept rdf:about="http://data.europa.eu/dr8/PublicValue">
        <skos:notation>PublicValue</skos:notation>
        <skos:prefLabel xml:lang="en">[ABB411] Public Value</skos:prefLabel>
        <skos:definition xml:lang="en">DESCRIPTION:
Public values are rooted in a reciprocal relationship between administrators and the citizenry. Value is created by satisfying politically expressed desires of citizens and clients. A digital public service should create and deliver public value to the society.</skos:definition>
        <skos:topConceptOf rdf:resource="http://data.europa.eu/dr8"/>
    </skos:Concept>

    <skos:Concept rdf:about="http://data.europa.eu/dr8/SuccessfulPublicServiceImplementationOrientation">
        <skos:notation>SuccessfulPublicServiceImplementationOrientation</skos:notation>
        <skos:prefLabel xml:lang="en">[ABB412] Successful Public Service Implementation Orientation</skos:prefLabel>
        <skos:definition xml:lang="en">DESCRIPTION:
This refers to the implementation of the European interoperability framework, which is guided by the following vision: Public administrations should make implementation decisions selecting a focus among alternative implementation orientations and considering the best fit with the public policy context. Examples of resource based implementation orientations are the integration orientation, the technology orientation, the governance orientation, and the legal orientation.</skos:definition>
        <skos:topConceptOf rdf:resource="http://data.europa.eu/dr8"/>
    </skos:Concept>

    <skos:Concept rdf:about="http://data.europa.eu/dr8/SocialParticipation">
        <skos:notation>SocialParticipation</skos:notation>
        <skos:prefLabel xml:lang="en">[ABB413] Social participation</skos:prefLabel>
        <skos:definition xml:lang="en">DESCRIPTION:
&quot;Social participiation refers to Promoting Civic Participation and Transparency
of Government Decision-Making Processes covering policies concerning ICT:
 E-democracy
 E-participation
 Government-to-citizen (G2C)  Citizen-to-government (C2G)  Citizen-to-citizen (C2C)
 Open governance partnership  Grass-root activism and social
networking
 Political campaigns  Online media
 I-voting
 Mechanisms: e-petitions, online consultation
and crowd-sourcing platforms etc.&quot;</skos:definition>
        <skos:topConceptOf rdf:resource="http://data.europa.eu/dr8"/>
    </skos:Concept>

    <skos:Concept rdf:about="http://data.europa.eu/dr8/Accountability">
        <skos:notation>Accountability</skos:notation>
        <skos:prefLabel xml:lang="en">[ABB414] Accountability</skos:prefLabel>
        <skos:definition xml:lang="en">DESCRIPTION:
&quot;Digital public services will enable accountability of users and of public administrations.
Transparency, liability, controllability, responsibility, and responsiveness are defined as distinct dimensions of accountability, providing an improvement on the current state of conceptual fuzziness. The typology provides a vocabulary for the core argument, that conflicting expectations borne of disparate conceptions of accountability undermine organizational effectiveness.&quot;</skos:definition>
        <skos:topConceptOf rdf:resource="http://data.europa.eu/dr8"/>
    </skos:Concept>

    <skos:Concept rdf:about="http://data.europa.eu/dr8/MarketCollaboration">
        <skos:notation>MarketCollaboration</skos:notation>
        <skos:prefLabel xml:lang="en">[ABB415] Market collaboration</skos:prefLabel>
        <skos:definition xml:lang="en">DESCRIPTION:
&quot;Digital public services will be designed and delivered considering partnership relationships with private sector.
Market Collaboration ensures efficient and effective use of resources, by seeking for reusable standards, that are open and supporting cost-effective interoperability between ICT capabilities and facilitate citizen-oriented business models&quot;</skos:definition>
        <skos:topConceptOf rdf:resource="http://data.europa.eu/dr8"/>
    </skos:Concept>

    <skos:Concept rdf:about="http://data.europa.eu/dr8/DigitalInclusion">
        <skos:notation>DigitalInclusion</skos:notation>
        <skos:prefLabel xml:lang="en">[ABB416] Digital Inclusion</skos:prefLabel>
        <skos:definition xml:lang="en">DESCRIPTION:
Digital Inclusion relates to seamless, transparent, accessible and user-friendly digital government services. Citizens must be able to use such digital services without having legal knowledge. The members of our societies should have the opportunity to help shape the digital transformation and share their ideas and content with others unimpeded, while respecting the rights of third parties. The public sector should encourage such wider participation in policy-making by involving society in the design of public services through co-creation, ex- perimentation and collaboration.</skos:definition>
        <skos:topConceptOf rdf:resource="http://data.europa.eu/dr8"/>
    </skos:Concept>

    <skos:Concept rdf:about="http://data.europa.eu/dr8/Accessibility">
        <skos:notation>Accessibility</skos:notation>
        <skos:prefLabel xml:lang="en">[ABB403] Accessibility</skos:prefLabel>
        <skos:definition xml:lang="en">DESCRIPTION:
Accessibility ensures that people with disabilities, the elderly and other disadvantaged groups can use public services at service levels comparable to those provided to other citizens.</skos:definition>
        <skos:topConceptOf rdf:resource="http://data.europa.eu/dr8"/>
    </skos:Concept>

    <skos:Concept rdf:about="http://data.europa.eu/dr8/EuropeanDigitalSovereignty">
        <skos:notation>EuropeanDigitalSovereignty</skos:notation>
        <skos:prefLabel xml:lang="en">[ABB417] European digital sovereignty</skos:prefLabel>
        <skos:definition xml:lang="en">DESCRIPTION:
European digital sovereignty entails the ensurance that all underlying digital components of ICT solutions (hardware, software, and services) meet European requirements, including the requirements to deploy a secure cloud infrastructure and interoperable services that fully comply with European legal provisions and ethical values.</skos:definition>
        <skos:topConceptOf rdf:resource="http://data.europa.eu/dr8"/>
    </skos:Concept>

    <skos:Concept rdf:about="http://data.europa.eu/dr8/EuLegislationCompliance">
        <skos:notation>EuLegislationCompliance</skos:notation>
        <skos:prefLabel xml:lang="en">[ABB389] EU Legislation Compliance</skos:prefLabel>
        <skos:definition xml:lang="en">DESCRIPTION:
&quot;EU Legislation Compliance is the property of a (national/local) legislation to be coherent or to implement European legislation.
A compliance assessment of EU Directives must be carried out in two stages:
(1) timely and systematic check whether Member States have transposed Union law;
(2) a timely and systematic conformity check of national transposing measures against the relevant Union legislation (correct transposition).

While Member States are responsible for the timely and accurate transposition of directives as well as the correct application of the entire acquis, the Commission has to monitor the Member States efforts and ensure that their legislation complies with Union law.&quot;</skos:definition>
        <skos:topConceptOf rdf:resource="http://data.europa.eu/dr8"/>
    </skos:Concept>

    <skos:Concept rdf:about="http://data.europa.eu/dr8/IntegratedHorizontalUserExperience">
        <skos:notation>IntegratedHorizontalUserExperience</skos:notation>
        <skos:prefLabel xml:lang="en">[ABB390] Integrated Horizontal User Experience</skos:prefLabel>
        <skos:definition xml:lang="en">DESCRIPTION:
&quot;Integrated horizontal user experience refers to a user&apos;s experience, when her/his experience using a digital interface is fluent and seamless, also when she/he navigates through different applications/contexts.&quot;</skos:definition>
        <skos:topConceptOf rdf:resource="http://data.europa.eu/dr8"/>
    </skos:Concept>

    <skos:Concept rdf:about="http://data.europa.eu/dr8/OnceOnly">
        <skos:notation>OnceOnly</skos:notation>
        <skos:prefLabel xml:lang="en">[ABB391] Once Only</skos:prefLabel>
        <skos:definition xml:lang="en">DESCRIPTION:
TheOnce Only Principle entails that citizens and businesses provide diverse data only once in contact with public administrations, while public administration bodies take actions to internally share and reuse these data  even across borders  always in respect of data protection regulations and other constraints.</skos:definition>
        <skos:topConceptOf rdf:resource="http://data.europa.eu/dr8"/>
    </skos:Concept>

    <skos:Concept rdf:about="http://data.europa.eu/dr8/CodeOfEthicsCompliance">
        <skos:notation>CodeOfEthicsCompliance</skos:notation>
        <skos:prefLabel xml:lang="en">[ABB392] Code of ethics compliance</skos:prefLabel>
        <skos:definition xml:lang="en">DESCRIPTION:
Code of ethics compliance refers to the expression of important values and standards that are also to be found in the law, but are not encumbered by the limitations and constraints that necessarily attach to legally-binding rules that can be used to impose sanctions.</skos:definition>
        <skos:topConceptOf rdf:resource="http://data.europa.eu/dr8"/>
    </skos:Concept>

    <skos:Concept rdf:about="http://data.europa.eu/dr8/Privacy">
        <skos:notation>Privacy</skos:notation>
        <skos:prefLabel xml:lang="en">[ABB393] Privacy</skos:prefLabel>
        <skos:definition xml:lang="en">DESCRIPTION:
Privacy refers to any freely given, specific, informed and unambiguous indication of the data subject&apos;s wishes by which he or she, by a statement or by a clear affirmative action, signifies agreement to the processing of personal data relating to him or her</skos:definition>
        <skos:topConceptOf rdf:resource="http://data.europa.eu/dr8"/>
    </skos:Concept>

    <skos:Concept rdf:about="http://data.europa.eu/dr8/EulfCompliance">
        <skos:notation>EulfCompliance</skos:notation>
        <skos:prefLabel xml:lang="en">[ABB394] EULF compliance</skos:prefLabel>
        <skos:definition xml:lang="en">DESCRIPTION:
&quot;The EULF concept consists of a package of case studies, specifications, guidelines, training materials, recommendations and actions required by public administrations and stakeholder communities to facilitate the implementation, use and expansion of INSPIRE in an e-government context.&quot;</skos:definition>
        <skos:topConceptOf rdf:resource="http://data.europa.eu/dr8"/>
    </skos:Concept>

    <skos:Concept rdf:about="http://data.europa.eu/dr8/TechnologyNeutrality">
        <skos:notation>TechnologyNeutrality</skos:notation>
        <skos:prefLabel xml:lang="en">[ABB395] Technology Neutrality</skos:prefLabel>
        <skos:definition xml:lang="en">DESCRIPTION:
Technology Neutrality refers to the independency of specific technology choices, that therefore can operate on a variety of technology platforms</skos:definition>
        <skos:topConceptOf rdf:resource="http://data.europa.eu/dr8"/>
    </skos:Concept>

    <skos:Concept rdf:about="http://data.europa.eu/dr8/ServiceOrientation">
        <skos:notation>ServiceOrientation</skos:notation>
        <skos:prefLabel xml:lang="en">[ABB386] Service Orientation</skos:prefLabel>
        <skos:definition xml:lang="en">DESCRIPTION:
The design and implementation of sufficient mechanisms in order to attain full visibility on effective realisation of public services, based on public policies, by putting in place processes and procedures that provide accountability to stakeholders</skos:definition>
        <skos:topConceptOf rdf:resource="http://data.europa.eu/dr8"/>
    </skos:Concept>

    <skos:Concept rdf:about="http://data.europa.eu/dr8/Proactiveness">
        <skos:notation>Proactiveness</skos:notation>
        <skos:prefLabel xml:lang="en">[ABB397] Proactiveness</skos:prefLabel>
        <skos:definition xml:lang="en">DESCRIPTION:
&quot;Proactiveness refers to proactive services, which are public services that a public institution delivers following its own initiative considering the presumable will by the person and that is delivered based on the information stored in the data collections belonging to the state information system.
Proactive service is based on life and business events and circumstances&quot;</skos:definition>
        <skos:topConceptOf rdf:resource="http://data.europa.eu/dr8"/>
    </skos:Concept>

    <skos:Concept rdf:about="http://data.europa.eu/dr8/AdministrativeSimplification">
        <skos:notation>AdministrativeSimplification</skos:notation>
        <skos:prefLabel xml:lang="en">[ABB388] Administrative Simplification</skos:prefLabel>
        <skos:definition xml:lang="en">DESCRIPTION:
&quot;Administrative Simplification refers to streamlined delivery services. e.g.:
- Harmonised rules on eligibility and durability
- Greater use of simplified costs
- Linking payments with results
- e-Cohesion
- Proportional approach to control
- Simplification of solutions&quot;</skos:definition>
        <skos:topConceptOf rdf:resource="http://data.europa.eu/dr8"/>
    </skos:Concept>

    <skos:Concept rdf:about="http://data.europa.eu/dr8/NewPublicManagementApproach">
        <skos:notation>NewPublicManagementApproach</skos:notation>
        <skos:prefLabel xml:lang="en">[ABB400] New Public Management approach</skos:prefLabel>
        <skos:definition xml:lang="en">DESCRIPTION:
&quot;New Public Management arose out of a concern with government failures, a belief in the efficacy and efficiency  of markets, a belief in economic rationality, and a push away from  large, centralized government agencies toward devolution and privatization.
In New Public Management, public managers are urged to &quot;&quot;steer,  not row.&quot;&quot; They steer by determining objectives, or what should be  done, and by catalyzing service delivery, or how it should be done (rowing), via their choice of a particular &quot;&quot;tool&quot;&quot; or combination of  tools (e.g., markets, regulation, taxes, subsidies, insurance, etc.) for achieving the objectives (Salamon 200)&quot;</skos:definition>
        <skos:topConceptOf rdf:resource="http://data.europa.eu/dr8"/>
    </skos:Concept>

    <skos:Concept rdf:about="http://data.europa.eu/dr8/ConvergenceAssuranceOnPublicPolicyGoalsAttainment">
        <skos:notation>ConvergenceAssuranceOnPublicPolicyGoalsAttainment</skos:notation>
        <skos:prefLabel xml:lang="en">[ABB401] Convergence assurance on public policy goals attainment</skos:prefLabel>
        <skos:definition xml:lang="en">DESCRIPTION:
The assessment of effective realisation of public services, based on public policies, by evaluating various technological solutions when striving to ensure the effectiveness and efficiency of a European public service.</skos:definition>
        <skos:topConceptOf rdf:resource="http://data.europa.eu/dr8"/>
    </skos:Concept>

    <skos:Concept rdf:about="http://data.europa.eu/dr8/Multilingulism">
        <skos:notation>Multilingulism</skos:notation>
        <skos:prefLabel xml:lang="en">[ABB402] Multilingulism</skos:prefLabel>
        <skos:definition xml:lang="en">DESCRIPTION:
Multilingualism requires striking a balance between the expectations of citizens and businesses to be served in their own language(s) or their preferred language(s) and the ability of Member States public administrations to offer services in all official EU languages</skos:definition>
        <skos:topConceptOf rdf:resource="http://data.europa.eu/dr8"/>
    </skos:Concept>

    <skos:Concept rdf:about="http://data.europa.eu/dr8/Openness">
        <skos:notation>Openness</skos:notation>
        <skos:prefLabel xml:lang="en">[ABB404] Openness</skos:prefLabel>
        <skos:definition xml:lang="en">DESCRIPTION:
In the context of interoperable public services, the concept ofopennessmainly relates to data, specifications and software.</skos:definition>
        <skos:topConceptOf rdf:resource="http://data.europa.eu/dr8"/>
    </skos:Concept>

    <skos:Concept rdf:about="http://data.europa.eu/dr8/User-centricity">
        <skos:notation>User-centricity</skos:notation>
        <skos:prefLabel xml:lang="en">[ABB405] User-centricity</skos:prefLabel>
        <skos:definition xml:lang="en">DESCRIPTION:
User-centricity refers to putting users needs at the centre when determining which public services should be provided and how they should be delivered. Therefore, as far as possible, user needs and requirements should guide the design and development of public services, in accordance with the following expectations: i A multi-channel service delivery approach; ii A single point of contact should be made available to users; iii Users feedback should be systematically collected, assessed and used to design new public services and to further improve existing ones.</skos:definition>
        <skos:topConceptOf rdf:resource="http://data.europa.eu/dr8"/>
    </skos:Concept>

    <skos:Concept rdf:about="http://data.europa.eu/dr8/Reusability">
        <skos:notation>Reusability</skos:notation>
        <skos:prefLabel xml:lang="en">[ABB406] Reusability</skos:prefLabel>
        <skos:definition xml:lang="en">DESCRIPTION:
&quot;Reusability refers to IT solutions (e.g. software components, Application Programming Interfaces, standards), European frameworks (reference architectures, architectural frameworks and ontologies), information and data.
- Reference Architecture: Architecture is the structure of components, their interrelationships, and the principles and guidelines governing their design and evolution over time. A reference architecture is a generalized architecture of a solution, based on best-practices, domain neutral and, occasionally, with a focus on a particular aspect. The goal of a reference architecture is reusability; it reduces the amount of work, reduces errors and accelerates the development of solutions. A reference architecture should be based in a [reference] model and in a style.
- Architectural framework: a tool for assisting in the production of organization-specific architectures. An architectural framework consists of a technical  reference model, a method for architecture development and a list of component standards, specifications, products and their interrelationships which can be used to build up architectures.&quot;</skos:definition>
        <skos:topConceptOf rdf:resource="http://data.europa.eu/dr8"/>
    </skos:Concept>

    <skos:Concept rdf:about="http://data.europa.eu/dr8/SubsidiarityAndProportionality">
        <skos:notation>SubsidiarityAndProportionality</skos:notation>
        <skos:prefLabel xml:lang="en">[ABB407] Subsidiarity and proportionality</skos:prefLabel>
        <skos:definition xml:lang="en">DESCRIPTION:
Thesubsidiarity principlerequires EU decisions to be taken as closely as possible to the citizen</skos:definition>
        <skos:topConceptOf rdf:resource="http://data.europa.eu/dr8"/>
    </skos:Concept>

    <skos:Concept rdf:about="http://data.europa.eu/dr8/DataPortability">
        <skos:notation>DataPortability</skos:notation>
        <skos:prefLabel xml:lang="en">[ABB408] Data portability</skos:prefLabel>
        <skos:definition xml:lang="en">DESCRIPTION:
Data portability refers to the ability to move and reuse data easily among different applications and systems, which becomes even more challenging in cross-border scenarios.</skos:definition>
        <skos:topConceptOf rdf:resource="http://data.europa.eu/dr8"/>
    </skos:Concept>

    <skos:Concept rdf:about="http://data.europa.eu/dr8/Security">
        <skos:notation>Security</skos:notation>
        <skos:prefLabel xml:lang="en">[ABB385] Security</skos:prefLabel>
        <skos:definition xml:lang="en">DESCRIPTION:
Security refers to the support of the application of the eGovernment security policies in ICT. The primary policies are: 1) Privacy by Design, 2) Encourage the development and use of highly secure systems (long-term), 3) Create stronger institutional supervision and oversight of security, 4) Substantiate the data minimization principle by using anonymization techniques in all European eGovernment systems, 5) Stimulate technical and legal solutions that avoid or limit privacy risks caused by re-identification of previously anonymized data, 6) Make Privacy Impact Assessments of eGovernment systems mandatory and public, 7) Use gateways to achieve interoperability of different national eGovernment security tools, but aim at Europe-wide availability and usability of tools, 7) Ensure open and transparent evaluations of the trade-offs between privacy, security, usability, interoperability and costs of an eGovernment system, 8) Develop a policy strategy for improving the security of IT-systems used in Europe</skos:definition>
        <skos:topConceptOf rdf:resource="http://data.europa.eu/dr8"/>
    </skos:Concept>

    <skos:Concept rdf:about="http://data.europa.eu/dr8/ConvergenceControlOnPublicPolicyGoalsAttainment">
        <skos:notation>ConvergenceControlOnPublicPolicyGoalsAttainment</skos:notation>
        <skos:prefLabel xml:lang="en">[ABB386] Convergence control on public policy goals attainment</skos:prefLabel>
        <skos:definition xml:lang="en">DESCRIPTION:
The design and implementation of sufficient mechanisms in order to attain full visibility on effective realisation of public services, based on public policies, by putting in place processes and procedures that provide accountability to stakeholders</skos:definition>
        <skos:topConceptOf rdf:resource="http://data.europa.eu/dr8"/>
    </skos:Concept>

    <skos:Concept rdf:about="http://data.europa.eu/dr8/PreservationOfInformation">
        <skos:notation>PreservationOfInformation</skos:notation>
        <skos:prefLabel xml:lang="en">[ABB387] Preservation of information</skos:prefLabel>
        <skos:definition xml:lang="en">DESCRIPTION:
Legislation requires that decisions and data are stored and can be accessed for a specified time. This means that records and information in electronic form held by public administrations for the purpose of documenting procedures and decisions must be preserved and be converted, where necessary, to new media when old media become obsolete</skos:definition>
        <skos:topConceptOf rdf:resource="http://data.europa.eu/dr8"/>
    </skos:Concept>

    <skos:Concept rdf:about="http://data.europa.eu/dr8/Trust">
        <skos:notation>Trust</skos:notation>
        <skos:prefLabel xml:lang="en">[ABB388] Trust</skos:prefLabel>
        <skos:definition xml:lang="en">DESCRIPTION:
&quot;Administrative Simplification refers to streamlined delivery services. e.g.:
- Harmonised rules on eligibility and durability
- Greater use of simplified costs
- Linking payments with results
- e-Cohesion
- Proportional approach to control
- Simplification of solutions&quot;</skos:definition>
        <skos:topConceptOf rdf:resource="http://data.europa.eu/dr8"/>
    </skos:Concept>

    <skos:Concept rdf:about="http://data.europa.eu/dr8/Innovation">
        <skos:notation>Innovation</skos:notation>
        <skos:prefLabel xml:lang="en">[ABB384] Innovation</skos:prefLabel>
        <skos:definition xml:lang="en">DESCRIPTION:
Innovation entails rethinking organisations and processes, and changing behaviour so that public services are delivered more efficiently to people. Implemented well, eGovernment enables citizens, enterprises and organisations to carry out their business with government more easily, more quickly and at lower cost.</skos:definition>
        <skos:topConceptOf rdf:resource="http://data.europa.eu/dr8"/>
    </skos:Concept>

</rdf:RDF>
